PREFIX dc: <http://purl.org/dc/elements/1.1/>
PREFIX dcterms: <http://purl.org/dc/terms/>
PREFIX geo: <http://www.opengis.net/ont/geosparql#>
PREFIX owl: <http://www.w3.org/2002/07/owl#>
PREFIX rdf: <http://www.w3.org/1999/02/22-rdf-syntax-ns#>
PREFIX rdfs: <http://www.w3.org/2000/01/rdf-schema#>
PREFIX schema: <https://schema.org/>
PREFIX skos: <http://www.w3.org/2004/02/skos/core#>
PREFIX xsd: <http://www.w3.org/2001/XMLSchema#>

<http://anzsoil.org/def/au/asls/substrate/Confidence>
    a
        rdfs:Class ,
        rdfs:Resource ,
        owl:Class ,
        skos:Collection ;
    rdfs:isDefinedBy <http://anzsoil.org/def/au/asls/substrate> ;
    rdfs:seeAlso <http://anzsoil.org/def/au/asls/substrate> ;
    rdfs:subClassOf
        <http://anzsoil.org/def/au/asls/substrate/Confidence> ,
        skos:Concept ;
    skos:definition "The observer should state the degree of confidence that the observed substrate material is in fact the parent material of the observed soil profile or the major part of that profile, that is, of the B horizon." ;
    skos:inScheme <http://anzsoil.org/def/au/asls/substrate> ;
    skos:member
        <http://anzsoil.org/def/au/asls/substrate/confidence-certain> ,
        <http://anzsoil.org/def/au/asls/substrate/confidence-doubtful> ,
        <http://anzsoil.org/def/au/asls/substrate/confidence-not-parent> ,
        <http://anzsoil.org/def/au/asls/substrate/confidence-probable> ;
    skos:prefLabel "Confidence that substrate is parent material - enumeration"@en ;
.

<http://anzsoil.org/def/au/asls/substrate/Field-texture>
    a
        rdfs:Class ,
        rdfs:Resource ,
        owl:Class ,
        skos:Collection ;
    rdfs:isDefinedBy <http://anzsoil.org/def/au/asls/substrate> ;
    rdfs:seeAlso <http://anzsoil.org/def/au/asls/substrate> ;
    rdfs:subClassOf
        <http://anzsoil.org/def/au/asls/substrate/Field-texture> ,
        skos:Concept ;
    skos:definition "Texture - enumeration"@en ;
    skos:inScheme <http://anzsoil.org/def/au/asls/substrate> ;
    skos:member
        <http://anzsoil.org/def/au/asls/substrate/texture-A> ,
        <http://anzsoil.org/def/au/asls/substrate/texture-F> ,
        <http://anzsoil.org/def/au/asls/substrate/texture-P> ,
        <http://anzsoil.org/def/au/asls/substrate/texture-X> ;
    skos:prefLabel "Texture - enumeration"@en ;
.

<http://anzsoil.org/def/au/asls/substrate/Lithology-rock>
    a
        rdfs:Class ,
        rdfs:Resource ,
        owl:Class ,
        skos:Collection ;
    dcterms:source "Table 35 Alphabetical checklist of lithological type of rock material and unconsolidated material." ;
    rdfs:isDefinedBy <http://anzsoil.org/def/au/asls/substrate> ;
    rdfs:seeAlso <http://anzsoil.org/def/au/asls/substrate> ;
    rdfs:subClassOf
        <http://anzsoil.org/def/au/asls/substrate/Lithology-rock> ,
        skos:Concept ;
    skos:definition "Lithological type - rock."@en ;
    skos:inScheme <http://anzsoil.org/def/au/asls/substrate> ;
    skos:member
        <http://anzsoil.org/def/au/asls/substrate/lithology-AC> ,
        <http://anzsoil.org/def/au/asls/substrate/lithology-AD> ,
        <http://anzsoil.org/def/au/asls/substrate/lithology-AF> ,
        <http://anzsoil.org/def/au/asls/substrate/lithology-AG> ,
        <http://anzsoil.org/def/au/asls/substrate/lithology-AH> ,
        <http://anzsoil.org/def/au/asls/substrate/lithology-AM> ,
        <http://anzsoil.org/def/au/asls/substrate/lithology-AN> ,
        <http://anzsoil.org/def/au/asls/substrate/lithology-AP> ,
        <http://anzsoil.org/def/au/asls/substrate/lithology-AR> ,
        <http://anzsoil.org/def/au/asls/substrate/lithology-AS> ,
        <http://anzsoil.org/def/au/asls/substrate/lithology-BA> ,
        <http://anzsoil.org/def/au/asls/substrate/lithology-BB> ,
        <http://anzsoil.org/def/au/asls/substrate/lithology-BR> ,
        <http://anzsoil.org/def/au/asls/substrate/lithology-C> ,
        <http://anzsoil.org/def/au/asls/substrate/lithology-CG> ,
        <http://anzsoil.org/def/au/asls/substrate/lithology-CH> ,
        <http://anzsoil.org/def/au/asls/substrate/lithology-CO> ,
        <http://anzsoil.org/def/au/asls/substrate/lithology-CU> ,
        <http://anzsoil.org/def/au/asls/substrate/lithology-DI> ,
        <http://anzsoil.org/def/au/asls/substrate/lithology-DM> ,
        <http://anzsoil.org/def/au/asls/substrate/lithology-DR> ,
        <http://anzsoil.org/def/au/asls/substrate/lithology-FC> ,
        <http://anzsoil.org/def/au/asls/substrate/lithology-GA> ,
        <http://anzsoil.org/def/au/asls/substrate/lithology-GD> ,
        <http://anzsoil.org/def/au/asls/substrate/lithology-GE> ,
        <http://anzsoil.org/def/au/asls/substrate/lithology-GN> ,
        <http://anzsoil.org/def/au/asls/substrate/lithology-GR> ,
        <http://anzsoil.org/def/au/asls/substrate/lithology-GS> ,
        <http://anzsoil.org/def/au/asls/substrate/lithology-GV> ,
        <http://anzsoil.org/def/au/asls/substrate/lithology-GW> ,
        <http://anzsoil.org/def/au/asls/substrate/lithology-GY> ,
        <http://anzsoil.org/def/au/asls/substrate/lithology-HA> ,
        <http://anzsoil.org/def/au/asls/substrate/lithology-HO> ,
        <http://anzsoil.org/def/au/asls/substrate/lithology-IG> ,
        <http://anzsoil.org/def/au/asls/substrate/lithology-JA> ,
        <http://anzsoil.org/def/au/asls/substrate/lithology-KA> ,
        <http://anzsoil.org/def/au/asls/substrate/lithology-KC> ,
        <http://anzsoil.org/def/au/asls/substrate/lithology-KL> ,
        <http://anzsoil.org/def/au/asls/substrate/lithology-KM> ,
        <http://anzsoil.org/def/au/asls/substrate/lithology-KR> ,
        <http://anzsoil.org/def/au/asls/substrate/lithology-KS> ,
        <http://anzsoil.org/def/au/asls/substrate/lithology-LC> ,
        <http://anzsoil.org/def/au/asls/substrate/lithology-LI> ,
        <http://anzsoil.org/def/au/asls/substrate/lithology-M> ,
        <http://anzsoil.org/def/au/asls/substrate/lithology-MB> ,
        <http://anzsoil.org/def/au/asls/substrate/lithology-MD> ,
        <http://anzsoil.org/def/au/asls/substrate/lithology-ME> ,
        <http://anzsoil.org/def/au/asls/substrate/lithology-MG> ,
        <http://anzsoil.org/def/au/asls/substrate/lithology-MI> ,
        <http://anzsoil.org/def/au/asls/substrate/lithology-ML> ,
        <http://anzsoil.org/def/au/asls/substrate/lithology-MS> ,
        <http://anzsoil.org/def/au/asls/substrate/lithology-MU> ,
        <http://anzsoil.org/def/au/asls/substrate/lithology-MY> ,
        <http://anzsoil.org/def/au/asls/substrate/lithology-PC> ,
        <http://anzsoil.org/def/au/asls/substrate/lithology-PE> ,
        <http://anzsoil.org/def/au/asls/substrate/lithology-PG> ,
        <http://anzsoil.org/def/au/asls/substrate/lithology-PH> ,
        <http://anzsoil.org/def/au/asls/substrate/lithology-PL> ,
        <http://anzsoil.org/def/au/asls/substrate/lithology-PO> ,
        <http://anzsoil.org/def/au/asls/substrate/lithology-PY> ,
        <http://anzsoil.org/def/au/asls/substrate/lithology-QP> ,
        <http://anzsoil.org/def/au/asls/substrate/lithology-QS> ,
        <http://anzsoil.org/def/au/asls/substrate/lithology-QU> ,
        <http://anzsoil.org/def/au/asls/substrate/lithology-QZ> ,
        <http://anzsoil.org/def/au/asls/substrate/lithology-R> ,
        <http://anzsoil.org/def/au/asls/substrate/lithology-RB> ,
        <http://anzsoil.org/def/au/asls/substrate/lithology-RH> ,
        <http://anzsoil.org/def/au/asls/substrate/lithology-S> ,
        <http://anzsoil.org/def/au/asls/substrate/lithology-SA> ,
        <http://anzsoil.org/def/au/asls/substrate/lithology-SD> ,
        <http://anzsoil.org/def/au/asls/substrate/lithology-SH> ,
        <http://anzsoil.org/def/au/asls/substrate/lithology-SK> ,
        <http://anzsoil.org/def/au/asls/substrate/lithology-SL> ,
        <http://anzsoil.org/def/au/asls/substrate/lithology-SR> ,
        <http://anzsoil.org/def/au/asls/substrate/lithology-ST> ,
        <http://anzsoil.org/def/au/asls/substrate/lithology-SY> ,
        <http://anzsoil.org/def/au/asls/substrate/lithology-TR> ,
        <http://anzsoil.org/def/au/asls/substrate/lithology-TU> ,
        <http://anzsoil.org/def/au/asls/substrate/lithology-UC> ,
        <http://anzsoil.org/def/au/asls/substrate/lithology-VB> ,
        <http://anzsoil.org/def/au/asls/substrate/lithology-VG> ,
        <http://anzsoil.org/def/au/asls/substrate/lithology-Z> ,
        <http://anzsoil.org/def/au/asls/substrate/lithology-ZS> ;
    skos:note "C_LITHOLOGY" ;
    skos:prefLabel "Lithological type- rock - enumeration"@en ;
.

<http://anzsoil.org/def/au/asls/substrate/Lithology-unconsolidated>
    a
        rdfs:Class ,
        rdfs:Resource ,
        owl:Class ,
        skos:Collection ;
    dcterms:source "Table 33 Unconsolidated material* classification" ;
    rdfs:isDefinedBy <http://anzsoil.org/def/au/asls/substrate> ;
    rdfs:seeAlso <http://anzsoil.org/def/au/asls/substrate> ;
    rdfs:subClassOf
        <http://anzsoil.org/def/au/asls/substrate/Lithology-unconsolidated> ,
        skos:Concept ;
    skos:definition "Lithological type - unconsoldiated material."@en ;
    skos:inScheme <http://anzsoil.org/def/au/asls/substrate> ;
    skos:member
        <http://anzsoil.org/def/au/asls/substrate/lithology-AF> ,
        <http://anzsoil.org/def/au/asls/substrate/lithology-AS> ,
        <http://anzsoil.org/def/au/asls/substrate/lithology-BB> ,
        <http://anzsoil.org/def/au/asls/substrate/lithology-BO> ,
        <http://anzsoil.org/def/au/asls/substrate/lithology-C> ,
        <http://anzsoil.org/def/au/asls/substrate/lithology-CB> ,
        <http://anzsoil.org/def/au/asls/substrate/lithology-GV> ,
        <http://anzsoil.org/def/au/asls/substrate/lithology-KS> ,
        <http://anzsoil.org/def/au/asls/substrate/lithology-ML> ,
        <http://anzsoil.org/def/au/asls/substrate/lithology-S> ,
        <http://anzsoil.org/def/au/asls/substrate/lithology-SK> ,
        <http://anzsoil.org/def/au/asls/substrate/lithology-SN> ,
        <http://anzsoil.org/def/au/asls/substrate/lithology-Z> ;
    skos:prefLabel "Lithological type- unconsolidated material - enumeration"@en ;
.

<http://anzsoil.org/def/au/asls/substrate/Mass-genetic-type>
    a
        rdfs:Class ,
        rdfs:Resource ,
        owl:Class ,
        skos:Collection ;
    rdfs:isDefinedBy <http://anzsoil.org/def/au/asls/substrate> ;
    rdfs:seeAlso <http://anzsoil.org/def/au/asls/substrate> ;
    rdfs:subClassOf
        <http://anzsoil.org/def/au/asls/substrate/Mass-genetic-type> ,
        skos:Concept ;
    skos:definition "Glossary of substrate mass genetic types"@en ;
    skos:inScheme <http://anzsoil.org/def/au/asls/substrate> ;
    skos:member
        <http://anzsoil.org/def/au/asls/substrate/Rock-genesis-hardened-artificial> ,
        <http://anzsoil.org/def/au/asls/substrate/Rock-genesis-hardened-chemical> ,
        <http://anzsoil.org/def/au/asls/substrate/Rock-genesis-hardened-evaporite> ,
        <http://anzsoil.org/def/au/asls/substrate/Rock-genesis-sediments> ,
        <http://anzsoil.org/def/au/asls/substrate/Rock-genesis-unweathered> ,
        <http://anzsoil.org/def/au/asls/substrate/Rock-genesis-weathered> ;
    skos:prefLabel "Glossary of substrate mass genetic types"@en ;
.

<http://anzsoil.org/def/au/asls/substrate/Material-strength>
    a
        rdfs:Class ,
        rdfs:Resource ,
        owl:Class ,
        skos:Collection ;
    rdfs:isDefinedBy <http://anzsoil.org/def/au/asls/substrate> ;
    rdfs:seeAlso <http://anzsoil.org/def/au/asls/substrate> ;
    rdfs:subClassOf
        <http://anzsoil.org/def/au/asls/substrate/Material-strength> ,
        skos:Concept ;
    skos:definition "The strength of a specimen of soil substrate material may be crudely estimated in the field by striking it with the head-end or the pick-end of a geological hammer or by trying to cut it with a knife, and then referring to Table 32 (ASLS Field Handbook). These estimates refer to the unconfined (or uniaxial) compressive strength. The strength is that of the intact material rather than that of the mass, the strength of which has generally been reduced by the development of fractures and other phenomena."@en ;
    skos:inScheme <http://anzsoil.org/def/au/asls/substrate> ;
    skos:member
        <http://anzsoil.org/def/au/asls/substrate/material-strength-M> ,
        <http://anzsoil.org/def/au/asls/substrate/material-strength-S> ,
        <http://anzsoil.org/def/au/asls/substrate/material-strength-VS> ,
        <http://anzsoil.org/def/au/asls/substrate/material-strength-VW> ,
        <http://anzsoil.org/def/au/asls/substrate/material-strength-W> ;
    skos:note "These are an exact match to coarse fragments strength in land surface chapter"@en ;
    skos:prefLabel "Strength of substrate material - enumeration"@en ;
.

<http://anzsoil.org/def/au/asls/substrate/Rock-alteration>
    a
        rdfs:Class ,
        rdfs:Resource ,
        owl:Class ,
        skos:Collection ;
    rdfs:isDefinedBy <http://anzsoil.org/def/au/asls/substrate> ;
    rdfs:seeAlso <http://anzsoil.org/def/au/asls/substrate> ;
    rdfs:subClassOf
        <http://anzsoil.org/def/au/asls/substrate/Rock-alteration> ,
        skos:Concept ;
    skos:definition "Substrate materials may be so extensively altered (as in deep weathering profiles) that it may be difficult or impossible to determine their original nature. Certain constituents may be either depleted or enriched. Thus, in many laterite profiles, some horizons are ferruginised, partially ferruginised and partially kaolinised, and the pallid zone kaolinised. Silicification may also be associated with deep weathering profiles although not exclusively so; for instance, some limestones may be variably silicified. In contrast, calcification, which is widespread in parts of southern Australia, is not usually associated with deep weathering." ;
    skos:inScheme <http://anzsoil.org/def/au/asls/substrate> ;
    skos:member
        <http://anzsoil.org/def/au/asls/substrate/alteration-F> ,
        <http://anzsoil.org/def/au/asls/substrate/alteration-K> ,
        <http://anzsoil.org/def/au/asls/substrate/alteration-L> ,
        <http://anzsoil.org/def/au/asls/substrate/alteration-O> ,
        <http://anzsoil.org/def/au/asls/substrate/alteration-S> ;
    skos:note "In some instances more than one type of alteration may be present, for example the mottled zone of a laterite profile may be both ferruginised and kaolinised. Where both types of alteration occur, record both." ;
    skos:prefLabel "Alteration - enumeration"@en ;
.

<http://anzsoil.org/def/au/asls/substrate/Rock-genesis-hardened-artificial>
    a
        rdfs:Class ,
        rdfs:Resource ,
        owl:Class ,
        skos:Collection ;
    rdfs:isDefinedBy <http://anzsoil.org/def/au/asls/substrate> ;
    rdfs:seeAlso <http://anzsoil.org/def/au/asls/substrate> ;
    rdfs:subClassOf
        <http://anzsoil.org/def/au/asls/substrate/Rock-genesis-hardened-artificial> ,
        skos:Concept ;
    skos:definition "Artificially hardened materials - enumeration"@en ;
    skos:inScheme <http://anzsoil.org/def/au/asls/substrate> ;
    skos:member
        <http://anzsoil.org/def/au/asls/substrate/genesis-AT> ,
        <http://anzsoil.org/def/au/asls/substrate/genesis-CN> ,
        <http://anzsoil.org/def/au/asls/substrate/genesis-ST> ;
    skos:prefLabel "Artificially hardened materials - enumeration"@en ;
.

<http://anzsoil.org/def/au/asls/substrate/Rock-genesis-hardened-chemical>
    a
        rdfs:Class ,
        rdfs:Resource ,
        owl:Class ,
        skos:Collection ;
    rdfs:isDefinedBy <http://anzsoil.org/def/au/asls/substrate> ;
    rdfs:seeAlso <http://anzsoil.org/def/au/asls/substrate> ;
    rdfs:subClassOf
        <http://anzsoil.org/def/au/asls/substrate/Rock-genesis-hardened-chemical> ,
        skos:Concept ;
    skos:definition "Chemically hardened materials - enumeration"@en ;
    skos:inScheme <http://anzsoil.org/def/au/asls/substrate> ;
    skos:member
        <http://anzsoil.org/def/au/asls/substrate/genesis-AC> ,
        <http://anzsoil.org/def/au/asls/substrate/genesis-FC> ,
        <http://anzsoil.org/def/au/asls/substrate/genesis-KC> ,
        <http://anzsoil.org/def/au/asls/substrate/genesis-LC> ,
        <http://anzsoil.org/def/au/asls/substrate/genesis-PC> ,
        <http://anzsoil.org/def/au/asls/substrate/genesis-RB> ;
    skos:prefLabel "Chemically hardened materials - enumeration"@en ;
.

<http://anzsoil.org/def/au/asls/substrate/Rock-genesis-hardened-evaporite>
    a
        rdfs:Class ,
        rdfs:Resource ,
        owl:Class ,
        skos:Collection ;
    rdfs:isDefinedBy <http://anzsoil.org/def/au/asls/substrate> ;
    rdfs:seeAlso <http://anzsoil.org/def/au/asls/substrate> ;
    rdfs:subClassOf
        <http://anzsoil.org/def/au/asls/substrate/Rock-genesis-hardened-evaporite> ,
        skos:Concept ;
    skos:definition "Evaporites - enumeration"@en ;
    skos:inScheme <http://anzsoil.org/def/au/asls/substrate> ;
    skos:member
        <http://anzsoil.org/def/au/asls/substrate/genesis-EV> ,
        <http://anzsoil.org/def/au/asls/substrate/genesis-GY> ,
        <http://anzsoil.org/def/au/asls/substrate/genesis-HA> ;
    skos:prefLabel "Evaporites - enumeration"@en ;
.

<http://anzsoil.org/def/au/asls/substrate/Rock-genesis-sediments>
    a
        rdfs:Class ,
        rdfs:Resource ,
        owl:Class ,
        skos:Collection ;
    rdfs:isDefinedBy <http://anzsoil.org/def/au/asls/substrate> ;
    rdfs:seeAlso <http://anzsoil.org/def/au/asls/substrate> ;
    rdfs:subClassOf
        <http://anzsoil.org/def/au/asls/substrate/Rock-genesis-sediments> ,
        skos:Concept ;
    skos:definition "Sediments (unconsolidated) - enumeration"@en ;
    skos:inScheme <http://anzsoil.org/def/au/asls/substrate> ;
    skos:member
        <http://anzsoil.org/def/au/asls/substrate/genesis-AL> ,
        <http://anzsoil.org/def/au/asls/substrate/genesis-BE> ,
        <http://anzsoil.org/def/au/asls/substrate/genesis-CD> ,
        <http://anzsoil.org/def/au/asls/substrate/genesis-CO> ,
        <http://anzsoil.org/def/au/asls/substrate/genesis-ED> ,
        <http://anzsoil.org/def/au/asls/substrate/genesis-ES> ,
        <http://anzsoil.org/def/au/asls/substrate/genesis-FI> ,
        <http://anzsoil.org/def/au/asls/substrate/genesis-GY> ,
        <http://anzsoil.org/def/au/asls/substrate/genesis-LA> ,
        <http://anzsoil.org/def/au/asls/substrate/genesis-LD> ,
        <http://anzsoil.org/def/au/asls/substrate/genesis-LO> ,
        <http://anzsoil.org/def/au/asls/substrate/genesis-MA> ,
        <http://anzsoil.org/def/au/asls/substrate/genesis-MD> ,
        <http://anzsoil.org/def/au/asls/substrate/genesis-PA> ,
        <http://anzsoil.org/def/au/asls/substrate/genesis-SE> ,
        <http://anzsoil.org/def/au/asls/substrate/genesis-SH> ,
        <http://anzsoil.org/def/au/asls/substrate/genesis-TI> ,
        <http://anzsoil.org/def/au/asls/substrate/genesis-VA> ;
    skos:notation "3" ;
    skos:prefLabel "Sediments (unconsolidated) - enumeration"@en ;
.

<http://anzsoil.org/def/au/asls/substrate/Rock-genesis-unweathered>
    a
        rdfs:Class ,
        rdfs:Resource ,
        owl:Class ,
        skos:Collection ;
    rdfs:isDefinedBy <http://anzsoil.org/def/au/asls/substrate> ;
    rdfs:seeAlso <http://anzsoil.org/def/au/asls/substrate> ;
    rdfs:subClassOf
        <http://anzsoil.org/def/au/asls/substrate/Rock-genesis-unweathered> ,
        skos:Concept ;
    skos:definition "Unweathered rocks of the bedrock zone - enumeration"@en ;
    skos:inScheme <http://anzsoil.org/def/au/asls/substrate> ;
    skos:member
        <http://anzsoil.org/def/au/asls/substrate/genesis-ET> ,
        <http://anzsoil.org/def/au/asls/substrate/genesis-IG> ,
        <http://anzsoil.org/def/au/asls/substrate/genesis-IN> ,
        <http://anzsoil.org/def/au/asls/substrate/genesis-ME> ,
        <http://anzsoil.org/def/au/asls/substrate/genesis-PL> ,
        <http://anzsoil.org/def/au/asls/substrate/genesis-SC> ,
        <http://anzsoil.org/def/au/asls/substrate/genesis-SD> ,
        <http://anzsoil.org/def/au/asls/substrate/genesis-SP> ,
        <http://anzsoil.org/def/au/asls/substrate/genesis-SR> ,
        <http://anzsoil.org/def/au/asls/substrate/genesis-VO> ;
    skos:notation "1" ;
    skos:prefLabel "Unweathered rocks of the bedrock zone - enumeration"@en ;
.

<http://anzsoil.org/def/au/asls/substrate/Rock-genesis-weathered>
    a
        rdfs:Class ,
        rdfs:Resource ,
        owl:Class ,
        skos:Collection ;
    rdfs:isDefinedBy <http://anzsoil.org/def/au/asls/substrate> ;
    rdfs:seeAlso <http://anzsoil.org/def/au/asls/substrate> ;
    rdfs:subClassOf
        <http://anzsoil.org/def/au/asls/substrate/Rock-genesis-weathered> ,
        skos:Concept ;
    skos:definition "Weathered rocks - enumeration"@en ;
    skos:inScheme <http://anzsoil.org/def/au/asls/substrate> ;
    skos:member
        <http://anzsoil.org/def/au/asls/substrate/genesis-DR> ,
        <http://anzsoil.org/def/au/asls/substrate/genesis-PW> ,
        <http://anzsoil.org/def/au/asls/substrate/genesis-SA> ;
    skos:notation "2" ;
    skos:prefLabel "Weathered rocks - enumeration"@en ;
.

<http://anzsoil.org/def/au/asls/substrate/Substrate-discontinuity-spacing>
    a
        rdfs:Class ,
        rdfs:Resource ,
        owl:Class ,
        skos:Collection ;
    rdfs:isDefinedBy <http://anzsoil.org/def/au/asls/substrate> ;
    rdfs:seeAlso <http://anzsoil.org/def/au/asls/substrate> ;
    rdfs:subClassOf
        <http://anzsoil.org/def/au/asls/substrate/Substrate-discontinuity-spacing> ,
        skos:Concept ;
    skos:definition "Physical weathering opens up fissures or joints that reduce the strength of the rock mass relative to that of the intact rock material.  These fissures generally increase in number towards the land surface.  The following categories of discontinuity spacing apply (Deere 1968, Selby 1982):" ;
    skos:inScheme <http://anzsoil.org/def/au/asls/substrate> ;
    skos:member
        <http://anzsoil.org/def/au/asls/substrate/discontinuity-spacing-B> ,
        <http://anzsoil.org/def/au/asls/substrate/discontinuity-spacing-C> ,
        <http://anzsoil.org/def/au/asls/substrate/discontinuity-spacing-F> ,
        <http://anzsoil.org/def/au/asls/substrate/discontinuity-spacing-M> ,
        <http://anzsoil.org/def/au/asls/substrate/discontinuity-spacing-S> ;
    skos:prefLabel "Spacing of discontinuities - enumeration"@en ;
.

<http://anzsoil.org/def/au/asls/substrate/Substrate-grain-size>
    a
        rdfs:Class ,
        rdfs:Resource ,
        owl:Class ,
        skos:Collection ;
    rdfs:isDefinedBy <http://anzsoil.org/def/au/asls/substrate> ;
    rdfs:seeAlso <http://anzsoil.org/def/au/asls/substrate> ;
    rdfs:subClassOf
        <http://anzsoil.org/def/au/asls/substrate/Substrate-grain-size> ,
        skos:Concept ;
    skos:definition "It is informative to estimate the size of the most common particles of a substrate material whether the material is thought to be of sedimentary, metamorphic or igneous origin." ;
    skos:inScheme <http://anzsoil.org/def/au/asls/substrate> ;
    skos:member
        <http://anzsoil.org/def/au/asls/substrate/grain-size-1> ,
        <http://anzsoil.org/def/au/asls/substrate/grain-size-2> ,
        <http://anzsoil.org/def/au/asls/substrate/grain-size-3> ;
    skos:note "* As shown by Figure 15, page 116, these size grade limits agree with the scale of Wentworth (1922), adopted by the United States National Research Council (Pettijohn 1957) and the American Geophysical Union (Lane et al. 1947), and with that of the Massachusetts Institute of Technology, also adopted by the British Standards Institution (1975) and the Standards Association of Australia (1977). The 0.06 mm boundary criterion (strictly 0.063 mm) separating sand and silt differs markedly from the value 0.02 mm of the International Scheme (proposed originally by Atterberg (1905) and accepted by the International Society of Soil Science); the 0.05 mm value of the United States Department of Agriculture (Soil Survey Staff 1975); and the 0.075 mm value of the Unified Soil Classification (Anon. 1953)." ;
    skos:prefLabel "Grain size - enumeration"@en ;
.

<http://anzsoil.org/def/au/asls/substrate/Substrate-mineral-composition>
    a
        rdfs:Class ,
        rdfs:Resource ,
        owl:Class ,
        skos:Collection ;
    rdfs:isDefinedBy <http://anzsoil.org/def/au/asls/substrate> ;
    rdfs:seeAlso <http://anzsoil.org/def/au/asls/substrate> ;
    rdfs:subClassOf
        <http://anzsoil.org/def/au/asls/substrate/Substrate-mineral-composition> ,
        skos:Concept ;
    skos:definition "Make provision for recording one dominant mineral and one or two minor minerals, as identified by inspection of the hand specimen." ;
    skos:inScheme <http://anzsoil.org/def/au/asls/substrate> ;
    skos:member
        <http://anzsoil.org/def/au/asls/substrate/mineral-composition-C> ,
        <http://anzsoil.org/def/au/asls/substrate/mineral-composition-D> ,
        <http://anzsoil.org/def/au/asls/substrate/mineral-composition-F> ,
        <http://anzsoil.org/def/au/asls/substrate/mineral-composition-G> ,
        <http://anzsoil.org/def/au/asls/substrate/mineral-composition-K> ,
        <http://anzsoil.org/def/au/asls/substrate/mineral-composition-L> ,
        <http://anzsoil.org/def/au/asls/substrate/mineral-composition-M> ,
        <http://anzsoil.org/def/au/asls/substrate/mineral-composition-Q> ,
        <http://anzsoil.org/def/au/asls/substrate/mineral-composition-S> ,
        <http://anzsoil.org/def/au/asls/substrate/mineral-composition-Y> ;
    skos:prefLabel "Mineral composition - enumeration"@en ;
.

<http://anzsoil.org/def/au/asls/substrate/Substrate-porosity>
    a
        rdfs:Class ,
        rdfs:Resource ,
        owl:Class ,
        skos:Collection ;
    rdfs:isDefinedBy <http://anzsoil.org/def/au/asls/substrate> ;
    rdfs:seeAlso <http://anzsoil.org/def/au/asls/substrate> ;
    rdfs:subClassOf
        <http://anzsoil.org/def/au/asls/substrate/Substrate-porosity> ,
        skos:Concept ;
    skos:definition "Porosity - enumeration"@en ;
    skos:inScheme <http://anzsoil.org/def/au/asls/substrate> ;
    skos:member
        <http://anzsoil.org/def/au/asls/substrate/porosity-0> ,
        <http://anzsoil.org/def/au/asls/substrate/porosity-1> ,
        <http://anzsoil.org/def/au/asls/substrate/porosity-2> ;
    skos:prefLabel "Porosity - enumeration"@en ;
.

<http://anzsoil.org/def/au/asls/substrate/Substrate-structure>
    a
        rdfs:Class ,
        rdfs:Resource ,
        owl:Class ,
        skos:Collection ;
    rdfs:isDefinedBy <http://anzsoil.org/def/au/asls/substrate> ;
    rdfs:seeAlso <http://anzsoil.org/def/au/asls/substrate> ;
    rdfs:subClassOf
        <http://anzsoil.org/def/au/asls/substrate/Substrate-structure> ,
        skos:Concept ;
    skos:definition "Structure - enumeration"@en ;
    skos:inScheme <http://anzsoil.org/def/au/asls/substrate> ;
    skos:member
        <http://anzsoil.org/def/au/asls/substrate/material-structure-B> ,
        <http://anzsoil.org/def/au/asls/substrate/material-structure-C> ,
        <http://anzsoil.org/def/au/asls/substrate/material-structure-F> ,
        <http://anzsoil.org/def/au/asls/substrate/material-structure-L> ,
        <http://anzsoil.org/def/au/asls/substrate/material-structure-P> ,
        <http://anzsoil.org/def/au/asls/substrate/material-structure-R> ,
        <http://anzsoil.org/def/au/asls/substrate/material-structure-S> ,
        <http://anzsoil.org/def/au/asls/substrate/material-structure-V> ;
    skos:prefLabel "Structure - enumeration"@en ;
.

<http://anzsoil.org/def/au/asls/substrate/sampling>
    a
        rdfs:Class ,
        rdfs:Resource ,
        skos:Collection ;
    rdfs:isDefinedBy <http://anzsoil.org/def/au/asls/substrate> ;
    rdfs:seeAlso <http://anzsoil.org/def/au/asls/substrate> ;
    skos:definition "Properties of substrate sampling"@en ;
    skos:inScheme <http://anzsoil.org/def/au/asls/substrate> ;
    skos:member
        <http://anzsoil.org/def/au/asls/substrate/Confidence> ,
        <http://anzsoil.org/def/au/asls/substrate/observation-depth> ,
        <http://anzsoil.org/def/au/asls/substrate/sample-distance> ,
        <http://anzsoil.org/def/au/asls/substrate/type-of-substrate-observation> ;
    skos:prefLabel "Properties of substrate sampling"@en ;
.

<http://anzsoil.org/def/au/asls/substrate/type-of-substrate-observation>
    a
        rdfs:Class ,
        rdfs:Resource ,
        owl:Class ,
        skos:Collection ;
    rdfs:isDefinedBy <http://anzsoil.org/def/au/asls/substrate> ;
    rdfs:seeAlso <http://anzsoil.org/def/au/asls/substrate> ;
    rdfs:subClassOf
        <http://anzsoil.org/def/au/asls/substrate/type-of-substrate-observation> ,
        skos:Concept ;
    skos:definition "The substrate may be described using several types of observation."@en ;
    skos:inScheme <http://anzsoil.org/def/au/asls/substrate> ;
    skos:member
        <http://anzsoil.org/def/au/asls/substrate/observation-type-A> ,
        <http://anzsoil.org/def/au/asls/substrate/observation-type-C> ,
        <http://anzsoil.org/def/au/asls/substrate/observation-type-E> ,
        <http://anzsoil.org/def/au/asls/substrate/observation-type-O> ,
        <http://anzsoil.org/def/au/asls/substrate/observation-type-P> ;
    skos:prefLabel "Type of substrate observation - enumeration"@en ;
.

geo:Feature
    a
        rdfs:Class ,
        rdfs:Resource ,
        owl:Class ;
    rdfs:label "Feature"@en ;
    dc:contributor "Matthew Perry" ;
    dc:creator "OGC GeoSPARQL 1.0 Standard Working Group" ;
    dc:date "2011-06-16"^^xsd:date ;
    dc:description """
      This class represents the top-level feature type. This class is 
      equivalent to GFI_Feature defined in ISO 19156:2011, and it is 
      superclass of all feature types.
    """@en ;
    rdfs:comment """
      This class represents the top-level feature type. This class is 
      equivalent to GFI_Feature defined in ISO 19156:2011, and it is 
      superclass of all feature types.
    """@en ;
    rdfs:isDefinedBy
        <http://www.opengis.net/ont/geosparql> ,
        <http://www.opengis.net/spec/geosparql/1.0> ;
    rdfs:seeAlso
        <http://www.opengis.net/ont/geosparql> ,
        <http://www.opengis.net/spec/geosparql/1.0> ;
    rdfs:subClassOf
        geo:Feature ,
        geo:SpatialObject ;
    owl:disjointWith geo:Geometry ;
    skos:definition """
      This class represents the top-level feature type. This class is 
      equivalent to GFI_Feature defined in ISO 19156:2011, and it is 
      superclass of all feature types.
    """@en ;
    skos:prefLabel "Feature"@en ;
.

geo:Geometry
    a
        rdfs:Class ,
        rdfs:Resource ,
        owl:Class ;
    rdfs:label "Geometry"@en ;
    dc:contributor "Matthew Perry" ;
    dc:creator "OGC GeoSPARQL 1.0 Standard Working Group" ;
    dc:date "2011-06-16"^^xsd:date ;
    dc:description """
      The class represents the top-level geometry type. This class is 
      equivalent to the UML class GM_Object defined in ISO 19107, and 
      it is superclass of all geometry types.
    """@en ;
    rdfs:comment """
      The class represents the top-level geometry type. This class is 
      equivalent to the UML class GM_Object defined in ISO 19107, and 
      it is superclass of all geometry types.
    """@en ;
    rdfs:isDefinedBy
        <http://www.opengis.net/ont/geosparql> ,
        <http://www.opengis.net/spec/geosparql/1.0> ;
    rdfs:seeAlso
        <http://www.opengis.net/ont/geosparql> ,
        <http://www.opengis.net/spec/geosparql/1.0> ;
    rdfs:subClassOf
        geo:Geometry ,
        geo:SpatialObject ;
    owl:disjointWith geo:Feature ;
    skos:definition """
      The class represents the top-level geometry type. This class is 
      equivalent to the UML class GM_Object defined in ISO 19107, and 
      it is superclass of all geometry types.
    """@en ;
    skos:prefLabel "Geometry"@en ;
.

geo:SpatialObject
    a
        rdfs:Class ,
        rdfs:Resource ,
        owl:Class ;
    rdfs:label "SpatialObject"@en ;
    dc:contributor "Matthew Perry" ;
    dc:creator "OGC GeoSPARQL 1.0 Standard Working Group" ;
    dc:date "2011-06-16"^^xsd:date ;
    dc:description """
      The class spatial-object represents everything that can have 
      a spatial representation. It is superclass of feature and geometry.
    """@en ;
    rdfs:comment """
      The class spatial-object represents everything that can have 
      a spatial representation. It is superclass of feature and geometry.
    """@en ;
    rdfs:isDefinedBy
        <http://www.opengis.net/ont/geosparql> ,
        <http://www.opengis.net/spec/geosparql/1.0> ;
    rdfs:seeAlso
        <http://www.opengis.net/ont/geosparql> ,
        <http://www.opengis.net/spec/geosparql/1.0> ;
    rdfs:subClassOf
        geo:SpatialObject ,
        rdfs:Resource ;
    skos:definition """
      The class spatial-object represents everything that can have 
      a spatial representation. It is superclass of feature and geometry.
    """@en ;
    skos:prefLabel "SpatialObject"@en ;
.

geo:gmlLiteral
    a
        rdfs:Class ,
        rdfs:Datatype ,
        rdfs:Resource ;
    rdfs:label "GML Literal"@en ;
    dc:contributor "Matthew Perry" ;
    dc:creator "OGC GeoSPARQL 1.0 Standard Working Group" ;
    dc:date "2011-06-16"^^xsd:date ;
    dc:description """
      A GML serialization of a geometry object.
    """@en ;
    rdfs:comment """
      A GML serialization of a geometry object.
    """@en ;
    rdfs:isDefinedBy
        <http://www.opengis.net/ont/geosparql> ,
        <http://www.opengis.net/spec/geosparql/1.0> ;
    rdfs:seeAlso
        <http://www.opengis.net/ont/geosparql> ,
        <http://www.opengis.net/spec/geosparql/1.0> ;
    rdfs:subClassOf
        geo:gmlLiteral ,
        rdfs:Resource ;
    skos:definition """
      A GML serialization of a geometry object.
    """@en ;
    skos:prefLabel "GML Literal"@en ;
.

geo:wktLiteral
    a
        rdfs:Class ,
        rdfs:Datatype ,
        rdfs:Resource ;
    rdfs:label "Well-known Text Literal"@en ;
    dc:contributor "Matthew Perry" ;
    dc:creator "OGC GeoSPARQL 1.0 Standard Working Group" ;
    dc:date "2011-06-16"^^xsd:date ;
    dc:description """
      A Well-known Text serialization of a geometry object.
    """@en ;
    rdfs:comment """
      A Well-known Text serialization of a geometry object.
    """@en ;
    rdfs:isDefinedBy
        <http://www.opengis.net/ont/geosparql> ,
        <http://www.opengis.net/spec/geosparql/1.0> ;
    rdfs:seeAlso
        <http://www.opengis.net/ont/geosparql> ,
        <http://www.opengis.net/spec/geosparql/1.0> ;
    rdfs:subClassOf
        geo:wktLiteral ,
        rdfs:Resource ;
    skos:definition """
      A Well-known Text serialization of a geometry object.
    """@en ;
    skos:prefLabel "Well-known Text Literal"@en ;
.

rdf:Alt
    a
        rdfs:Class ,
        rdfs:Resource ;
    rdfs:subClassOf
        rdf:Alt ,
        rdfs:Container ;
.

rdf:Bag
    a
        rdfs:Class ,
        rdfs:Resource ;
    rdfs:subClassOf
        rdf:Bag ,
        rdfs:Container ;
.

rdf:List
    a
        rdfs:Class ,
        rdfs:Resource ;
    rdfs:subClassOf rdfs:Resource ;
.

rdf:Property
    a
        rdfs:Class ,
        rdfs:Resource ;
    rdfs:subClassOf
        rdf:Property ,
        rdfs:Resource ;
.

rdf:Seq
    a
        rdfs:Class ,
        rdfs:Resource ;
    rdfs:subClassOf
        rdf:Seq ,
        rdfs:Container ;
.

rdf:Statement
    a
        rdfs:Class ,
        rdfs:Resource ;
    rdfs:subClassOf rdfs:Resource ;
.

rdf:XMLLiteral
    a
        rdfs:Class ,
        rdfs:Datatype ,
        rdfs:Resource ;
.

rdfs:Class
    a
        rdfs:Class ,
        rdfs:Resource ;
    rdfs:subClassOf
        rdfs:Class ,
        rdfs:Resource ;
.

rdfs:Container
    a
        rdfs:Class ,
        rdfs:Resource ;
    rdfs:subClassOf rdfs:Container ;
.

rdfs:ContainerMembershipProperty
    a
        rdfs:Class ,
        rdfs:Resource ;
    rdfs:subClassOf
        rdf:Property ,
        rdfs:ContainerMembershipProperty ;
.

rdfs:Datatype
    a
        rdfs:Class ,
        rdfs:Resource ;
    rdfs:subClassOf
        rdfs:Class ,
        rdfs:Datatype ;
.

rdfs:Literal
    a
        rdfs:Class ,
        rdfs:Resource ;
    rdfs:subClassOf rdfs:Resource ;
.

rdfs:Resource
    a
        rdfs:Class ,
        rdfs:Resource ;
.

xsd:boolean
    a
        rdfs:Class ,
        rdfs:Resource ;
    rdfs:subClassOf
        rdfs:Resource ,
        xsd:boolean ;
.

xsd:integer
    a
        rdfs:Class ,
        rdfs:Resource ;
    rdfs:subClassOf
        rdfs:Resource ,
        xsd:integer ;
.

owl:Class
    a
        rdfs:Class ,
        rdfs:Resource ;
.

owl:DatatypeProperty
    a
        rdfs:Class ,
        rdfs:Resource ;
.

owl:ObjectProperty
    a
        rdfs:Class ,
        rdfs:Resource ;
.

owl:Ontology
    a
        rdfs:Class ,
        rdfs:Resource ;
.

skos:Collection
    a
        rdfs:Class ,
        rdfs:Resource ;
.

skos:Concept
    a
        rdfs:Class ,
        rdfs:Resource ;
    rdfs:subClassOf skos:Concept ;
.

skos:ConceptScheme
    a
        rdfs:Class ,
        rdfs:Resource ;
.

schema:Person
    a
        rdfs:Class ,
        rdfs:Resource ;
.

<http://anzsoil.org/def/au/asls/substrate/Genesis>
    a skos:Collection ;
    rdfs:isDefinedBy <http://anzsoil.org/def/au/asls/substrate> ;
    rdfs:seeAlso <http://anzsoil.org/def/au/asls/substrate> ;
    skos:definition """Scheme of classification

Table 37 presents a scheme of classification of soil substrate masses as they are found in soil and land surveys. The main classes represent rock masses not yet weathered, those now being weathered, those transported and deposited but not yet consolidated, and those hardened while still near the surface.

Named classes in this table are defined in the following glossary. Since this is a genetic classification, diagnostic attributes may be hard to specify. Associated landforms should not be used as recognition criteria for observed substrate masses. They can be used to infer the nature of substrate masses that cannot be observed. In the same way, substrate observations should not be used as recognition criteria for landforms.""" ;
    skos:inScheme <http://anzsoil.org/def/au/asls/substrate> ;
    skos:member
        <http://anzsoil.org/def/au/asls/substrate/Mass-genetic-type> ,
        <http://anzsoil.org/def/au/asls/substrate/Rock-genesis-sediments> ,
        <http://anzsoil.org/def/au/asls/substrate/Rock-genesis-unweathered> ,
        <http://anzsoil.org/def/au/asls/substrate/Rock-genesis-weathered> ,
        <http://anzsoil.org/def/au/asls/substrate/genesis-hardened> ;
    skos:note """Bedrock and regolith zones

The mantle of earth and rock, including weathered rocks and sediments, altered or formed by land surface processes is called the regolith. The underlying zone of rocks formed or altered by deep-seated crustal processes is the bedrock. Regolith and bedrock are regarded here as zones characterised by different processes, rather than as classes of material. The original definition of regolith by Merrill (1897) stresses the latter view and includes only unconsolidated materials.

The depth of the regolith zone ranges from zero, where bedrock outcrops at the surface, to over 100 m in areas of deep weathering (Ollier 1984).

In areas without much sediment, the lower boundary of the regolith is the weathering front (Mabbutt 1961) where features due to weathering first appear. Where sediments are very thick, their lower layers become isolated from land surface processes by their depth and by reduced permeability due to compaction. Here the base of the regolith, which could be called a ‘lithification front’, is where most of the sediments transform to sedimentary rocks. Sedimentary rocks are often folded and faulted but, at least in Australia’s stable environment, most unconsolidated sediments remain flat-lying.

Masses within the regolith zone, in contrast with those within the bedrock zone, tend to have low density, very low strength, and little cohesion between their particles or fragments. Despite Merrill’s definition, not all materials follow this tendency. Strong and cohesive masses (for example ferricrete) may be characteristic of the regolith. On the other hand, some layers of sedimentary rock never become strong. Other rocks are weakened within the bedrock zone by deep-seated processes. Table 36 assigns types of substrate mass to either the regolith zone or the bedrock zone.""" ;
    skos:prefLabel "Genetic type of substrate masses"@en ;
.

<http://anzsoil.org/def/au/asls/substrate/mass>
    a skos:Collection ;
    rdfs:isDefinedBy <http://anzsoil.org/def/au/asls/substrate> ;
    rdfs:seeAlso <http://anzsoil.org/def/au/asls/substrate> ;
    skos:definition "These properties generally require observation of a near-vertical face 1 m2 or more in area." ;
    skos:inScheme <http://anzsoil.org/def/au/asls/substrate> ;
    skos:member
        <http://anzsoil.org/def/au/asls/substrate/Rock-alteration> ,
        <http://anzsoil.org/def/au/asls/substrate/Substrate-discontinuity-spacing> ;
    skos:prefLabel "Properties of substrate masses"@en ;
.

<http://anzsoil.org/def/au/asls/substrate/material>
    a skos:Collection ;
    rdfs:isDefinedBy <http://anzsoil.org/def/au/asls/substrate> ;
    rdfs:seeAlso <http://anzsoil.org/def/au/asls/substrate> ;
    skos:definition "The properties in this section refer to intact hand-size samples or very small areas of outcrop. In many cases it will be necessary to use a x10 hand lens to determine some of them."@en ;
    skos:inScheme <http://anzsoil.org/def/au/asls/substrate> ;
    skos:member
        <http://anzsoil.org/def/au/asls/substrate/Field-texture> ,
        <http://anzsoil.org/def/au/asls/substrate/Material-strength> ,
        <http://anzsoil.org/def/au/asls/substrate/Substrate-grain-size> ,
        <http://anzsoil.org/def/au/asls/substrate/Substrate-mineral-composition> ,
        <http://anzsoil.org/def/au/asls/substrate/Substrate-porosity> ,
        <http://anzsoil.org/def/au/asls/substrate/Substrate-structure> ,
        <http://anzsoil.org/def/au/asls/substrate/lithology> ;
    skos:prefLabel "Properties of substrate material"@en ;
.

geo:coordinateDimension
    a
        rdf:Property ,
        rdfs:Resource ,
        owl:DatatypeProperty ;
    rdfs:label "coordinateDimension"@en ;
    dc:contributor "Matthew Perry" ;
    dc:creator "OGC GeoSPARQL 1.0 Standard Working Group" ;
    dc:date "2011-06-16"^^xsd:date ;
    dc:description """
      The number of measurements or axes needed to describe the position of this
      geometry in a coordinate system.
    """@en ;
    rdfs:comment """
      The number of measurements or axes needed to describe the position of this
      geometry in a coordinate system.
    """@en ;
    rdfs:domain geo:Geometry ;
    rdfs:isDefinedBy
        <http://www.opengis.net/ont/geosparql> ,
        <http://www.opengis.net/spec/geosparql/1.0> ;
    rdfs:range xsd:integer ;
    rdfs:seeAlso
        <http://www.opengis.net/ont/geosparql> ,
        <http://www.opengis.net/spec/geosparql/1.0> ;
    skos:definition """
      The number of measurements or axes needed to describe the position of this
      geometry in a coordinate system.
    """@en ;
    skos:prefLabel "coordinateDimension"@en ;
.

geo:dimension
    a
        rdf:Property ,
        rdfs:Resource ,
        owl:DatatypeProperty ;
    rdfs:label "dimension"@en ;
    dc:contributor "Matthew Perry" ;
    dc:creator "OGC GeoSPARQL 1.0 Standard Working Group" ;
    dc:date "2011-06-16"^^xsd:date ;
    dc:description """
      The topological dimension of this geometric object, which 
      must be less than or equal to the coordinate dimension. 
      In non-homogeneous collections, this will return the largest 
      topological dimension of the contained objects.
    """@en ;
    rdfs:comment """
      The topological dimension of this geometric object, which 
      must be less than or equal to the coordinate dimension. 
      In non-homogeneous collections, this will return the largest 
      topological dimension of the contained objects.
    """@en ;
    rdfs:domain geo:Geometry ;
    rdfs:isDefinedBy
        <http://www.opengis.net/ont/geosparql> ,
        <http://www.opengis.net/spec/geosparql/1.0> ;
    rdfs:range xsd:integer ;
    rdfs:seeAlso
        <http://www.opengis.net/ont/geosparql> ,
        <http://www.opengis.net/spec/geosparql/1.0> ;
    skos:definition """
      The topological dimension of this geometric object, which 
      must be less than or equal to the coordinate dimension. 
      In non-homogeneous collections, this will return the largest 
      topological dimension of the contained objects.
    """@en ;
    skos:prefLabel "dimension"@en ;
.

geo:ehContains
    a
        rdf:Property ,
        rdfs:Resource ,
        owl:ObjectProperty ;
    rdfs:label "contains"@en ;
    dc:contributor "Matthew Perry" ;
    dc:creator "OGC GeoSPARQL 1.0 Standard Working Group" ;
    dc:date "2011-06-16"^^xsd:date ;
    dc:description """
      Exists if the subject SpatialObject spatially contains the 
      object SpatialObject. DE-9IM: T*TFF*FF*
    """@en ;
    rdfs:comment """
      Exists if the subject SpatialObject spatially contains the 
      object SpatialObject. DE-9IM: T*TFF*FF*
    """@en ;
    rdfs:domain geo:SpatialObject ;
    rdfs:isDefinedBy
        <http://www.opengis.net/ont/geosparql> ,
        <http://www.opengis.net/spec/geosparql/1.0> ;
    rdfs:range geo:SpatialObject ;
    rdfs:seeAlso
        <http://www.opengis.net/ont/geosparql> ,
        <http://www.opengis.net/spec/geosparql/1.0> ;
    skos:definition """
      Exists if the subject SpatialObject spatially contains the 
      object SpatialObject. DE-9IM: T*TFF*FF*
    """@en ;
    skos:prefLabel "contains"@en ;
.

geo:ehCoveredBy
    a
        rdf:Property ,
        rdfs:Resource ,
        owl:ObjectProperty ;
    rdfs:label "coveredBy"@en ;
    dc:contributor "Matthew Perry" ;
    dc:creator "OGC GeoSPARQL 1.0 Standard Working Group" ;
    dc:date "2011-06-16"^^xsd:date ;
    dc:description """
      Exists if the subject SpatialObject is spatially covered 
      by the object SpatialObject. DE-9IM: TFF*TFT**
    """@en ;
    rdfs:comment """
      Exists if the subject SpatialObject is spatially covered 
      by the object SpatialObject. DE-9IM: TFF*TFT**
    """@en ;
    rdfs:domain geo:SpatialObject ;
    rdfs:isDefinedBy
        <http://www.opengis.net/ont/geosparql> ,
        <http://www.opengis.net/spec/geosparql/1.0> ;
    rdfs:range geo:SpatialObject ;
    rdfs:seeAlso
        <http://www.opengis.net/ont/geosparql> ,
        <http://www.opengis.net/spec/geosparql/1.0> ;
    skos:definition """
      Exists if the subject SpatialObject is spatially covered 
      by the object SpatialObject. DE-9IM: TFF*TFT**
    """@en ;
    skos:prefLabel "coveredBy"@en ;
.

geo:ehCovers
    a
        rdf:Property ,
        rdfs:Resource ,
        owl:ObjectProperty ;
    rdfs:label "covers"@en ;
    dc:contributor "Matthew Perry" ;
    dc:creator "OGC GeoSPARQL 1.0 Standard Working Group" ;
    dc:date "2011-06-16"^^xsd:date ;
    dc:description """
      Exists if the subject SpatialObject spatially covers the 
      object SpatialObject. DE-9IM: T*TFT*FF*
    """@en ;
    rdfs:comment """
      Exists if the subject SpatialObject spatially covers the 
      object SpatialObject. DE-9IM: T*TFT*FF*
    """@en ;
    rdfs:domain geo:SpatialObject ;
    rdfs:isDefinedBy
        <http://www.opengis.net/ont/geosparql> ,
        <http://www.opengis.net/spec/geosparql/1.0> ;
    rdfs:range geo:SpatialObject ;
    rdfs:seeAlso
        <http://www.opengis.net/ont/geosparql> ,
        <http://www.opengis.net/spec/geosparql/1.0> ;
    skos:definition """
      Exists if the subject SpatialObject spatially covers the 
      object SpatialObject. DE-9IM: T*TFT*FF*
    """@en ;
    skos:prefLabel "covers"@en ;
.

geo:ehDisjoint
    a
        rdf:Property ,
        rdfs:Resource ,
        owl:ObjectProperty ;
    rdfs:label "disjoint"@en ;
    dc:contributor "Matthew Perry" ;
    dc:creator "OGC GeoSPARQL 1.0 Standard Working Group" ;
    dc:date "2011-06-16"^^xsd:date ;
    dc:description """
      Exists if the subject SpatialObject is spatially disjoint
      from the object SpatialObject. DE-9IM: FF*FF****
    """@en ;
    rdfs:comment """
      Exists if the subject SpatialObject is spatially disjoint
      from the object SpatialObject. DE-9IM: FF*FF****
    """@en ;
    rdfs:domain geo:SpatialObject ;
    rdfs:isDefinedBy
        <http://www.opengis.net/ont/geosparql> ,
        <http://www.opengis.net/spec/geosparql/1.0> ;
    rdfs:range geo:SpatialObject ;
    rdfs:seeAlso
        <http://www.opengis.net/ont/geosparql> ,
        <http://www.opengis.net/spec/geosparql/1.0> ;
    skos:definition """
      Exists if the subject SpatialObject is spatially disjoint
      from the object SpatialObject. DE-9IM: FF*FF****
    """@en ;
    skos:prefLabel "disjoint"@en ;
.

geo:ehEquals
    a
        rdf:Property ,
        rdfs:Resource ,
        owl:ObjectProperty ;
    rdfs:label "equals"@en ;
    dc:contributor "Matthew Perry" ;
    dc:creator "OGC GeoSPARQL 1.0 Standard Working Group" ;
    dc:date "2011-06-16"^^xsd:date ;
    dc:description """
      Exists if the subject SpatialObject spatially equals the 
      object SpatialObject. DE-9IM: TFFFTFFFT
    """@en ;
    rdfs:comment """
      Exists if the subject SpatialObject spatially equals the 
      object SpatialObject. DE-9IM: TFFFTFFFT
    """@en ;
    rdfs:domain geo:SpatialObject ;
    rdfs:isDefinedBy
        <http://www.opengis.net/ont/geosparql> ,
        <http://www.opengis.net/spec/geosparql/1.0> ;
    rdfs:range geo:SpatialObject ;
    rdfs:seeAlso
        <http://www.opengis.net/ont/geosparql> ,
        <http://www.opengis.net/spec/geosparql/1.0> ;
    skos:definition """
      Exists if the subject SpatialObject spatially equals the 
      object SpatialObject. DE-9IM: TFFFTFFFT
    """@en ;
    skos:prefLabel "equals"@en ;
.

geo:ehInside
    a
        rdf:Property ,
        rdfs:Resource ,
        owl:ObjectProperty ;
    rdfs:label "inside"@en ;
    dc:contributor "Matthew Perry" ;
    dc:creator "OGC GeoSPARQL 1.0 Standard Working Group" ;
    dc:date "2011-06-16"^^xsd:date ;
    dc:description """
      Exists if the subject SpatialObject is spatially inside 
      the object SpatialObject. DE-9IM: TFF*FFT**
    """@en ;
    rdfs:comment """
      Exists if the subject SpatialObject is spatially inside 
      the object SpatialObject. DE-9IM: TFF*FFT**
    """@en ;
    rdfs:domain geo:SpatialObject ;
    rdfs:isDefinedBy
        <http://www.opengis.net/ont/geosparql> ,
        <http://www.opengis.net/spec/geosparql/1.0> ;
    rdfs:range geo:SpatialObject ;
    rdfs:seeAlso
        <http://www.opengis.net/ont/geosparql> ,
        <http://www.opengis.net/spec/geosparql/1.0> ;
    skos:definition """
      Exists if the subject SpatialObject is spatially inside 
      the object SpatialObject. DE-9IM: TFF*FFT**
    """@en ;
    skos:prefLabel "inside"@en ;
.

geo:ehMeet
    a
        rdf:Property ,
        rdfs:Resource ,
        owl:ObjectProperty ;
    rdfs:label "meet"@en ;
    dc:contributor "Matthew Perry" ;
    dc:creator "OGC GeoSPARQL 1.0 Standard Working Group" ;
    dc:date "2011-06-16"^^xsd:date ;
    dc:description """
      Exists if the subject SpatialObject spatially meets the 
      object SpatialObject. 
      DE-9IM: FT******* ^ F**T***** ^ F***T****
    """@en ;
    rdfs:comment """
      Exists if the subject SpatialObject spatially meets the 
      object SpatialObject. 
      DE-9IM: FT******* ^ F**T***** ^ F***T****
    """@en ;
    rdfs:domain geo:SpatialObject ;
    rdfs:isDefinedBy
        <http://www.opengis.net/ont/geosparql> ,
        <http://www.opengis.net/spec/geosparql/1.0> ;
    rdfs:range geo:SpatialObject ;
    rdfs:seeAlso
        <http://www.opengis.net/ont/geosparql> ,
        <http://www.opengis.net/spec/geosparql/1.0> ;
    skos:definition """
      Exists if the subject SpatialObject spatially meets the 
      object SpatialObject. 
      DE-9IM: FT******* ^ F**T***** ^ F***T****
    """@en ;
    skos:prefLabel "meet"@en ;
.

geo:ehOverlap
    a
        rdf:Property ,
        rdfs:Resource ,
        owl:ObjectProperty ;
    rdfs:label "overlap"@en ;
    dc:contributor "Matthew Perry" ;
    dc:creator "OGC GeoSPARQL 1.0 Standard Working Group" ;
    dc:date "2011-06-16"^^xsd:date ;
    dc:description """
      Exists if the subject SpatialObject spatially overlaps the 
      object SpatialObject. DE-9IM: T*T***T**
    """@en ;
    rdfs:comment """
      Exists if the subject SpatialObject spatially overlaps the 
      object SpatialObject. DE-9IM: T*T***T**
    """@en ;
    rdfs:domain geo:SpatialObject ;
    rdfs:isDefinedBy
        <http://www.opengis.net/ont/geosparql> ,
        <http://www.opengis.net/spec/geosparql/1.0> ;
    rdfs:range geo:SpatialObject ;
    rdfs:seeAlso
        <http://www.opengis.net/ont/geosparql> ,
        <http://www.opengis.net/spec/geosparql/1.0> ;
    skos:definition """
      Exists if the subject SpatialObject spatially overlaps the 
      object SpatialObject. DE-9IM: T*T***T**
    """@en ;
    skos:prefLabel "overlap"@en ;
.

geo:isEmpty
    a
        rdf:Property ,
        rdfs:Resource ,
        owl:DatatypeProperty ;
    rdfs:label "isEmpty"@en ;
    dc:contributor "Matthew Perry" ;
    dc:creator "OGC GeoSPARQL 1.0 Standard Working Group" ;
    dc:date "2011-06-16"^^xsd:date ;
    dc:description """
      (true) if this geometric object is the empty Geometry. If 
      true, then this geometric object represents the empty point 
      set for the coordinate space.
    """@en ;
    rdfs:comment """
      (true) if this geometric object is the empty Geometry. If 
      true, then this geometric object represents the empty point 
      set for the coordinate space.
    """@en ;
    rdfs:domain geo:Geometry ;
    rdfs:isDefinedBy
        <http://www.opengis.net/ont/geosparql> ,
        <http://www.opengis.net/spec/geosparql/1.0> ;
    rdfs:range xsd:boolean ;
    rdfs:seeAlso
        <http://www.opengis.net/ont/geosparql> ,
        <http://www.opengis.net/spec/geosparql/1.0> ;
    skos:definition """
      (true) if this geometric object is the empty Geometry. If 
      true, then this geometric object represents the empty point 
      set for the coordinate space.
    """@en ;
    skos:prefLabel "isEmpty"@en ;
.

geo:isSimple
    a
        rdf:Property ,
        rdfs:Resource ,
        owl:DatatypeProperty ;
    rdfs:label "isSimple"@en ;
    dc:contributor "Matthew Perry" ;
    dc:creator "OGC GeoSPARQL 1.0 Standard Working Group" ;
    dc:date "2011-06-16"^^xsd:date ;
    dc:description """
      (true) if this geometric object has no anomalous geometric 
      points, such as self intersection or self tangency.
    """@en ;
    rdfs:comment """
      (true) if this geometric object has no anomalous geometric 
      points, such as self intersection or self tangency.
    """@en ;
    rdfs:domain geo:Geometry ;
    rdfs:isDefinedBy
        <http://www.opengis.net/ont/geosparql> ,
        <http://www.opengis.net/spec/geosparql/1.0> ;
    rdfs:range xsd:boolean ;
    rdfs:seeAlso
        <http://www.opengis.net/ont/geosparql> ,
        <http://www.opengis.net/spec/geosparql/1.0> ;
    skos:definition """
      (true) if this geometric object has no anomalous geometric 
      points, such as self intersection or self tangency.
    """@en ;
    skos:prefLabel "isSimple"@en ;
.

geo:rcc8dc
    a
        rdf:Property ,
        rdfs:Resource ,
        owl:ObjectProperty ;
    rdfs:label "disconnected"@en ;
    dc:contributor "Matthew Perry" ;
    dc:creator "OGC GeoSPARQL 1.0 Standard Working Group" ;
    dc:date "2011-06-16"^^xsd:date ;
    dc:description """
      Exists if the subject SpatialObject is spatially disjoint
      from the object SpatialObject. DE-9IM: FFTFFTTTT
    """@en ;
    rdfs:comment """
      Exists if the subject SpatialObject is spatially disjoint
      from the object SpatialObject. DE-9IM: FFTFFTTTT
    """@en ;
    rdfs:domain geo:SpatialObject ;
    rdfs:isDefinedBy
        <http://www.opengis.net/ont/geosparql> ,
        <http://www.opengis.net/spec/geosparql/1.0> ;
    rdfs:range geo:SpatialObject ;
    rdfs:seeAlso
        <http://www.opengis.net/ont/geosparql> ,
        <http://www.opengis.net/spec/geosparql/1.0> ;
    skos:definition """
      Exists if the subject SpatialObject is spatially disjoint
      from the object SpatialObject. DE-9IM: FFTFFTTTT
    """@en ;
    skos:prefLabel "disconnected"@en ;
.

geo:rcc8ec
    a
        rdf:Property ,
        rdfs:Resource ,
        owl:ObjectProperty ;
    rdfs:label "externally connected"@en ;
    dc:contributor "Matthew Perry" ;
    dc:creator "OGC GeoSPARQL 1.0 Standard Working Group" ;
    dc:date "2011-06-16"^^xsd:date ;
    dc:description """
      Exists if the subject SpatialObject spatially meets the 
      object SpatialObject. DE-9IM: FFTFTTTTT
    """@en ;
    rdfs:comment """
      Exists if the subject SpatialObject spatially meets the 
      object SpatialObject. DE-9IM: FFTFTTTTT
    """@en ;
    rdfs:domain geo:SpatialObject ;
    rdfs:isDefinedBy
        <http://www.opengis.net/ont/geosparql> ,
        <http://www.opengis.net/spec/geosparql/1.0> ;
    rdfs:range geo:SpatialObject ;
    rdfs:seeAlso
        <http://www.opengis.net/ont/geosparql> ,
        <http://www.opengis.net/spec/geosparql/1.0> ;
    skos:definition """
      Exists if the subject SpatialObject spatially meets the 
      object SpatialObject. DE-9IM: FFTFTTTTT
    """@en ;
    skos:prefLabel "externally connected"@en ;
.

geo:rcc8eq
    a
        rdf:Property ,
        rdfs:Resource ,
        owl:ObjectProperty ;
    rdfs:label "equals"@en ;
    dc:contributor "Matthew Perry" ;
    dc:creator "OGC GeoSPARQL 1.0 Standard Working Group" ;
    dc:date "2011-06-16"^^xsd:date ;
    dc:description """
      Exists if the subject SpatialObject spatially equals the 
      object SpatialObject. DE-9IM: TFFFTFFFT
    """@en ;
    rdfs:comment """
      Exists if the subject SpatialObject spatially equals the 
      object SpatialObject. DE-9IM: TFFFTFFFT
    """@en ;
    rdfs:domain geo:SpatialObject ;
    rdfs:isDefinedBy
        <http://www.opengis.net/ont/geosparql> ,
        <http://www.opengis.net/spec/geosparql/1.0> ;
    rdfs:range geo:SpatialObject ;
    rdfs:seeAlso
        <http://www.opengis.net/ont/geosparql> ,
        <http://www.opengis.net/spec/geosparql/1.0> ;
    skos:definition """
      Exists if the subject SpatialObject spatially equals the 
      object SpatialObject. DE-9IM: TFFFTFFFT
    """@en ;
    skos:prefLabel "equals"@en ;
.

geo:rcc8ntpp
    a
        rdf:Property ,
        rdfs:Resource ,
        owl:ObjectProperty ;
    rdfs:label "non-tangential proper part"@en ;
    dc:contributor "Matthew Perry" ;
    dc:creator "OGC GeoSPARQL 1.0 Standard Working Group" ;
    dc:date "2011-06-16"^^xsd:date ;
    dc:description """
      Exists if the subject SpatialObject is spatially inside 
      the object SpatialObject. DE-9IM: TFFTFFTTT
    """@en ;
    rdfs:comment """
      Exists if the subject SpatialObject is spatially inside 
      the object SpatialObject. DE-9IM: TFFTFFTTT
    """@en ;
    rdfs:domain geo:SpatialObject ;
    rdfs:isDefinedBy
        <http://www.opengis.net/ont/geosparql> ,
        <http://www.opengis.net/spec/geosparql/1.0> ;
    rdfs:range geo:SpatialObject ;
    rdfs:seeAlso
        <http://www.opengis.net/ont/geosparql> ,
        <http://www.opengis.net/spec/geosparql/1.0> ;
    skos:definition """
      Exists if the subject SpatialObject is spatially inside 
      the object SpatialObject. DE-9IM: TFFTFFTTT
    """@en ;
    skos:prefLabel "non-tangential proper part"@en ;
.

geo:rcc8ntppi
    a
        rdf:Property ,
        rdfs:Resource ,
        owl:ObjectProperty ;
    rdfs:label "non-tangential proper part inverse"@en ;
    dc:contributor "Matthew Perry" ;
    dc:creator "OGC GeoSPARQL 1.0 Standard Working Group" ;
    dc:date "2011-06-16"^^xsd:date ;
    dc:description """
      Exists if the subject SpatialObject spatially contains the 
      object SpatialObject. DE-9IM: TTTFFTFFT
    """@en ;
    rdfs:comment """
      Exists if the subject SpatialObject spatially contains the 
      object SpatialObject. DE-9IM: TTTFFTFFT
    """@en ;
    rdfs:domain geo:SpatialObject ;
    rdfs:isDefinedBy
        <http://www.opengis.net/ont/geosparql> ,
        <http://www.opengis.net/spec/geosparql/1.0> ;
    rdfs:range geo:SpatialObject ;
    rdfs:seeAlso
        <http://www.opengis.net/ont/geosparql> ,
        <http://www.opengis.net/spec/geosparql/1.0> ;
    skos:definition """
      Exists if the subject SpatialObject spatially contains the 
      object SpatialObject. DE-9IM: TTTFFTFFT
    """@en ;
    skos:prefLabel "non-tangential proper part inverse"@en ;
.

geo:rcc8po
    a
        rdf:Property ,
        rdfs:Resource ,
        owl:ObjectProperty ;
    rdfs:label "partially overlapping"@en ;
    dc:contributor "Matthew Perry" ;
    dc:creator "OGC GeoSPARQL 1.0 Standard Working Group" ;
    dc:date "2011-06-16"^^xsd:date ;
    dc:description """
      Exists if the subject SpatialObject spatially overlaps the 
      object SpatialObject. DE-9IM: TTTTTTTTT
    """@en ;
    rdfs:comment """
      Exists if the subject SpatialObject spatially overlaps the 
      object SpatialObject. DE-9IM: TTTTTTTTT
    """@en ;
    rdfs:domain geo:SpatialObject ;
    rdfs:isDefinedBy
        <http://www.opengis.net/ont/geosparql> ,
        <http://www.opengis.net/spec/geosparql/1.0> ;
    rdfs:range geo:SpatialObject ;
    rdfs:seeAlso
        <http://www.opengis.net/ont/geosparql> ,
        <http://www.opengis.net/spec/geosparql/1.0> ;
    skos:definition """
      Exists if the subject SpatialObject spatially overlaps the 
      object SpatialObject. DE-9IM: TTTTTTTTT
    """@en ;
    skos:prefLabel "partially overlapping"@en ;
.

geo:rcc8tpp
    a
        rdf:Property ,
        rdfs:Resource ,
        owl:ObjectProperty ;
    rdfs:label "tangential proper part"@en ;
    dc:contributor "Matthew Perry" ;
    dc:creator "OGC GeoSPARQL 1.0 Standard Working Group" ;
    dc:date "2011-06-16"^^xsd:date ;
    dc:description """
      Exists if the subject SpatialObject is spatially covered 
      by the object SpatialObject. DE-9IM: TFFTTFTTT
    """@en ;
    rdfs:comment """
      Exists if the subject SpatialObject is spatially covered 
      by the object SpatialObject. DE-9IM: TFFTTFTTT
    """@en ;
    rdfs:domain geo:SpatialObject ;
    rdfs:isDefinedBy
        <http://www.opengis.net/ont/geosparql> ,
        <http://www.opengis.net/spec/geosparql/1.0> ;
    rdfs:range geo:SpatialObject ;
    rdfs:seeAlso
        <http://www.opengis.net/ont/geosparql> ,
        <http://www.opengis.net/spec/geosparql/1.0> ;
    skos:definition """
      Exists if the subject SpatialObject is spatially covered 
      by the object SpatialObject. DE-9IM: TFFTTFTTT
    """@en ;
    skos:prefLabel "tangential proper part"@en ;
.

geo:rcc8tppi
    a
        rdf:Property ,
        rdfs:Resource ,
        owl:ObjectProperty ;
    rdfs:label "tangential proper part inverse"@en ;
    dc:contributor "Matthew Perry" ;
    dc:creator "OGC GeoSPARQL 1.0 Standard Working Group" ;
    dc:date "2011-06-16"^^xsd:date ;
    dc:description """
      Exists if the subject SpatialObject spatially covers the 
      object SpatialObject. DE-9IM: TTTFTTFFT
    """@en ;
    rdfs:comment """
      Exists if the subject SpatialObject spatially covers the 
      object SpatialObject. DE-9IM: TTTFTTFFT
    """@en ;
    rdfs:domain geo:SpatialObject ;
    rdfs:isDefinedBy
        <http://www.opengis.net/ont/geosparql> ,
        <http://www.opengis.net/spec/geosparql/1.0> ;
    rdfs:range geo:SpatialObject ;
    rdfs:seeAlso
        <http://www.opengis.net/ont/geosparql> ,
        <http://www.opengis.net/spec/geosparql/1.0> ;
    skos:definition """
      Exists if the subject SpatialObject spatially covers the 
      object SpatialObject. DE-9IM: TTTFTTFFT
    """@en ;
    skos:prefLabel "tangential proper part inverse"@en ;
.

geo:sfContains
    a
        rdf:Property ,
        rdfs:Resource ,
        owl:ObjectProperty ;
    rdfs:label "contains"@en ;
    dc:contributor "Matthew Perry" ;
    dc:creator "OGC GeoSPARQL 1.0 Standard Working Group" ;
    dc:date "2011-06-16"^^xsd:date ;
    dc:description """
      Exists if the subject SpatialObject spatially contains the 
      object SpatialObject. DE-9IM: T*****FF*
    """@en ;
    rdfs:comment """
      Exists if the subject SpatialObject spatially contains the 
      object SpatialObject. DE-9IM: T*****FF*
    """@en ;
    rdfs:domain geo:SpatialObject ;
    rdfs:isDefinedBy
        <http://www.opengis.net/ont/geosparql> ,
        <http://www.opengis.net/spec/geosparql/1.0> ;
    rdfs:range geo:SpatialObject ;
    rdfs:seeAlso
        <http://www.opengis.net/ont/geosparql> ,
        <http://www.opengis.net/spec/geosparql/1.0> ;
    skos:definition """
      Exists if the subject SpatialObject spatially contains the 
      object SpatialObject. DE-9IM: T*****FF*
    """@en ;
    skos:prefLabel "contains"@en ;
.

geo:sfCrosses
    a
        rdf:Property ,
        rdfs:Resource ,
        owl:ObjectProperty ;
    rdfs:label "crosses"@en ;
    dc:contributor "Matthew Perry" ;
    dc:creator "OGC GeoSPARQL 1.0 Standard Working Group" ;
    dc:date "2011-06-16"^^xsd:date ;
    dc:description """
      Exists if the subject SpatialObject spatially crosses the 
      object SpatialObject. DE-9IM: T*T******
    """@en ;
    rdfs:comment """
      Exists if the subject SpatialObject spatially crosses the 
      object SpatialObject. DE-9IM: T*T******
    """@en ;
    rdfs:domain geo:SpatialObject ;
    rdfs:isDefinedBy
        <http://www.opengis.net/ont/geosparql> ,
        <http://www.opengis.net/spec/geosparql/1.0> ;
    rdfs:range geo:SpatialObject ;
    rdfs:seeAlso
        <http://www.opengis.net/ont/geosparql> ,
        <http://www.opengis.net/spec/geosparql/1.0> ;
    skos:definition """
      Exists if the subject SpatialObject spatially crosses the 
      object SpatialObject. DE-9IM: T*T******
    """@en ;
    skos:prefLabel "crosses"@en ;
.

geo:sfDisjoint
    a
        rdf:Property ,
        rdfs:Resource ,
        owl:ObjectProperty ;
    rdfs:label "disjoint"@en ;
    dc:contributor "Matthew Perry" ;
    dc:creator "OGC GeoSPARQL 1.0 Standard Working Group" ;
    dc:date "2011-06-16"^^xsd:date ;
    dc:description """
      Exists if the subject SpatialObject is spatially disjoint 
      from the object SpatialObject. DE-9IM: FF*FF****
    """@en ;
    rdfs:comment """
      Exists if the subject SpatialObject is spatially disjoint 
      from the object SpatialObject. DE-9IM: FF*FF****
    """@en ;
    rdfs:domain geo:SpatialObject ;
    rdfs:isDefinedBy
        <http://www.opengis.net/ont/geosparql> ,
        <http://www.opengis.net/spec/geosparql/1.0> ;
    rdfs:range geo:SpatialObject ;
    rdfs:seeAlso
        <http://www.opengis.net/ont/geosparql> ,
        <http://www.opengis.net/spec/geosparql/1.0> ;
    skos:definition """
      Exists if the subject SpatialObject is spatially disjoint 
      from the object SpatialObject. DE-9IM: FF*FF****
    """@en ;
    skos:prefLabel "disjoint"@en ;
.

geo:sfEquals
    a
        rdf:Property ,
        rdfs:Resource ,
        owl:ObjectProperty ;
    rdfs:label "equals"@en ;
    dc:contributor "Matthew Perry" ;
    dc:creator "OGC GeoSPARQL 1.0 Standard Working Group" ;
    dc:date "2011-06-16"^^xsd:date ;
    dc:description """
      Exists if the subject SpatialObject spatially equals the 
      object SpatialObject. DE-9IM: TFFFTFFFT
    """@en ;
    rdfs:comment """
      Exists if the subject SpatialObject spatially equals the 
      object SpatialObject. DE-9IM: TFFFTFFFT
    """@en ;
    rdfs:domain geo:SpatialObject ;
    rdfs:isDefinedBy
        <http://www.opengis.net/ont/geosparql> ,
        <http://www.opengis.net/spec/geosparql/1.0> ;
    rdfs:range geo:SpatialObject ;
    rdfs:seeAlso
        <http://www.opengis.net/ont/geosparql> ,
        <http://www.opengis.net/spec/geosparql/1.0> ;
    skos:definition """
      Exists if the subject SpatialObject spatially equals the 
      object SpatialObject. DE-9IM: TFFFTFFFT
    """@en ;
    skos:prefLabel "equals"@en ;
.

geo:sfIntersects
    a
        rdf:Property ,
        rdfs:Resource ,
        owl:ObjectProperty ;
    rdfs:label "intersects"@en ;
    dc:contributor "Matthew Perry" ;
    dc:creator "OGC GeoSPARQL 1.0 Standard Working Group" ;
    dc:date "2011-06-16"^^xsd:date ;
    dc:description """
      Exists if the subject SpatialObject is not spatially disjoint 
      from the object SpatialObject.
      DE-9IM: T******** ^ *T******* ^ ***T***** ^ ****T**** 
    """@en ;
    rdfs:comment """
      Exists if the subject SpatialObject is not spatially disjoint 
      from the object SpatialObject.
      DE-9IM: T******** ^ *T******* ^ ***T***** ^ ****T**** 
    """@en ;
    rdfs:domain geo:SpatialObject ;
    rdfs:isDefinedBy
        <http://www.opengis.net/ont/geosparql> ,
        <http://www.opengis.net/spec/geosparql/1.0> ;
    rdfs:range geo:SpatialObject ;
    rdfs:seeAlso
        <http://www.opengis.net/ont/geosparql> ,
        <http://www.opengis.net/spec/geosparql/1.0> ;
    skos:definition """
      Exists if the subject SpatialObject is not spatially disjoint 
      from the object SpatialObject.
      DE-9IM: T******** ^ *T******* ^ ***T***** ^ ****T**** 
    """@en ;
    skos:prefLabel "intersects"@en ;
.

geo:sfOverlaps
    a
        rdf:Property ,
        rdfs:Resource ,
        owl:ObjectProperty ;
    rdfs:label "overlaps"@en ;
    dc:contributor "Matthew Perry" ;
    dc:creator "OGC GeoSPARQL 1.0 Standard Working Group" ;
    dc:date "2011-06-16"^^xsd:date ;
    dc:description """
      Exists if the subject SpatialObject spatially overlaps the 
      object SpatialObject. DE-9IM: T*T***T** 
    """@en ;
    rdfs:comment """
      Exists if the subject SpatialObject spatially overlaps the 
      object SpatialObject. DE-9IM: T*T***T** 
    """@en ;
    rdfs:domain geo:SpatialObject ;
    rdfs:isDefinedBy
        <http://www.opengis.net/ont/geosparql> ,
        <http://www.opengis.net/spec/geosparql/1.0> ;
    rdfs:range geo:SpatialObject ;
    rdfs:seeAlso
        <http://www.opengis.net/ont/geosparql> ,
        <http://www.opengis.net/spec/geosparql/1.0> ;
    skos:definition """
      Exists if the subject SpatialObject spatially overlaps the 
      object SpatialObject. DE-9IM: T*T***T** 
    """@en ;
    skos:prefLabel "overlaps"@en ;
.

geo:sfTouches
    a
        rdf:Property ,
        rdfs:Resource ,
        owl:ObjectProperty ;
    rdfs:label "touches"@en ;
    dc:contributor "Matthew Perry" ;
    dc:creator "OGC GeoSPARQL 1.0 Standard Working Group" ;
    dc:date "2011-06-16"^^xsd:date ;
    dc:description """
      Exists if the subject SpatialObject spatially touches the 
      object SpatialObject.
      DE-9IM: FT******* ^ F**T***** ^ F***T****
    """@en ;
    rdfs:comment """
      Exists if the subject SpatialObject spatially touches the 
      object SpatialObject.
      DE-9IM: FT******* ^ F**T***** ^ F***T****
    """@en ;
    rdfs:domain geo:SpatialObject ;
    rdfs:isDefinedBy
        <http://www.opengis.net/ont/geosparql> ,
        <http://www.opengis.net/spec/geosparql/1.0> ;
    rdfs:range geo:SpatialObject ;
    rdfs:seeAlso
        <http://www.opengis.net/ont/geosparql> ,
        <http://www.opengis.net/spec/geosparql/1.0> ;
    skos:definition """
      Exists if the subject SpatialObject spatially touches the 
      object SpatialObject.
      DE-9IM: FT******* ^ F**T***** ^ F***T****
    """@en ;
    skos:prefLabel "touches"@en ;
.

geo:sfWithin
    a
        rdf:Property ,
        rdfs:Resource ,
        owl:ObjectProperty ;
    rdfs:label "within"@en ;
    dc:contributor "Matthew Perry" ;
    dc:creator "OGC GeoSPARQL 1.0 Standard Working Group" ;
    dc:date "2011-06-16"^^xsd:date ;
    dc:description """
      Exists if the subject SpatialObject is spatially within the 
      object SpatialObject. DE-9IM: T*F**F***
    """@en ;
    rdfs:comment """
      Exists if the subject SpatialObject is spatially within the 
      object SpatialObject. DE-9IM: T*F**F***
    """@en ;
    rdfs:domain geo:SpatialObject ;
    rdfs:isDefinedBy
        <http://www.opengis.net/ont/geosparql> ,
        <http://www.opengis.net/spec/geosparql/1.0> ;
    rdfs:range geo:SpatialObject ;
    rdfs:seeAlso
        <http://www.opengis.net/ont/geosparql> ,
        <http://www.opengis.net/spec/geosparql/1.0> ;
    skos:definition """
      Exists if the subject SpatialObject is spatially within the 
      object SpatialObject. DE-9IM: T*F**F***
    """@en ;
    skos:prefLabel "within"@en ;
.

geo:spatialDimension
    a
        rdf:Property ,
        rdfs:Resource ,
        owl:DatatypeProperty ;
    rdfs:label "spatialDimension"@en ;
    dc:contributor "Matthew Perry" ;
    dc:creator "OGC GeoSPARQL 1.0 Standard Working Group" ;
    dc:date "2011-06-16"^^xsd:date ;
    dc:description """
      The number of measurements or axes needed to describe the spatial position of 
      this geometry in a coordinate system.
    """@en ;
    rdfs:comment """
      The number of measurements or axes needed to describe the spatial position of 
      this geometry in a coordinate system.
    """@en ;
    rdfs:domain geo:Geometry ;
    rdfs:isDefinedBy
        <http://www.opengis.net/ont/geosparql> ,
        <http://www.opengis.net/spec/geosparql/1.0> ;
    rdfs:range xsd:integer ;
    rdfs:seeAlso
        <http://www.opengis.net/ont/geosparql> ,
        <http://www.opengis.net/spec/geosparql/1.0> ;
    skos:definition """
      The number of measurements or axes needed to describe the spatial position of 
      this geometry in a coordinate system.
    """@en ;
    skos:prefLabel "spatialDimension"@en ;
.

()
    a
        rdf:List ,
        rdfs:Resource ;
.

rdf:type
    a
        rdf:Property ,
        rdfs:Resource ;
    rdfs:range rdfs:Class ;
.

rdfs:comment
    a
        rdf:Property ,
        rdfs:Resource ;
    rdfs:range rdfs:Literal ;
.

rdfs:domain
    a
        rdf:Property ,
        rdfs:Resource ;
    rdfs:domain rdf:Property ;
    rdfs:range rdfs:Class ;
.

rdfs:label
    a
        rdf:Property ,
        rdfs:Resource ;
    rdfs:range rdfs:Literal ;
.

rdfs:range
    a
        rdf:Property ,
        rdfs:Resource ;
    rdfs:domain rdf:Property ;
    rdfs:range rdfs:Class ;
.

rdfs:subClassOf
    a
        rdf:Property ,
        rdfs:Resource ;
    rdfs:domain rdfs:Class ;
    rdfs:range rdfs:Class ;
.

rdfs:subPropertyOf
    a
        rdf:Property ,
        rdfs:Resource ;
    rdfs:domain rdf:Property ;
    rdfs:range rdf:Property ;
.

<http://anzsoil.org/def/au/asls/substrate/genesis-hardened>
    a skos:Collection ;
    rdfs:isDefinedBy <http://anzsoil.org/def/au/asls/substrate> ;
    rdfs:seeAlso <http://anzsoil.org/def/au/asls/substrate> ;
    skos:definition "Masses hardened in the regolith"@en ;
    skos:inScheme <http://anzsoil.org/def/au/asls/substrate> ;
    skos:member
        <http://anzsoil.org/def/au/asls/substrate/Rock-genesis-hardened-artificial> ,
        <http://anzsoil.org/def/au/asls/substrate/Rock-genesis-hardened-chemical> ,
        <http://anzsoil.org/def/au/asls/substrate/Rock-genesis-hardened-evaporite> ;
    skos:notation "4" ;
    skos:prefLabel "Masses hardened in the regolith"@en ;
.

<http://anzsoil.org/def/au/asls/substrate/lithology>
    a skos:Collection ;
    rdfs:isDefinedBy <http://anzsoil.org/def/au/asls/substrate> ;
    rdfs:seeAlso <http://anzsoil.org/def/au/asls/substrate> ;
    skos:definition "Lithological type of rock material and unconsolidated material."@en ;
    skos:inScheme <http://anzsoil.org/def/au/asls/substrate> ;
    skos:member
        <http://anzsoil.org/def/au/asls/substrate/Lithology-rock> ,
        <http://anzsoil.org/def/au/asls/substrate/Lithology-unconsolidated> ;
    skos:note
        "C_LITHOLOGY" ,
        """The properties above will key out many of the rock types and unconsolidated materials listed in Tables 33 and 34.

Record the rock type only if it is definitely known or is confidently presumed. An alphabetic checklist for types of substrate material, both rocks and unconsolidated materials, is given in Table 35. Only the more common materials are listed. Others can be recorded in free format.""" ;
    skos:prefLabel "Lithology"@en ;
.

geo:asGML
    a
        rdf:Property ,
        rdfs:Resource ,
        owl:DatatypeProperty ;
    rdfs:label "asGML"@en ;
    dc:contributor "Matthew Perry" ;
    dc:creator "OGC GeoSPARQL 1.0 Standard Working Group" ;
    dc:date "2011-06-16"^^xsd:date ;
    dc:description """
      The GML serialization of a geometry
    """@en ;
    rdfs:comment """
      The GML serialization of a geometry
    """@en ;
    rdfs:domain geo:Geometry ;
    rdfs:isDefinedBy
        <http://www.opengis.net/ont/geosparql> ,
        <http://www.opengis.net/spec/geosparql/1.0> ;
    rdfs:range geo:gmlLiteral ;
    rdfs:seeAlso
        <http://www.opengis.net/ont/geosparql> ,
        <http://www.opengis.net/spec/geosparql/1.0> ;
    rdfs:subPropertyOf
        geo:asGML ,
        geo:hasSerialization ;
    skos:definition """
      The GML serialization of a geometry
    """@en ;
    skos:prefLabel "asGML"@en ;
.

geo:asWKT
    a
        rdf:Property ,
        rdfs:Resource ,
        owl:DatatypeProperty ;
    rdfs:label "asWKT"@en ;
    dc:contributor "Matthew Perry" ;
    dc:creator "OGC GeoSPARQL 1.0 Standard Working Group" ;
    dc:date "2011-06-16"^^xsd:date ;
    dc:description """
      The WKT serialization of a geometry
    """@en ;
    rdfs:comment """
      The WKT serialization of a geometry
    """@en ;
    rdfs:domain geo:Geometry ;
    rdfs:isDefinedBy
        <http://www.opengis.net/ont/geosparql> ,
        <http://www.opengis.net/spec/geosparql/1.0> ;
    rdfs:range geo:wktLiteral ;
    rdfs:seeAlso
        <http://www.opengis.net/ont/geosparql> ,
        <http://www.opengis.net/spec/geosparql/1.0> ;
    rdfs:subPropertyOf
        geo:asWKT ,
        geo:hasSerialization ;
    skos:definition """
      The WKT serialization of a geometry
    """@en ;
    skos:prefLabel "asWKT"@en ;
.

geo:hasDefaultGeometry
    a
        rdf:Property ,
        rdfs:Resource ,
        owl:ObjectProperty ;
    rdfs:label "hasDefaultGeometry"@en ;
    dc:contributor "Matthew Perry" ;
    dc:creator "OGC GeoSPARQL 1.0 Standard Working Group" ;
    dc:date "2011-06-16"^^xsd:date ;
    dc:description """
      The default geometry to be used in spatial calculations.
      It is Usually the most detailed geometry.
    """@en ;
    rdfs:comment """
      The default geometry to be used in spatial calculations.
      It is Usually the most detailed geometry.
    """@en ;
    rdfs:domain geo:Feature ;
    rdfs:isDefinedBy
        <http://www.opengis.net/ont/geosparql> ,
        <http://www.opengis.net/spec/geosparql/1.0> ;
    rdfs:range geo:Geometry ;
    rdfs:seeAlso
        <http://www.opengis.net/ont/geosparql> ,
        <http://www.opengis.net/spec/geosparql/1.0> ;
    rdfs:subPropertyOf
        geo:hasDefaultGeometry ,
        geo:hasGeometry ;
    skos:definition """
      The default geometry to be used in spatial calculations.
      It is Usually the most detailed geometry.
    """@en ;
    skos:prefLabel "hasDefaultGeometry"@en ;
.

rdf:first
    a
        rdf:Property ,
        rdfs:Resource ;
    rdfs:domain rdf:List ;
    rdfs:subPropertyOf rdf:first ;
.

rdf:object
    a
        rdf:Property ,
        rdfs:Resource ;
    rdfs:domain rdf:Statement ;
    rdfs:subPropertyOf rdf:object ;
.

rdf:predicate
    a
        rdf:Property ,
        rdfs:Resource ;
    rdfs:domain rdf:Statement ;
    rdfs:subPropertyOf rdf:predicate ;
.

rdf:rest
    a
        rdf:Property ,
        rdfs:Resource ;
    rdfs:domain rdf:List ;
    rdfs:range rdf:List ;
    rdfs:subPropertyOf rdf:rest ;
.

rdf:subject
    a
        rdf:Property ,
        rdfs:Resource ;
    rdfs:domain rdf:Statement ;
    rdfs:subPropertyOf rdf:subject ;
.

rdfs:isDefinedBy
    a
        rdf:Property ,
        rdfs:Resource ;
    rdfs:subPropertyOf
        rdfs:isDefinedBy ,
        rdfs:seeAlso ;
.

<http://anzsoil.org/def/au/asls/substrate/alteration-F>
    a
        <http://anzsoil.org/def/au/asls/substrate/Rock-alteration> ,
        skos:Concept ;
    rdfs:isDefinedBy <http://anzsoil.org/def/au/asls/substrate> ;
    rdfs:seeAlso <http://anzsoil.org/def/au/asls/substrate> ;
    skos:definition "iron enriched." ;
    skos:inScheme <http://anzsoil.org/def/au/asls/substrate> ;
    skos:notation "F" ;
    skos:prefLabel "Ferruginised"@en ;
    skos:topConceptOf <http://anzsoil.org/def/au/asls/substrate> ;
.

<http://anzsoil.org/def/au/asls/substrate/alteration-K>
    a
        <http://anzsoil.org/def/au/asls/substrate/Rock-alteration> ,
        skos:Concept ;
    rdfs:isDefinedBy <http://anzsoil.org/def/au/asls/substrate> ;
    rdfs:seeAlso <http://anzsoil.org/def/au/asls/substrate> ;
    skos:definition "calcium carbonate enriched." ;
    skos:inScheme <http://anzsoil.org/def/au/asls/substrate> ;
    skos:notation "K" ;
    skos:prefLabel "Calcified"@en ;
    skos:topConceptOf <http://anzsoil.org/def/au/asls/substrate> ;
.

<http://anzsoil.org/def/au/asls/substrate/alteration-L>
    a
        <http://anzsoil.org/def/au/asls/substrate/Rock-alteration> ,
        skos:Concept ;
    rdfs:isDefinedBy <http://anzsoil.org/def/au/asls/substrate> ;
    rdfs:seeAlso <http://anzsoil.org/def/au/asls/substrate> ;
    skos:definition "clay enriched, usually pale coloured, for example the pallid zone of a laterite profile." ;
    skos:inScheme <http://anzsoil.org/def/au/asls/substrate> ;
    skos:notation "L" ;
    skos:prefLabel "Kaolinised"@en ;
    skos:topConceptOf <http://anzsoil.org/def/au/asls/substrate> ;
.

<http://anzsoil.org/def/au/asls/substrate/alteration-O>
    a
        <http://anzsoil.org/def/au/asls/substrate/Rock-alteration> ,
        skos:Concept ;
    rdfs:isDefinedBy <http://anzsoil.org/def/au/asls/substrate> ;
    rdfs:seeAlso <http://anzsoil.org/def/au/asls/substrate> ;
    skos:definition "deeply weathered but no specific nature." ;
    skos:inScheme <http://anzsoil.org/def/au/asls/substrate> ;
    skos:notation "O" ;
    skos:prefLabel "Other"@en ;
    skos:topConceptOf <http://anzsoil.org/def/au/asls/substrate> ;
.

<http://anzsoil.org/def/au/asls/substrate/alteration-S>
    a
        <http://anzsoil.org/def/au/asls/substrate/Rock-alteration> ,
        skos:Concept ;
    rdfs:isDefinedBy <http://anzsoil.org/def/au/asls/substrate> ;
    rdfs:seeAlso <http://anzsoil.org/def/au/asls/substrate> ;
    skos:definition "silica enriched." ;
    skos:inScheme <http://anzsoil.org/def/au/asls/substrate> ;
    skos:notation "S" ;
    skos:prefLabel "Silicified"@en ;
    skos:topConceptOf <http://anzsoil.org/def/au/asls/substrate> ;
.

<http://anzsoil.org/def/au/asls/substrate/confidence-certain>
    a
        <http://anzsoil.org/def/au/asls/substrate/Confidence> ,
        skos:Concept ;
    rdfs:isDefinedBy <http://anzsoil.org/def/au/asls/substrate> ;
    rdfs:seeAlso <http://anzsoil.org/def/au/asls/substrate> ;
    skos:definition "Almost certain or certain" ;
    skos:inScheme <http://anzsoil.org/def/au/asls/substrate> ;
    skos:notation "A" ;
    skos:prefLabel "Almost certain or certain"@en ;
    skos:topConceptOf <http://anzsoil.org/def/au/asls/substrate> ;
.

<http://anzsoil.org/def/au/asls/substrate/confidence-doubtful>
    a
        <http://anzsoil.org/def/au/asls/substrate/Confidence> ,
        skos:Concept ;
    rdfs:isDefinedBy <http://anzsoil.org/def/au/asls/substrate> ;
    rdfs:seeAlso <http://anzsoil.org/def/au/asls/substrate> ;
    skos:definition "Dubious, doubtful" ;
    skos:inScheme <http://anzsoil.org/def/au/asls/substrate> ;
    skos:notation "D" ;
    skos:prefLabel "Dubious, doubtful"@en ;
    skos:topConceptOf <http://anzsoil.org/def/au/asls/substrate> ;
.

<http://anzsoil.org/def/au/asls/substrate/confidence-not-parent>
    a
        <http://anzsoil.org/def/au/asls/substrate/Confidence> ,
        skos:Concept ;
    rdfs:isDefinedBy <http://anzsoil.org/def/au/asls/substrate> ;
    rdfs:seeAlso <http://anzsoil.org/def/au/asls/substrate> ;
    skos:definition "Not parent material" ;
    skos:inScheme <http://anzsoil.org/def/au/asls/substrate> ;
    skos:notation "N" ;
    skos:prefLabel "Not parent material"@en ;
    skos:topConceptOf <http://anzsoil.org/def/au/asls/substrate> ;
.

<http://anzsoil.org/def/au/asls/substrate/confidence-probable>
    a
        <http://anzsoil.org/def/au/asls/substrate/Confidence> ,
        skos:Concept ;
    rdfs:isDefinedBy <http://anzsoil.org/def/au/asls/substrate> ;
    rdfs:seeAlso <http://anzsoil.org/def/au/asls/substrate> ;
    skos:definition "Probable" ;
    skos:inScheme <http://anzsoil.org/def/au/asls/substrate> ;
    skos:notation "P" ;
    skos:prefLabel "Probable"@en ;
    skos:topConceptOf <http://anzsoil.org/def/au/asls/substrate> ;
.

<http://anzsoil.org/def/au/asls/substrate/discontinuity-spacing-B>
    a
        <http://anzsoil.org/def/au/asls/substrate/Substrate-discontinuity-spacing> ,
        skos:Concept ;
    rdfs:isDefinedBy <http://anzsoil.org/def/au/asls/substrate> ;
    rdfs:seeAlso <http://anzsoil.org/def/au/asls/substrate> ;
    skos:definition "300 mm – 1 m" ;
    skos:inScheme <http://anzsoil.org/def/au/asls/substrate> ;
    skos:notation "B" ;
    skos:prefLabel "blocky; moderately jointed."@en ;
    skos:topConceptOf <http://anzsoil.org/def/au/asls/substrate> ;
.

<http://anzsoil.org/def/au/asls/substrate/discontinuity-spacing-C>
    a
        <http://anzsoil.org/def/au/asls/substrate/Substrate-discontinuity-spacing> ,
        skos:Concept ;
    rdfs:isDefinedBy <http://anzsoil.org/def/au/asls/substrate> ;
    rdfs:seeAlso <http://anzsoil.org/def/au/asls/substrate> ;
    skos:definition "<50 mm" ;
    skos:inScheme <http://anzsoil.org/def/au/asls/substrate> ;
    skos:notation "C" ;
    skos:prefLabel "crushed or shattered."@en ;
    skos:topConceptOf <http://anzsoil.org/def/au/asls/substrate> ;
.

<http://anzsoil.org/def/au/asls/substrate/discontinuity-spacing-F>
    a
        <http://anzsoil.org/def/au/asls/substrate/Substrate-discontinuity-spacing> ,
        skos:Concept ;
    rdfs:isDefinedBy <http://anzsoil.org/def/au/asls/substrate> ;
    rdfs:seeAlso <http://anzsoil.org/def/au/asls/substrate> ;
    skos:definition "50-300 mm" ;
    skos:inScheme <http://anzsoil.org/def/au/asls/substrate> ;
    skos:notation "F" ;
    skos:prefLabel "fractured; intensely jointed."@en ;
    skos:topConceptOf <http://anzsoil.org/def/au/asls/substrate> ;
.

<http://anzsoil.org/def/au/asls/substrate/discontinuity-spacing-M>
    a
        <http://anzsoil.org/def/au/asls/substrate/Substrate-discontinuity-spacing> ,
        skos:Concept ;
    rdfs:isDefinedBy <http://anzsoil.org/def/au/asls/substrate> ;
    rdfs:seeAlso <http://anzsoil.org/def/au/asls/substrate> ;
    skos:definition "1-3 m" ;
    skos:inScheme <http://anzsoil.org/def/au/asls/substrate> ;
    skos:notation "M" ;
    skos:prefLabel "massive; few joints."@en ;
    skos:topConceptOf <http://anzsoil.org/def/au/asls/substrate> ;
.

<http://anzsoil.org/def/au/asls/substrate/discontinuity-spacing-S>
    a
        <http://anzsoil.org/def/au/asls/substrate/Substrate-discontinuity-spacing> ,
        skos:Concept ;
    rdfs:isDefinedBy <http://anzsoil.org/def/au/asls/substrate> ;
    rdfs:seeAlso <http://anzsoil.org/def/au/asls/substrate> ;
    skos:definition ">3 m" ;
    skos:inScheme <http://anzsoil.org/def/au/asls/substrate> ;
    skos:notation "S" ;
    skos:prefLabel "solid; virtually unjointed"@en ;
    skos:topConceptOf <http://anzsoil.org/def/au/asls/substrate> ;
.

<http://anzsoil.org/def/au/asls/substrate/genesis-AC>
    a
        <http://anzsoil.org/def/au/asls/substrate/Mass-genetic-type> ,
        <http://anzsoil.org/def/au/asls/substrate/Rock-genesis-hardened-chemical> ,
        skos:Concept ;
    rdfs:isDefinedBy <http://anzsoil.org/def/au/asls/substrate> ;
    rdfs:seeAlso <http://anzsoil.org/def/au/asls/substrate> ;
    skos:definition "indurated material rich in aluminium hydroxides. Commonly consists of cemented pisoliths and usually known as bauxite." ;
    skos:inScheme <http://anzsoil.org/def/au/asls/substrate> ;
    skos:notation "AC" ;
    skos:prefLabel "Alcrete (bauxite)"@en ;
    skos:topConceptOf <http://anzsoil.org/def/au/asls/substrate> ;
.

<http://anzsoil.org/def/au/asls/substrate/genesis-AL>
    a
        <http://anzsoil.org/def/au/asls/substrate/Mass-genetic-type> ,
        <http://anzsoil.org/def/au/asls/substrate/Rock-genesis-sediments> ,
        skos:Concept ;
    rdfs:isDefinedBy <http://anzsoil.org/def/au/asls/substrate> ;
    rdfs:seeAlso <http://anzsoil.org/def/au/asls/substrate> ;
    skos:definition "sediment mass deposited from transport by channelled stream flow or over-bank stream flow." ;
    skos:inScheme <http://anzsoil.org/def/au/asls/substrate> ;
    skos:notation "AL" ;
    skos:prefLabel "Alluvium"@en ;
    skos:topConceptOf <http://anzsoil.org/def/au/asls/substrate> ;
.

<http://anzsoil.org/def/au/asls/substrate/genesis-AT>
    a
        <http://anzsoil.org/def/au/asls/substrate/Rock-genesis-hardened-artificial> ,
        skos:Concept ;
    rdfs:isDefinedBy <http://anzsoil.org/def/au/asls/substrate> ;
    rdfs:seeAlso <http://anzsoil.org/def/au/asls/substrate> ;
    skos:definition "Other artificially hardened materials" ;
    skos:inScheme <http://anzsoil.org/def/au/asls/substrate> ;
    skos:notation "AT" ;
    skos:prefLabel "Other artificially hardened materials"@en ;
    skos:topConceptOf <http://anzsoil.org/def/au/asls/substrate> ;
.

<http://anzsoil.org/def/au/asls/substrate/genesis-BE>
    a
        <http://anzsoil.org/def/au/asls/substrate/Mass-genetic-type> ,
        <http://anzsoil.org/def/au/asls/substrate/Rock-genesis-sediments> ,
        skos:Concept ;
    rdfs:isDefinedBy <http://anzsoil.org/def/au/asls/substrate> ;
    rdfs:seeAlso <http://anzsoil.org/def/au/asls/substrate> ;
    skos:definition "sediment mass deposited from transport by waves or tides at the shore of a sea or lake." ;
    skos:inScheme <http://anzsoil.org/def/au/asls/substrate> ;
    skos:notation "BE" ;
    skos:prefLabel "Beach sediment"@en ;
    skos:topConceptOf <http://anzsoil.org/def/au/asls/substrate> ;
.

<http://anzsoil.org/def/au/asls/substrate/genesis-CD>
    a
        <http://anzsoil.org/def/au/asls/substrate/Mass-genetic-type> ,
        <http://anzsoil.org/def/au/asls/substrate/Rock-genesis-sediments> ,
        skos:Concept ;
    rdfs:isDefinedBy <http://anzsoil.org/def/au/asls/substrate> ;
    rdfs:seeAlso <http://anzsoil.org/def/au/asls/substrate> ;
    skos:definition "colluvium slowly displaced a short distance downslope as a result of small irregular movements, with the net movement increasing towards the land surface." ;
    skos:inScheme <http://anzsoil.org/def/au/asls/substrate> ;
    skos:notation "CD" ;
    skos:prefLabel "Creep deposit"@en ;
    skos:topConceptOf <http://anzsoil.org/def/au/asls/substrate> ;
.

<http://anzsoil.org/def/au/asls/substrate/genesis-CN>
    a
        <http://anzsoil.org/def/au/asls/substrate/Mass-genetic-type> ,
        <http://anzsoil.org/def/au/asls/substrate/Rock-genesis-hardened-artificial> ,
        skos:Concept ;
    rdfs:isDefinedBy <http://anzsoil.org/def/au/asls/substrate> ;
    rdfs:seeAlso <http://anzsoil.org/def/au/asls/substrate> ;
    skos:definition "artificial conglomerate rock mass of selected size grade material that has been hardened using Portland cement or other kinds of cement. Concrete is a weak rock (ca. 35 MPa unconfined compressive strength) usually reinforced with steel to increase its tensile strength." ;
    skos:inScheme <http://anzsoil.org/def/au/asls/substrate> ;
    skos:notation "CN" ;
    skos:prefLabel "Concrete"@en ;
    skos:topConceptOf <http://anzsoil.org/def/au/asls/substrate> ;
.

<http://anzsoil.org/def/au/asls/substrate/genesis-CO>
    a
        <http://anzsoil.org/def/au/asls/substrate/Mass-genetic-type> ,
        <http://anzsoil.org/def/au/asls/substrate/Rock-genesis-sediments> ,
        skos:Concept ;
    rdfs:isDefinedBy <http://anzsoil.org/def/au/asls/substrate> ;
    rdfs:seeAlso <http://anzsoil.org/def/au/asls/substrate> ;
    skos:definition "sediment mass deposited from transport down a slope by gravity (scree), landslide (landslide deposit), mudflow (mudflow deposit), creep (creep deposit) or sheet flow (sheet flow deposit), but not by stream flow. Compared with alluvium, colluvium lacks bedding structure; is more variable in grain size (that is, more poorly sorted); contains much local material; and is generally much more angular. Coarse particles may have particular alignments." ;
    skos:inScheme <http://anzsoil.org/def/au/asls/substrate> ;
    skos:notation "CO" ;
    skos:prefLabel "Colluvium"@en ;
    skos:topConceptOf <http://anzsoil.org/def/au/asls/substrate> ;
.

<http://anzsoil.org/def/au/asls/substrate/genesis-DR>
    a
        <http://anzsoil.org/def/au/asls/substrate/Mass-genetic-type> ,
        <http://anzsoil.org/def/au/asls/substrate/Rock-genesis-weathered> ,
        skos:Concept ;
    rdfs:isDefinedBy <http://anzsoil.org/def/au/asls/substrate> ;
    rdfs:seeAlso <http://anzsoil.org/def/au/asls/substrate> ;
    skos:definition "weathered material (typically soft and clay-rich) produced by thorough decomposition of rock masses due to exposure to land surface processes, but with no transport. It generally lacks any structures that may have been present in the unweathered rock (see also saprolite and partially weathered rock)." ;
    skos:inScheme <http://anzsoil.org/def/au/asls/substrate> ;
    skos:notation "DR" ;
    skos:prefLabel "Decomposed rock"@en ;
    skos:topConceptOf <http://anzsoil.org/def/au/asls/substrate> ;
.

<http://anzsoil.org/def/au/asls/substrate/genesis-ED>
    a
        <http://anzsoil.org/def/au/asls/substrate/Mass-genetic-type> ,
        <http://anzsoil.org/def/au/asls/substrate/Rock-genesis-sediments> ,
        skos:Concept ;
    rdfs:isDefinedBy <http://anzsoil.org/def/au/asls/substrate> ;
    rdfs:seeAlso <http://anzsoil.org/def/au/asls/substrate> ;
    skos:definition "sediment mass deposited from transport by the wind." ;
    skos:inScheme <http://anzsoil.org/def/au/asls/substrate> ;
    skos:notation "ED" ;
    skos:prefLabel "Eolian sediment"@en ;
    skos:topConceptOf <http://anzsoil.org/def/au/asls/substrate> ;
.

<http://anzsoil.org/def/au/asls/substrate/genesis-ES>
    a
        <http://anzsoil.org/def/au/asls/substrate/Mass-genetic-type> ,
        <http://anzsoil.org/def/au/asls/substrate/Rock-genesis-sediments> ,
        skos:Concept ;
    rdfs:isDefinedBy <http://anzsoil.org/def/au/asls/substrate> ;
    rdfs:seeAlso <http://anzsoil.org/def/au/asls/substrate> ;
    skos:definition "eolian sediment of sand size, often taking the form of dunes, with characteristic bedding structures." ;
    skos:inScheme <http://anzsoil.org/def/au/asls/substrate> ;
    skos:notation "ES" ;
    skos:prefLabel "Eolian sand"@en ;
    skos:topConceptOf <http://anzsoil.org/def/au/asls/substrate> ;
.

<http://anzsoil.org/def/au/asls/substrate/genesis-ET>
    a
        <http://anzsoil.org/def/au/asls/substrate/Mass-genetic-type> ,
        <http://anzsoil.org/def/au/asls/substrate/Rock-genesis-unweathered> ,
        skos:Concept ;
    rdfs:isDefinedBy <http://anzsoil.org/def/au/asls/substrate> ;
    rdfs:seeAlso <http://anzsoil.org/def/au/asls/substrate> ;
    skos:definition "consolidated sedimentary rock consisting of clastic material deposited by the wind.* Includes bioclastic calcarenites." ;
    skos:inScheme <http://anzsoil.org/def/au/asls/substrate> ;
    skos:notation "ET" ;
    skos:prefLabel "Eolianite"@en ;
    skos:topConceptOf <http://anzsoil.org/def/au/asls/substrate> ;
.

<http://anzsoil.org/def/au/asls/substrate/genesis-EV>
    a
        <http://anzsoil.org/def/au/asls/substrate/Mass-genetic-type> ,
        <http://anzsoil.org/def/au/asls/substrate/Rock-genesis-hardened-evaporite> ,
        skos:Concept ;
    rdfs:isDefinedBy <http://anzsoil.org/def/au/asls/substrate> ;
    rdfs:seeAlso <http://anzsoil.org/def/au/asls/substrate> ;
    skos:definition "weak sedimentary rock or sediment formed by the precipitation of solutes from water bodies on the land surface, typically as lacustrine sediments. Includes halite and gypsum." ;
    skos:inScheme <http://anzsoil.org/def/au/asls/substrate> ;
    skos:notation "EV" ;
    skos:prefLabel "Evaporite"@en ;
    skos:topConceptOf <http://anzsoil.org/def/au/asls/substrate> ;
.

<http://anzsoil.org/def/au/asls/substrate/genesis-FC>
    a
        <http://anzsoil.org/def/au/asls/substrate/Mass-genetic-type> ,
        <http://anzsoil.org/def/au/asls/substrate/Rock-genesis-hardened-chemical> ,
        skos:Concept ;
    rdfs:isDefinedBy <http://anzsoil.org/def/au/asls/substrate> ;
    rdfs:seeAlso <http://anzsoil.org/def/au/asls/substrate> ;
    skos:definition "indurated material rich in hydrated oxides of iron (usually goethite and hematite) occurring as cemented nodules and/or concretions, or as massive sheets. This material has been commonly referred to in local usage around Australia as laterite, duricrust or ironstone." ;
    skos:inScheme <http://anzsoil.org/def/au/asls/substrate> ;
    skos:notation "FC" ;
    skos:prefLabel "Ferricrete"@en ;
    skos:topConceptOf <http://anzsoil.org/def/au/asls/substrate> ;
.

<http://anzsoil.org/def/au/asls/substrate/genesis-FI>
    a
        <http://anzsoil.org/def/au/asls/substrate/Mass-genetic-type> ,
        <http://anzsoil.org/def/au/asls/substrate/Rock-genesis-sediments> ,
        skos:Concept ;
    rdfs:isDefinedBy <http://anzsoil.org/def/au/asls/substrate> ;
    rdfs:seeAlso <http://anzsoil.org/def/au/asls/substrate> ;
    skos:definition "mass of artificial sediment formed by earth-moving works. Fill is sometimes compacted to the status of a very weak rock mass (stabilised soil), but typically remains an earth mass (Table 36). Garbage forms a very low-density, low-strength fill." ;
    skos:inScheme <http://anzsoil.org/def/au/asls/substrate> ;
    skos:notation "FI" ;
    skos:prefLabel "Fill"@en ;
    skos:topConceptOf <http://anzsoil.org/def/au/asls/substrate> ;
.

<http://anzsoil.org/def/au/asls/substrate/genesis-HA>
    a
        <http://anzsoil.org/def/au/asls/substrate/Mass-genetic-type> ,
        <http://anzsoil.org/def/au/asls/substrate/Rock-genesis-hardened-evaporite> ,
        skos:Concept ;
    rdfs:isDefinedBy <http://anzsoil.org/def/au/asls/substrate> ;
    rdfs:seeAlso <http://anzsoil.org/def/au/asls/substrate> ;
    skos:definition "evaporite consisting of sodium chloride." ;
    skos:inScheme <http://anzsoil.org/def/au/asls/substrate> ;
    skos:notation "HA" ;
    skos:prefLabel "Halite (rock salt)"@en ;
    skos:topConceptOf <http://anzsoil.org/def/au/asls/substrate> ;
.

<http://anzsoil.org/def/au/asls/substrate/genesis-IG>
    a
        <http://anzsoil.org/def/au/asls/substrate/Mass-genetic-type> ,
        <http://anzsoil.org/def/au/asls/substrate/Rock-genesis-unweathered> ,
        skos:Concept ;
    rdfs:isDefinedBy <http://anzsoil.org/def/au/asls/substrate> ;
    rdfs:seeAlso <http://anzsoil.org/def/au/asls/substrate> ;
    skos:definition "strong or very strong rock masses formed by solidification of molten rock matter (magma) derived from below the Earth’s surface. The rocks are mainly composed of interlocking crystals. Types are distinguished in Table 34. Plutonic rocks and volcanic rocks are included." ;
    skos:inScheme <http://anzsoil.org/def/au/asls/substrate> ;
    skos:notation "IG" ;
    skos:prefLabel "Igneous rocks"@en ;
    skos:topConceptOf <http://anzsoil.org/def/au/asls/substrate> ;
.

<http://anzsoil.org/def/au/asls/substrate/genesis-IN>
    a
        <http://anzsoil.org/def/au/asls/substrate/Mass-genetic-type> ,
        <http://anzsoil.org/def/au/asls/substrate/Rock-genesis-unweathered> ,
        skos:Concept ;
    rdfs:isDefinedBy <http://anzsoil.org/def/au/asls/substrate> ;
    rdfs:seeAlso <http://anzsoil.org/def/au/asls/substrate> ;
    skos:definition "very weak to strong volcanic rock mass deposited from a flow of ash, the stronger forms being welded together by residual heat during deposition." ;
    skos:inScheme <http://anzsoil.org/def/au/asls/substrate> ;
    skos:notation "IN" ;
    skos:prefLabel "Ignimbrite"@en ;
    skos:topConceptOf <http://anzsoil.org/def/au/asls/substrate> ;
.

<http://anzsoil.org/def/au/asls/substrate/genesis-KC>
    a
        <http://anzsoil.org/def/au/asls/substrate/Mass-genetic-type> ,
        <http://anzsoil.org/def/au/asls/substrate/Rock-genesis-hardened-chemical> ,
        skos:Concept ;
    rdfs:isDefinedBy <http://anzsoil.org/def/au/asls/substrate> ;
    rdfs:seeAlso <http://anzsoil.org/def/au/asls/substrate> ;
    skos:definition "any cemented, terrestrial carbonate accumulation that may vary significantly in morphology and degree of cementation. Also known as carbonate pan, calcareous pan, caliche, kunkar, secondary limestone, travertine. All show slight to strong effervescence with 1-molar HCl." ;
    skos:inScheme <http://anzsoil.org/def/au/asls/substrate> ;
    skos:notation "KC" ;
    skos:prefLabel "Calcrete"@en ;
    skos:topConceptOf <http://anzsoil.org/def/au/asls/substrate> ;
.

<http://anzsoil.org/def/au/asls/substrate/genesis-LA>
    a
        <http://anzsoil.org/def/au/asls/substrate/Mass-genetic-type> ,
        <http://anzsoil.org/def/au/asls/substrate/Rock-genesis-sediments> ,
        skos:Concept ;
    rdfs:isDefinedBy <http://anzsoil.org/def/au/asls/substrate> ;
    rdfs:seeAlso <http://anzsoil.org/def/au/asls/substrate> ;
    skos:definition "sediment mass deposited from transport by waves and from sediment solution and suspension in still water in a closed depression on land." ;
    skos:inScheme <http://anzsoil.org/def/au/asls/substrate> ;
    skos:notation "LA" ;
    skos:prefLabel "Lacustrine sediment"@en ;
    skos:topConceptOf <http://anzsoil.org/def/au/asls/substrate> ;
.

<http://anzsoil.org/def/au/asls/substrate/genesis-LC>
    a
        <http://anzsoil.org/def/au/asls/substrate/Mass-genetic-type> ,
        <http://anzsoil.org/def/au/asls/substrate/Rock-genesis-hardened-chemical> ,
        skos:Concept ;
    rdfs:isDefinedBy <http://anzsoil.org/def/au/asls/substrate> ;
    rdfs:seeAlso <http://anzsoil.org/def/au/asls/substrate> ;
    skos:definition "strongly indurated siliceous material cemented by, and largely composed of, forms of silica, including quartz, chalcedony, opal and chert." ;
    skos:inScheme <http://anzsoil.org/def/au/asls/substrate> ;
    skos:notation "LC" ;
    skos:prefLabel "Silcrete"@en ;
    skos:topConceptOf <http://anzsoil.org/def/au/asls/substrate> ;
.

<http://anzsoil.org/def/au/asls/substrate/genesis-LD>
    a
        <http://anzsoil.org/def/au/asls/substrate/Mass-genetic-type> ,
        <http://anzsoil.org/def/au/asls/substrate/Rock-genesis-sediments> ,
        skos:Concept ;
    rdfs:isDefinedBy <http://anzsoil.org/def/au/asls/substrate> ;
    rdfs:seeAlso <http://anzsoil.org/def/au/asls/substrate> ;
    skos:definition "colluvium rapidly displaced many metres downslope by failure of a mass of earth or rock. If the mass is not already a part of the regolith, the landslide incorporates it in the regolith. Original rock structures are fragmented and disorganised by the action of the landslide." ;
    skos:inScheme <http://anzsoil.org/def/au/asls/substrate> ;
    skos:notation "LD" ;
    skos:prefLabel "Landslide deposit"@en ;
    skos:topConceptOf <http://anzsoil.org/def/au/asls/substrate> ;
.

<http://anzsoil.org/def/au/asls/substrate/genesis-LO>
    a
        <http://anzsoil.org/def/au/asls/substrate/Mass-genetic-type> ,
        <http://anzsoil.org/def/au/asls/substrate/Rock-genesis-sediments> ,
        skos:Concept ;
    rdfs:isDefinedBy <http://anzsoil.org/def/au/asls/substrate> ;
    rdfs:seeAlso <http://anzsoil.org/def/au/asls/substrate> ;
    skos:definition "eolian sediment of silt size." ;
    skos:inScheme <http://anzsoil.org/def/au/asls/substrate> ;
    skos:notation "LO" ;
    skos:prefLabel "Loess"@en ;
    skos:topConceptOf <http://anzsoil.org/def/au/asls/substrate> ;
.

<http://anzsoil.org/def/au/asls/substrate/genesis-MA>
    a
        <http://anzsoil.org/def/au/asls/substrate/Mass-genetic-type> ,
        <http://anzsoil.org/def/au/asls/substrate/Rock-genesis-sediments> ,
        skos:Concept ;
    rdfs:isDefinedBy <http://anzsoil.org/def/au/asls/substrate> ;
    rdfs:seeAlso <http://anzsoil.org/def/au/asls/substrate> ;
    skos:definition "sediment mass deposited from transport by waves and from solution and suspension in sea water." ;
    skos:inScheme <http://anzsoil.org/def/au/asls/substrate> ;
    skos:notation "MA" ;
    skos:prefLabel "Marine sediment"@en ;
    skos:topConceptOf <http://anzsoil.org/def/au/asls/substrate> ;
.

<http://anzsoil.org/def/au/asls/substrate/genesis-MD>
    a
        <http://anzsoil.org/def/au/asls/substrate/Mass-genetic-type> ,
        <http://anzsoil.org/def/au/asls/substrate/Rock-genesis-sediments> ,
        skos:Concept ;
    rdfs:isDefinedBy <http://anzsoil.org/def/au/asls/substrate> ;
    rdfs:seeAlso <http://anzsoil.org/def/au/asls/substrate> ;
    skos:definition "colluvium mixed with water to form dense fluid, and rapidly displaced metres or kilometres downslope. The material is more thoroughly disaggregated than that of a landslide deposit and lacks the bedding and sorting of grain sizes seen in alluvium." ;
    skos:inScheme <http://anzsoil.org/def/au/asls/substrate> ;
    skos:notation "MD" ;
    skos:prefLabel "Mudflow deposit"@en ;
    skos:topConceptOf <http://anzsoil.org/def/au/asls/substrate> ;
.

<http://anzsoil.org/def/au/asls/substrate/genesis-ME>
    a
        <http://anzsoil.org/def/au/asls/substrate/Mass-genetic-type> ,
        <http://anzsoil.org/def/au/asls/substrate/Rock-genesis-unweathered> ,
        skos:Concept ;
    rdfs:isDefinedBy <http://anzsoil.org/def/au/asls/substrate> ;
    rdfs:seeAlso <http://anzsoil.org/def/au/asls/substrate> ;
    skos:definition "moderately strong to very strong rock masses formed by the chemical and physical alterations of igneous or sedimentary rocks under high temperatures and/or very high pressures within the Earth’s crust. Types are distinguished in Table 34." ;
    skos:inScheme <http://anzsoil.org/def/au/asls/substrate> ;
    skos:notation "ME" ;
    skos:prefLabel "Metamorphic rocks"@en ;
    skos:topConceptOf <http://anzsoil.org/def/au/asls/substrate> ;
.

<http://anzsoil.org/def/au/asls/substrate/genesis-PA>
    a
        <http://anzsoil.org/def/au/asls/substrate/Mass-genetic-type> ,
        <http://anzsoil.org/def/au/asls/substrate/Rock-genesis-sediments> ,
        skos:Concept ;
    rdfs:isDefinedBy <http://anzsoil.org/def/au/asls/substrate> ;
    rdfs:seeAlso <http://anzsoil.org/def/au/asls/substrate> ;
    skos:definition "fine-grained calcareous eolian sediment consisting of 30–70% clay." ;
    skos:inScheme <http://anzsoil.org/def/au/asls/substrate> ;
    skos:notation "PA" ;
    skos:prefLabel "Parna"@en ;
    skos:topConceptOf <http://anzsoil.org/def/au/asls/substrate> ;
.

<http://anzsoil.org/def/au/asls/substrate/genesis-PC>
    a
        <http://anzsoil.org/def/au/asls/substrate/Mass-genetic-type> ,
        <http://anzsoil.org/def/au/asls/substrate/Rock-genesis-hardened-chemical> ,
        skos:Concept ;
    rdfs:isDefinedBy <http://anzsoil.org/def/au/asls/substrate> ;
    rdfs:seeAlso <http://anzsoil.org/def/au/asls/substrate> ;
    skos:definition "dense argillaceous rock of varying degree of silicification with a conchoidal fracture and general appearance of unglazed porcelain." ;
    skos:inScheme <http://anzsoil.org/def/au/asls/substrate> ;
    skos:notation "PC" ;
    skos:prefLabel "Porcellanite"@en ;
    skos:topConceptOf <http://anzsoil.org/def/au/asls/substrate> ;
.

<http://anzsoil.org/def/au/asls/substrate/genesis-PL>
    a
        <http://anzsoil.org/def/au/asls/substrate/Mass-genetic-type> ,
        <http://anzsoil.org/def/au/asls/substrate/Rock-genesis-unweathered> ,
        skos:Concept ;
    rdfs:isDefinedBy <http://anzsoil.org/def/au/asls/substrate> ;
    rdfs:seeAlso <http://anzsoil.org/def/au/asls/substrate> ;
    skos:definition "igneous rocks solidified at depth within the Earth’s crust." ;
    skos:inScheme <http://anzsoil.org/def/au/asls/substrate> ;
    skos:notation "PL" ;
    skos:prefLabel "Plutonic rocks"@en ;
    skos:topConceptOf <http://anzsoil.org/def/au/asls/substrate> ;
.

<http://anzsoil.org/def/au/asls/substrate/genesis-PW>
    a
        <http://anzsoil.org/def/au/asls/substrate/Mass-genetic-type> ,
        <http://anzsoil.org/def/au/asls/substrate/Rock-genesis-weathered> ,
        skos:Concept ;
    rdfs:isDefinedBy <http://anzsoil.org/def/au/asls/substrate> ;
    rdfs:seeAlso <http://anzsoil.org/def/au/asls/substrate> ;
    skos:definition "weathered material produced by exposure of rock masses to land surface processes but with no transport. Partial decomposition results in changes in colour, texture, composition, strength or form of the parent rock mass (see also decomposed rock and saprolite)." ;
    skos:inScheme <http://anzsoil.org/def/au/asls/substrate> ;
    skos:notation "PW" ;
    skos:prefLabel "Partially weathered rock"@en ;
    skos:topConceptOf <http://anzsoil.org/def/au/asls/substrate> ;
.

<http://anzsoil.org/def/au/asls/substrate/genesis-RB>
    a
        <http://anzsoil.org/def/au/asls/substrate/Mass-genetic-type> ,
        <http://anzsoil.org/def/au/asls/substrate/Rock-genesis-hardened-chemical> ,
        skos:Concept ;
    rdfs:isDefinedBy <http://anzsoil.org/def/au/asls/substrate> ;
    rdfs:seeAlso <http://anzsoil.org/def/au/asls/substrate> ;
    skos:definition "an informal name used for a particular indurated earthy material (see ‘Pans’, page 143). In many instances it is not known if the red-brown hardpan is a paleosol or a cemented sediment.*" ;
    skos:inScheme <http://anzsoil.org/def/au/asls/substrate> ;
    skos:notation "RB" ;
    skos:prefLabel "Red-brown hardpan"@en ;
    skos:topConceptOf <http://anzsoil.org/def/au/asls/substrate> ;
.

<http://anzsoil.org/def/au/asls/substrate/genesis-SA>
    a
        <http://anzsoil.org/def/au/asls/substrate/Mass-genetic-type> ,
        <http://anzsoil.org/def/au/asls/substrate/Rock-genesis-weathered> ,
        skos:Concept ;
    rdfs:isDefinedBy <http://anzsoil.org/def/au/asls/substrate> ;
    rdfs:seeAlso <http://anzsoil.org/def/au/asls/substrate> ;
    skos:definition "a particular form of decomposed rock. It is characterised by the preservation of structures (including ‘texture’ in the petrological sense) that were present in the unweathered rock." ;
    skos:inScheme <http://anzsoil.org/def/au/asls/substrate> ;
    skos:notation "SA" ;
    skos:prefLabel "Saprolite"@en ;
    skos:topConceptOf <http://anzsoil.org/def/au/asls/substrate> ;
.

<http://anzsoil.org/def/au/asls/substrate/genesis-SC>
    a
        <http://anzsoil.org/def/au/asls/substrate/Mass-genetic-type> ,
        <http://anzsoil.org/def/au/asls/substrate/Rock-genesis-unweathered> ,
        skos:Concept ;
    rdfs:isDefinedBy <http://anzsoil.org/def/au/asls/substrate> ;
    rdfs:seeAlso <http://anzsoil.org/def/au/asls/substrate> ;
    skos:definition "sedimentary rocks in which mineral grains or fragments are not important constituents. The group includes coal, chert and non-fragmental limestones as well as saline rocks (evaporites) such as halite (rock salt) and gypsum. Chemical and organic sedimentary rocks are common in the regolith zone." ;
    skos:inScheme <http://anzsoil.org/def/au/asls/substrate> ;
    skos:notation "SC" ;
    skos:prefLabel "Chemical and organic sedimentary rocks"@en ;
    skos:topConceptOf <http://anzsoil.org/def/au/asls/substrate> ;
.

<http://anzsoil.org/def/au/asls/substrate/genesis-SD>
    a
        <http://anzsoil.org/def/au/asls/substrate/Mass-genetic-type> ,
        <http://anzsoil.org/def/au/asls/substrate/Rock-genesis-unweathered> ,
        skos:Concept ;
    rdfs:isDefinedBy <http://anzsoil.org/def/au/asls/substrate> ;
    rdfs:seeAlso <http://anzsoil.org/def/au/asls/substrate> ;
    skos:definition "sedimentary rocks composed of mineral grains or fragments derived from pre-existing rocks. Types are distinguished in Table 34." ;
    skos:inScheme <http://anzsoil.org/def/au/asls/substrate> ;
    skos:notation "SD" ;
    skos:prefLabel "Detrital sedimentary rocks"@en ;
    skos:topConceptOf <http://anzsoil.org/def/au/asls/substrate> ;
.

<http://anzsoil.org/def/au/asls/substrate/genesis-SE>
    a
        <http://anzsoil.org/def/au/asls/substrate/Mass-genetic-type> ,
        <http://anzsoil.org/def/au/asls/substrate/Rock-genesis-sediments> ,
        skos:Concept ;
    rdfs:isDefinedBy <http://anzsoil.org/def/au/asls/substrate> ;
    rdfs:seeAlso <http://anzsoil.org/def/au/asls/substrate> ;
    skos:definition "colluvium deposited after falling or rolling from cliffed or steep slopes, consisting of loose rock fragments of gravel size or larger and generally lacking a fine interstitial component." ;
    skos:inScheme <http://anzsoil.org/def/au/asls/substrate> ;
    skos:notation "SE" ;
    skos:prefLabel "Scree"@en ;
    skos:topConceptOf <http://anzsoil.org/def/au/asls/substrate> ;
.

<http://anzsoil.org/def/au/asls/substrate/genesis-SH>
    a
        <http://anzsoil.org/def/au/asls/substrate/Mass-genetic-type> ,
        <http://anzsoil.org/def/au/asls/substrate/Rock-genesis-sediments> ,
        skos:Concept ;
    rdfs:isDefinedBy <http://anzsoil.org/def/au/asls/substrate> ;
    rdfs:seeAlso <http://anzsoil.org/def/au/asls/substrate> ;
    skos:definition "colluvium deposited from transport by a very shallow flow of water as a sheet, or network of rills on the land surface. Sheet flow deposits are very thin except at the foot of a slope and beneath sheet-flood fans." ;
    skos:inScheme <http://anzsoil.org/def/au/asls/substrate> ;
    skos:notation "SH" ;
    skos:prefLabel "Sheet flow deposit"@en ;
    skos:topConceptOf <http://anzsoil.org/def/au/asls/substrate> ;
.

<http://anzsoil.org/def/au/asls/substrate/genesis-SP>
    a
        <http://anzsoil.org/def/au/asls/substrate/Mass-genetic-type> ,
        <http://anzsoil.org/def/au/asls/substrate/Rock-genesis-unweathered> ,
        skos:Concept ;
    rdfs:isDefinedBy <http://anzsoil.org/def/au/asls/substrate> ;
    rdfs:seeAlso <http://anzsoil.org/def/au/asls/substrate> ;
    skos:definition "sedimentary rocks resulting from the deposition of airborne materials produced by volcanic eruptions." ;
    skos:inScheme <http://anzsoil.org/def/au/asls/substrate> ;
    skos:notation "SP" ;
    skos:prefLabel "Pyroclastic rocks"@en ;
    skos:topConceptOf <http://anzsoil.org/def/au/asls/substrate> ;
.

<http://anzsoil.org/def/au/asls/substrate/genesis-SR>
    a
        <http://anzsoil.org/def/au/asls/substrate/Mass-genetic-type> ,
        <http://anzsoil.org/def/au/asls/substrate/Rock-genesis-unweathered> ,
        skos:Concept ;
    rdfs:isDefinedBy <http://anzsoil.org/def/au/asls/substrate> ;
    rdfs:seeAlso <http://anzsoil.org/def/au/asls/substrate> ;
    skos:definition "weak or moderately strong rock masses formed by the hardening of sediments due to compaction, recrystallisation or cementation. These processes can occur within the regolith but are promoted by burial within the Earth’s crust. Major categories of sedimentary rocks are detrital sedimentary rocks, pyroclastic rocks, and chemical and organic sedimentary rocks." ;
    skos:inScheme <http://anzsoil.org/def/au/asls/substrate> ;
    skos:notation "SR" ;
    skos:prefLabel "Sedimentary rocks"@en ;
    skos:topConceptOf <http://anzsoil.org/def/au/asls/substrate> ;
.

<http://anzsoil.org/def/au/asls/substrate/genesis-ST>
    a
        <http://anzsoil.org/def/au/asls/substrate/Mass-genetic-type> ,
        <http://anzsoil.org/def/au/asls/substrate/Rock-genesis-hardened-artificial> ,
        skos:Concept ;
    rdfs:isDefinedBy <http://anzsoil.org/def/au/asls/substrate> ;
    rdfs:seeAlso <http://anzsoil.org/def/au/asls/substrate> ;
    skos:definition "artificial mass with the strength grade of very weak rock. It results from the ‘stabilisation’ of an earth mass by a variety of processes: compaction; the admixture of lime, Portland cement, bitumen or other substances; heating; freezing; or electro-hardening. Cement stabilisation can produce a mass as strong as 10 MPa unconfined compressive strength.*" ;
    skos:inScheme <http://anzsoil.org/def/au/asls/substrate> ;
    skos:notation "ST" ;
    skos:prefLabel "Stabilised soil"@en ;
    skos:topConceptOf <http://anzsoil.org/def/au/asls/substrate> ;
.

<http://anzsoil.org/def/au/asls/substrate/genesis-TI>
    a
        <http://anzsoil.org/def/au/asls/substrate/Mass-genetic-type> ,
        <http://anzsoil.org/def/au/asls/substrate/Rock-genesis-sediments> ,
        skos:Concept ;
    rdfs:isDefinedBy <http://anzsoil.org/def/au/asls/substrate> ;
    rdfs:seeAlso <http://anzsoil.org/def/au/asls/substrate> ;
    skos:definition "sediment mass deposited from transport in ice, as in a glacier. Till is neither bedded nor sorted; it has a matrix of clay or silt enclosing larger particles of unweathered rock ranging up to large boulders." ;
    skos:inScheme <http://anzsoil.org/def/au/asls/substrate> ;
    skos:notation "TI" ;
    skos:prefLabel "Till"@en ;
    skos:topConceptOf <http://anzsoil.org/def/au/asls/substrate> ;
.

<http://anzsoil.org/def/au/asls/substrate/genesis-VA>
    a
        <http://anzsoil.org/def/au/asls/substrate/Mass-genetic-type> ,
        <http://anzsoil.org/def/au/asls/substrate/Rock-genesis-sediments> ,
        skos:Concept ;
    rdfs:isDefinedBy <http://anzsoil.org/def/au/asls/substrate> ;
    rdfs:seeAlso <http://anzsoil.org/def/au/asls/substrate> ;
    skos:definition "eolian sediment consisting of relatively fine (<2 mm) pyroclastic material. It often contains a proportion of highly weatherable glass." ;
    skos:inScheme <http://anzsoil.org/def/au/asls/substrate> ;
    skos:notation "VA" ;
    skos:prefLabel "Volcanic ash"@en ;
    skos:topConceptOf <http://anzsoil.org/def/au/asls/substrate> ;
.

<http://anzsoil.org/def/au/asls/substrate/genesis-VO>
    a
        <http://anzsoil.org/def/au/asls/substrate/Mass-genetic-type> ,
        <http://anzsoil.org/def/au/asls/substrate/Rock-genesis-unweathered> ,
        skos:Concept ;
    rdfs:isDefinedBy <http://anzsoil.org/def/au/asls/substrate> ;
    rdfs:seeAlso <http://anzsoil.org/def/au/asls/substrate> ;
    skos:definition "igneous rocks solidified after eruption on to the land surface." ;
    skos:inScheme <http://anzsoil.org/def/au/asls/substrate> ;
    skos:notation "VO" ;
    skos:prefLabel "Volcanic rocks"@en ;
    skos:topConceptOf <http://anzsoil.org/def/au/asls/substrate> ;
.

<http://anzsoil.org/def/au/asls/substrate/grain-size-1>
    a
        <http://anzsoil.org/def/au/asls/substrate/Substrate-grain-size> ,
        skos:Concept ;
    rdfs:isDefinedBy <http://anzsoil.org/def/au/asls/substrate> ;
    rdfs:seeAlso <http://anzsoil.org/def/au/asls/substrate> ;
    skos:definition "<0.06 mm:	silt- or clay-sized; grains not visible; for example chert, shale, basalt, silt, coal." ;
    skos:inScheme <http://anzsoil.org/def/au/asls/substrate> ;
    skos:notation "1" ;
    skos:prefLabel "<0.06 mm"@en ;
    skos:topConceptOf <http://anzsoil.org/def/au/asls/substrate> ;
.

<http://anzsoil.org/def/au/asls/substrate/grain-size-2>
    a
        <http://anzsoil.org/def/au/asls/substrate/Substrate-grain-size> ,
        skos:Concept ;
    rdfs:isDefinedBy <http://anzsoil.org/def/au/asls/substrate> ;
    rdfs:seeAlso <http://anzsoil.org/def/au/asls/substrate> ;
    skos:definition "0.06–2 mm:	sand-sized; grains visible; for example sand, sandstone, dolerite, porphyry, sandy tuff, graywacke, micro-granite, schist, quartzite." ;
    skos:inScheme <http://anzsoil.org/def/au/asls/substrate> ;
    skos:notation "2" ;
    skos:prefLabel "0.06-2 mm"@en ;
    skos:topConceptOf <http://anzsoil.org/def/au/asls/substrate> ;
.

<http://anzsoil.org/def/au/asls/substrate/grain-size-3>
    a
        <http://anzsoil.org/def/au/asls/substrate/Substrate-grain-size> ,
        skos:Concept ;
    rdfs:isDefinedBy <http://anzsoil.org/def/au/asls/substrate> ;
    rdfs:seeAlso <http://anzsoil.org/def/au/asls/substrate> ;
    skos:definition ">2 mm:	gravel-sized; for example gravel, conglomerate, breccia, pebbles, cobbles, stones, boulders, pegmatite, granite, agglomerate." ;
    skos:inScheme <http://anzsoil.org/def/au/asls/substrate> ;
    skos:notation "3" ;
    skos:prefLabel ">2 mm"@en ;
    skos:topConceptOf <http://anzsoil.org/def/au/asls/substrate> ;
.

<http://anzsoil.org/def/au/asls/substrate/lithology-AC>
    a
        <http://anzsoil.org/def/au/asls/substrate/Lithology-rock> ,
        skos:Concept ;
    rdfs:isDefinedBy <http://anzsoil.org/def/au/asls/substrate> ;
    rdfs:seeAlso <http://anzsoil.org/def/au/asls/substrate> ;
    skos:altLabel "Bauxite"@en ;
    skos:definition "Alcrete (Sedimentary rock, chemical or organic)"@en ;
    skos:inScheme <http://anzsoil.org/def/au/asls/substrate> ;
    skos:notation "AC" ;
    skos:note "C_LITHOLOGY" ;
    skos:prefLabel "Alcrete"@en ;
    skos:topConceptOf <http://anzsoil.org/def/au/asls/substrate> ;
.

<http://anzsoil.org/def/au/asls/substrate/lithology-AD>
    a
        <http://anzsoil.org/def/au/asls/substrate/Lithology-rock> ,
        skos:Concept ;
    rdfs:isDefinedBy <http://anzsoil.org/def/au/asls/substrate> ;
    rdfs:seeAlso <http://anzsoil.org/def/au/asls/substrate> ;
    skos:definition "Adamellite (Igneous rock)"@en ;
    skos:inScheme <http://anzsoil.org/def/au/asls/substrate> ;
    skos:notation "AD" ;
    skos:note "C_LITHOLOGY" ;
    skos:prefLabel "Adamellite"@en ;
    skos:topConceptOf <http://anzsoil.org/def/au/asls/substrate> ;
.

<http://anzsoil.org/def/au/asls/substrate/lithology-AG>
    a
        <http://anzsoil.org/def/au/asls/substrate/Lithology-rock> ,
        skos:Concept ;
    rdfs:isDefinedBy <http://anzsoil.org/def/au/asls/substrate> ;
    rdfs:seeAlso <http://anzsoil.org/def/au/asls/substrate> ;
    skos:definition "Agglomerate (Sedimentary rock, pyroclastic)"@en ;
    skos:inScheme <http://anzsoil.org/def/au/asls/substrate> ;
    skos:notation "AG" ;
    skos:note "C_LITHOLOGY" ;
    skos:prefLabel "Agglomerate"@en ;
    skos:topConceptOf <http://anzsoil.org/def/au/asls/substrate> ;
.

<http://anzsoil.org/def/au/asls/substrate/lithology-AH>
    a
        <http://anzsoil.org/def/au/asls/substrate/Lithology-rock> ,
        skos:Concept ;
    rdfs:isDefinedBy <http://anzsoil.org/def/au/asls/substrate> ;
    rdfs:seeAlso <http://anzsoil.org/def/au/asls/substrate> ;
    skos:definition "Anhydrite (Sedimentary rock, chemical or organic)"@en ;
    skos:inScheme <http://anzsoil.org/def/au/asls/substrate> ;
    skos:notation "AH" ;
    skos:note "C_LITHOLOGY" ;
    skos:prefLabel "Anhydrite"@en ;
    skos:topConceptOf <http://anzsoil.org/def/au/asls/substrate> ;
.

<http://anzsoil.org/def/au/asls/substrate/lithology-AM>
    a
        <http://anzsoil.org/def/au/asls/substrate/Lithology-rock> ,
        skos:Concept ;
    rdfs:isDefinedBy <http://anzsoil.org/def/au/asls/substrate> ;
    rdfs:seeAlso <http://anzsoil.org/def/au/asls/substrate> ;
    skos:definition "Amphibolite (Metamorphic rock)"@en ;
    skos:inScheme <http://anzsoil.org/def/au/asls/substrate> ;
    skos:notation "AM" ;
    skos:note "C_LITHOLOGY" ;
    skos:prefLabel "Amphibolite"@en ;
    skos:topConceptOf <http://anzsoil.org/def/au/asls/substrate> ;
.

<http://anzsoil.org/def/au/asls/substrate/lithology-AN>
    a
        <http://anzsoil.org/def/au/asls/substrate/Lithology-rock> ,
        skos:Concept ;
    rdfs:isDefinedBy <http://anzsoil.org/def/au/asls/substrate> ;
    rdfs:seeAlso <http://anzsoil.org/def/au/asls/substrate> ;
    skos:definition "Andesite (Igneous rock)"@en ;
    skos:inScheme <http://anzsoil.org/def/au/asls/substrate> ;
    skos:notation "AN" ;
    skos:note "C_LITHOLOGY" ;
    skos:prefLabel "Andesite"@en ;
    skos:topConceptOf <http://anzsoil.org/def/au/asls/substrate> ;
.

<http://anzsoil.org/def/au/asls/substrate/lithology-AP>
    a
        <http://anzsoil.org/def/au/asls/substrate/Lithology-rock> ,
        skos:Concept ;
    rdfs:isDefinedBy <http://anzsoil.org/def/au/asls/substrate> ;
    rdfs:seeAlso <http://anzsoil.org/def/au/asls/substrate> ;
    skos:definition "Aplite (Igneous rock)"@en ;
    skos:inScheme <http://anzsoil.org/def/au/asls/substrate> ;
    skos:notation "AP" ;
    skos:note "C_LITHOLOGY" ;
    skos:prefLabel "Aplite"@en ;
    skos:topConceptOf <http://anzsoil.org/def/au/asls/substrate> ;
.

<http://anzsoil.org/def/au/asls/substrate/lithology-AR>
    a
        <http://anzsoil.org/def/au/asls/substrate/Lithology-rock> ,
        skos:Concept ;
    rdfs:isDefinedBy <http://anzsoil.org/def/au/asls/substrate> ;
    rdfs:seeAlso <http://anzsoil.org/def/au/asls/substrate> ;
    skos:definition "Arkose (Sedimentary rock, detrital)"@en ;
    skos:inScheme <http://anzsoil.org/def/au/asls/substrate> ;
    skos:notation "AR" ;
    skos:note "C_LITHOLOGY" ;
    skos:prefLabel "Arkose"@en ;
    skos:topConceptOf <http://anzsoil.org/def/au/asls/substrate> ;
.

<http://anzsoil.org/def/au/asls/substrate/lithology-BA>
    a
        <http://anzsoil.org/def/au/asls/substrate/Lithology-rock> ,
        skos:Concept ;
    rdfs:isDefinedBy <http://anzsoil.org/def/au/asls/substrate> ;
    rdfs:seeAlso <http://anzsoil.org/def/au/asls/substrate> ;
    skos:definition "Basalt (Igneous rock)"@en ;
    skos:inScheme <http://anzsoil.org/def/au/asls/substrate> ;
    skos:notation "BA" ;
    skos:note "C_LITHOLOGY" ;
    skos:prefLabel "Basalt"@en ;
    skos:topConceptOf <http://anzsoil.org/def/au/asls/substrate> ;
.

<http://anzsoil.org/def/au/asls/substrate/lithology-BO>
    a
        <http://anzsoil.org/def/au/asls/substrate/Lithology-unconsolidated> ,
        skos:Concept ;
    dcterms:identifier "http://anzsoil.org/def/au/asls/substrate/lithology-BO" ;
    rdfs:isDefinedBy <http://anzsoil.org/def/au/asls/substrate> ;
    rdfs:seeAlso <http://anzsoil.org/def/au/asls/substrate> ;
    skos:definition """Very coarse grained
>60 mm
Non-volcanic
Without significant carbonate""" ;
    skos:inScheme <http://anzsoil.org/def/au/asls/substrate> ;
    skos:notation "BO" ;
    skos:prefLabel "Boulders"@en ;
    skos:topConceptOf <http://anzsoil.org/def/au/asls/substrate> ;
.

<http://anzsoil.org/def/au/asls/substrate/lithology-BR>
    a
        <http://anzsoil.org/def/au/asls/substrate/Lithology-rock> ,
        skos:Concept ;
    rdfs:isDefinedBy <http://anzsoil.org/def/au/asls/substrate> ;
    rdfs:seeAlso <http://anzsoil.org/def/au/asls/substrate> ;
    skos:definition "Breccia (Sedimentary rock, detrital)"@en ;
    skos:inScheme <http://anzsoil.org/def/au/asls/substrate> ;
    skos:notation "BR" ;
    skos:note "C_LITHOLOGY" ;
    skos:prefLabel "Breccia"@en ;
    skos:topConceptOf <http://anzsoil.org/def/au/asls/substrate> ;
.

<http://anzsoil.org/def/au/asls/substrate/lithology-CB>
    a
        <http://anzsoil.org/def/au/asls/substrate/Lithology-unconsolidated> ,
        skos:Concept ;
    dcterms:identifier "http://anzsoil.org/def/au/asls/substrate/lithology-CB" ;
    rdfs:isDefinedBy <http://anzsoil.org/def/au/asls/substrate> ;
    rdfs:seeAlso <http://anzsoil.org/def/au/asls/substrate> ;
    skos:definition """Very coarse grained
>60 mm
Non-volcanic
Without significant carbonate""" ;
    skos:inScheme <http://anzsoil.org/def/au/asls/substrate> ;
    skos:notation "CB" ;
    skos:prefLabel "Cobbles"@en ;
    skos:topConceptOf <http://anzsoil.org/def/au/asls/substrate> ;
.

<http://anzsoil.org/def/au/asls/substrate/lithology-CG>
    a
        <http://anzsoil.org/def/au/asls/substrate/Lithology-rock> ,
        skos:Concept ;
    rdfs:isDefinedBy <http://anzsoil.org/def/au/asls/substrate> ;
    rdfs:seeAlso <http://anzsoil.org/def/au/asls/substrate> ;
    skos:definition "Conglomerate (Sedimentary rock, detrital)"@en ;
    skos:inScheme <http://anzsoil.org/def/au/asls/substrate> ;
    skos:notation "CG" ;
    skos:note "C_LITHOLOGY" ;
    skos:prefLabel "Conglomerate"@en ;
    skos:topConceptOf <http://anzsoil.org/def/au/asls/substrate> ;
.

<http://anzsoil.org/def/au/asls/substrate/lithology-CH>
    a
        <http://anzsoil.org/def/au/asls/substrate/Lithology-rock> ,
        skos:Concept ;
    rdfs:isDefinedBy <http://anzsoil.org/def/au/asls/substrate> ;
    rdfs:seeAlso <http://anzsoil.org/def/au/asls/substrate> ;
    skos:definition "Chert (Sedimentary rock, chemical or organic)"@en ;
    skos:inScheme <http://anzsoil.org/def/au/asls/substrate> ;
    skos:notation "CH" ;
    skos:note "C_LITHOLOGY" ;
    skos:prefLabel "Chert"@en ;
    skos:topConceptOf <http://anzsoil.org/def/au/asls/substrate> ;
.

<http://anzsoil.org/def/au/asls/substrate/lithology-CO>
    a
        <http://anzsoil.org/def/au/asls/substrate/Lithology-rock> ,
        skos:Concept ;
    rdfs:isDefinedBy <http://anzsoil.org/def/au/asls/substrate> ;
    rdfs:seeAlso <http://anzsoil.org/def/au/asls/substrate> ;
    skos:definition "Coal (Sedimentary rock, chemical or organic)"@en ;
    skos:inScheme <http://anzsoil.org/def/au/asls/substrate> ;
    skos:notation "CO" ;
    skos:note "C_LITHOLOGY" ;
    skos:prefLabel "Coal"@en ;
    skos:topConceptOf <http://anzsoil.org/def/au/asls/substrate> ;
.

<http://anzsoil.org/def/au/asls/substrate/lithology-CU>
    a
        <http://anzsoil.org/def/au/asls/substrate/Lithology-rock> ,
        skos:Concept ;
    rdfs:isDefinedBy <http://anzsoil.org/def/au/asls/substrate> ;
    rdfs:seeAlso <http://anzsoil.org/def/au/asls/substrate> ;
    skos:definition "Consolidated rock (Unidentified)"@en ;
    skos:inScheme <http://anzsoil.org/def/au/asls/substrate> ;
    skos:notation "CU" ;
    skos:note "C_LITHOLOGY" ;
    skos:prefLabel "Consolidated rock"@en ;
    skos:topConceptOf <http://anzsoil.org/def/au/asls/substrate> ;
.

<http://anzsoil.org/def/au/asls/substrate/lithology-DI>
    a
        <http://anzsoil.org/def/au/asls/substrate/Lithology-rock> ,
        skos:Concept ;
    rdfs:isDefinedBy <http://anzsoil.org/def/au/asls/substrate> ;
    rdfs:seeAlso <http://anzsoil.org/def/au/asls/substrate> ;
    skos:definition "Diorite (Igneous rock)"@en ;
    skos:inScheme <http://anzsoil.org/def/au/asls/substrate> ;
    skos:notation "DI" ;
    skos:note "C_LITHOLOGY" ;
    skos:prefLabel "Diorite"@en ;
    skos:topConceptOf <http://anzsoil.org/def/au/asls/substrate> ;
.

<http://anzsoil.org/def/au/asls/substrate/lithology-DM>
    a
        <http://anzsoil.org/def/au/asls/substrate/Lithology-rock> ,
        skos:Concept ;
    rdfs:isDefinedBy <http://anzsoil.org/def/au/asls/substrate> ;
    rdfs:seeAlso <http://anzsoil.org/def/au/asls/substrate> ;
    skos:definition "Dolomite (Sedimentary rock, detrital)"@en ;
    skos:inScheme <http://anzsoil.org/def/au/asls/substrate> ;
    skos:notation "DM" ;
    skos:note "C_LITHOLOGY" ;
    skos:prefLabel "Dolomite"@en ;
    skos:topConceptOf <http://anzsoil.org/def/au/asls/substrate> ;
.

<http://anzsoil.org/def/au/asls/substrate/lithology-DR>
    a
        <http://anzsoil.org/def/au/asls/substrate/Lithology-rock> ,
        skos:Concept ;
    rdfs:isDefinedBy <http://anzsoil.org/def/au/asls/substrate> ;
    rdfs:seeAlso <http://anzsoil.org/def/au/asls/substrate> ;
    skos:definition "Dolerite (Igneous rock)"@en ;
    skos:inScheme <http://anzsoil.org/def/au/asls/substrate> ;
    skos:notation "DR" ;
    skos:note "C_LITHOLOGY" ;
    skos:prefLabel "Dolerite"@en ;
    skos:topConceptOf <http://anzsoil.org/def/au/asls/substrate> ;
.

<http://anzsoil.org/def/au/asls/substrate/lithology-FC>
    a
        <http://anzsoil.org/def/au/asls/substrate/Lithology-rock> ,
        skos:Concept ;
    rdfs:isDefinedBy <http://anzsoil.org/def/au/asls/substrate> ;
    rdfs:seeAlso <http://anzsoil.org/def/au/asls/substrate> ;
    skos:definition "Ferricrete (Sedimentary rock, chemical or organic)"@en ;
    skos:inScheme <http://anzsoil.org/def/au/asls/substrate> ;
    skos:notation "FC" ;
    skos:note "C_LITHOLOGY" ;
    skos:prefLabel "Ferricrete"@en ;
    skos:topConceptOf <http://anzsoil.org/def/au/asls/substrate> ;
.

<http://anzsoil.org/def/au/asls/substrate/lithology-GA>
    a
        <http://anzsoil.org/def/au/asls/substrate/Lithology-rock> ,
        skos:Concept ;
    rdfs:isDefinedBy <http://anzsoil.org/def/au/asls/substrate> ;
    rdfs:seeAlso <http://anzsoil.org/def/au/asls/substrate> ;
    skos:definition "Gabbro (Igneous rock)"@en ;
    skos:inScheme <http://anzsoil.org/def/au/asls/substrate> ;
    skos:notation "GA" ;
    skos:note "C_LITHOLOGY" ;
    skos:prefLabel "Gabbro"@en ;
    skos:topConceptOf <http://anzsoil.org/def/au/asls/substrate> ;
.

<http://anzsoil.org/def/au/asls/substrate/lithology-GD>
    a
        <http://anzsoil.org/def/au/asls/substrate/Lithology-rock> ,
        skos:Concept ;
    rdfs:isDefinedBy <http://anzsoil.org/def/au/asls/substrate> ;
    rdfs:seeAlso <http://anzsoil.org/def/au/asls/substrate> ;
    skos:definition "Granodiorite (Igneous rock)"@en ;
    skos:inScheme <http://anzsoil.org/def/au/asls/substrate> ;
    skos:notation "GD" ;
    skos:note "C_LITHOLOGY" ;
    skos:prefLabel "Granodiorite"@en ;
    skos:topConceptOf <http://anzsoil.org/def/au/asls/substrate> ;
.

<http://anzsoil.org/def/au/asls/substrate/lithology-GE>
    a
        <http://anzsoil.org/def/au/asls/substrate/Lithology-rock> ,
        skos:Concept ;
    rdfs:isDefinedBy <http://anzsoil.org/def/au/asls/substrate> ;
    rdfs:seeAlso <http://anzsoil.org/def/au/asls/substrate> ;
    skos:definition "Greenstone (Metamorphic rock)"@en ;
    skos:inScheme <http://anzsoil.org/def/au/asls/substrate> ;
    skos:notation "GE" ;
    skos:note "C_LITHOLOGY" ;
    skos:prefLabel "Greenstone"@en ;
    skos:topConceptOf <http://anzsoil.org/def/au/asls/substrate> ;
.

<http://anzsoil.org/def/au/asls/substrate/lithology-GN>
    a
        <http://anzsoil.org/def/au/asls/substrate/Lithology-rock> ,
        skos:Concept ;
    rdfs:isDefinedBy <http://anzsoil.org/def/au/asls/substrate> ;
    rdfs:seeAlso <http://anzsoil.org/def/au/asls/substrate> ;
    skos:definition "Granite (Igneous rock)"@en ;
    skos:inScheme <http://anzsoil.org/def/au/asls/substrate> ;
    skos:notation "GN" ;
    skos:note "C_LITHOLOGY" ;
    skos:prefLabel "Granite"@en ;
    skos:topConceptOf <http://anzsoil.org/def/au/asls/substrate> ;
.

<http://anzsoil.org/def/au/asls/substrate/lithology-GR>
    a
        <http://anzsoil.org/def/au/asls/substrate/Lithology-rock> ,
        skos:Concept ;
    rdfs:isDefinedBy <http://anzsoil.org/def/au/asls/substrate> ;
    rdfs:seeAlso <http://anzsoil.org/def/au/asls/substrate> ;
    skos:definition "Granulite (Metamorphic rock)"@en ;
    skos:inScheme <http://anzsoil.org/def/au/asls/substrate> ;
    skos:notation "GR" ;
    skos:note "C_LITHOLOGY" ;
    skos:prefLabel "Granulite"@en ;
    skos:topConceptOf <http://anzsoil.org/def/au/asls/substrate> ;
.

<http://anzsoil.org/def/au/asls/substrate/lithology-GS>
    a
        <http://anzsoil.org/def/au/asls/substrate/Lithology-rock> ,
        skos:Concept ;
    rdfs:isDefinedBy <http://anzsoil.org/def/au/asls/substrate> ;
    rdfs:seeAlso <http://anzsoil.org/def/au/asls/substrate> ;
    skos:definition "Gneiss (Metamorphic rock)"@en ;
    skos:inScheme <http://anzsoil.org/def/au/asls/substrate> ;
    skos:notation "GS" ;
    skos:note "C_LITHOLOGY" ;
    skos:prefLabel "Gneiss"@en ;
    skos:topConceptOf <http://anzsoil.org/def/au/asls/substrate> ;
.

<http://anzsoil.org/def/au/asls/substrate/lithology-GW>
    a
        <http://anzsoil.org/def/au/asls/substrate/Lithology-rock> ,
        skos:Concept ;
    rdfs:isDefinedBy <http://anzsoil.org/def/au/asls/substrate> ;
    rdfs:seeAlso <http://anzsoil.org/def/au/asls/substrate> ;
    skos:definition "Graywacke (Sedimentary rock, detrital)"@en ;
    skos:inScheme <http://anzsoil.org/def/au/asls/substrate> ;
    skos:notation "GW" ;
    skos:note "C_LITHOLOGY" ;
    skos:prefLabel "Graywacke"@en ;
    skos:topConceptOf <http://anzsoil.org/def/au/asls/substrate> ;
.

<http://anzsoil.org/def/au/asls/substrate/lithology-GY>
    a
        <http://anzsoil.org/def/au/asls/substrate/Lithology-rock> ,
        skos:Concept ;
    rdfs:isDefinedBy <http://anzsoil.org/def/au/asls/substrate> ;
    rdfs:seeAlso <http://anzsoil.org/def/au/asls/substrate> ;
    skos:definition "Gypsum (Sedimentary rock, chemical or organic)"@en ;
    skos:inScheme <http://anzsoil.org/def/au/asls/substrate> ;
    skos:notation "GY" ;
    skos:note "C_LITHOLOGY" ;
    skos:prefLabel "Gypsum"@en ;
    skos:topConceptOf <http://anzsoil.org/def/au/asls/substrate> ;
.

<http://anzsoil.org/def/au/asls/substrate/lithology-HA>
    a
        <http://anzsoil.org/def/au/asls/substrate/Lithology-rock> ,
        skos:Concept ;
    rdfs:isDefinedBy <http://anzsoil.org/def/au/asls/substrate> ;
    rdfs:seeAlso <http://anzsoil.org/def/au/asls/substrate> ;
    skos:definition "Halite (Sedimentary rock, chemical or organic)"@en ;
    skos:inScheme <http://anzsoil.org/def/au/asls/substrate> ;
    skos:notation "HA" ;
    skos:note "C_LITHOLOGY" ;
    skos:prefLabel "Halite"@en ;
    skos:topConceptOf <http://anzsoil.org/def/au/asls/substrate> ;
.

<http://anzsoil.org/def/au/asls/substrate/lithology-HO>
    a
        <http://anzsoil.org/def/au/asls/substrate/Lithology-rock> ,
        skos:Concept ;
    rdfs:isDefinedBy <http://anzsoil.org/def/au/asls/substrate> ;
    rdfs:seeAlso <http://anzsoil.org/def/au/asls/substrate> ;
    skos:definition "Hornfels (Metamorphic rock)"@en ;
    skos:inScheme <http://anzsoil.org/def/au/asls/substrate> ;
    skos:notation "HO" ;
    skos:note "C_LITHOLOGY" ;
    skos:prefLabel "Hornfels"@en ;
    skos:topConceptOf <http://anzsoil.org/def/au/asls/substrate> ;
.

<http://anzsoil.org/def/au/asls/substrate/lithology-IG>
    a
        <http://anzsoil.org/def/au/asls/substrate/Lithology-rock> ,
        skos:Concept ;
    rdfs:isDefinedBy <http://anzsoil.org/def/au/asls/substrate> ;
    rdfs:seeAlso <http://anzsoil.org/def/au/asls/substrate> ;
    skos:definition "Igneous rock (Unidentified)"@en ;
    skos:inScheme <http://anzsoil.org/def/au/asls/substrate> ;
    skos:notation "IG" ;
    skos:note "C_LITHOLOGY" ;
    skos:prefLabel "Igneous rock"@en ;
    skos:topConceptOf <http://anzsoil.org/def/au/asls/substrate> ;
.

<http://anzsoil.org/def/au/asls/substrate/lithology-JA>
    a
        <http://anzsoil.org/def/au/asls/substrate/Lithology-rock> ,
        skos:Concept ;
    rdfs:isDefinedBy <http://anzsoil.org/def/au/asls/substrate> ;
    rdfs:seeAlso <http://anzsoil.org/def/au/asls/substrate> ;
    skos:definition "Jasper (Sedimentary rock, chemical or organic)"@en ;
    skos:inScheme <http://anzsoil.org/def/au/asls/substrate> ;
    skos:notation "JA" ;
    skos:note "C_LITHOLOGY" ;
    skos:prefLabel "Jasper"@en ;
    skos:topConceptOf <http://anzsoil.org/def/au/asls/substrate> ;
.

<http://anzsoil.org/def/au/asls/substrate/lithology-KA>
    a
        <http://anzsoil.org/def/au/asls/substrate/Lithology-rock> ,
        skos:Concept ;
    rdfs:isDefinedBy <http://anzsoil.org/def/au/asls/substrate> ;
    rdfs:seeAlso <http://anzsoil.org/def/au/asls/substrate> ;
    skos:definition "Calcarenite (Sedimentary rock, detrital)"@en ;
    skos:inScheme <http://anzsoil.org/def/au/asls/substrate> ;
    skos:notation "KA" ;
    skos:note "C_LITHOLOGY" ;
    skos:prefLabel "Calcarenite"@en ;
    skos:topConceptOf <http://anzsoil.org/def/au/asls/substrate> ;
.

<http://anzsoil.org/def/au/asls/substrate/lithology-KC>
    a
        <http://anzsoil.org/def/au/asls/substrate/Lithology-rock> ,
        skos:Concept ;
    rdfs:isDefinedBy <http://anzsoil.org/def/au/asls/substrate> ;
    rdfs:seeAlso <http://anzsoil.org/def/au/asls/substrate> ;
    skos:definition "Calcrete (Sedimentary rock, chemical or organic)"@en ;
    skos:inScheme <http://anzsoil.org/def/au/asls/substrate> ;
    skos:notation "KC" ;
    skos:note "C_LITHOLOGY" ;
    skos:prefLabel "Calcrete"@en ;
    skos:topConceptOf <http://anzsoil.org/def/au/asls/substrate> ;
.

<http://anzsoil.org/def/au/asls/substrate/lithology-KL>
    a
        <http://anzsoil.org/def/au/asls/substrate/Lithology-rock> ,
        skos:Concept ;
    rdfs:isDefinedBy <http://anzsoil.org/def/au/asls/substrate> ;
    rdfs:seeAlso <http://anzsoil.org/def/au/asls/substrate> ;
    skos:definition "Calcilutite (Sedimentary rock, detrital)"@en ;
    skos:inScheme <http://anzsoil.org/def/au/asls/substrate> ;
    skos:notation "KL" ;
    skos:note "C_LITHOLOGY" ;
    skos:prefLabel "Calcilutite"@en ;
    skos:topConceptOf <http://anzsoil.org/def/au/asls/substrate> ;
.

<http://anzsoil.org/def/au/asls/substrate/lithology-KM>
    a
        <http://anzsoil.org/def/au/asls/substrate/Lithology-rock> ,
        skos:Concept ;
    rdfs:isDefinedBy <http://anzsoil.org/def/au/asls/substrate> ;
    rdfs:seeAlso <http://anzsoil.org/def/au/asls/substrate> ;
    skos:definition "Calcareous mudstone (Sedimentary rock, detrital)"@en ;
    skos:inScheme <http://anzsoil.org/def/au/asls/substrate> ;
    skos:notation "KM" ;
    skos:note "C_LITHOLOGY" ;
    skos:prefLabel "Calcareous mudstone"@en ;
    skos:topConceptOf <http://anzsoil.org/def/au/asls/substrate> ;
.

<http://anzsoil.org/def/au/asls/substrate/lithology-KR>
    a
        <http://anzsoil.org/def/au/asls/substrate/Lithology-rock> ,
        skos:Concept ;
    rdfs:isDefinedBy <http://anzsoil.org/def/au/asls/substrate> ;
    rdfs:seeAlso <http://anzsoil.org/def/au/asls/substrate> ;
    skos:definition "Calcirudite (Sedimentary rock, detrital)"@en ;
    skos:inScheme <http://anzsoil.org/def/au/asls/substrate> ;
    skos:notation "KR" ;
    skos:note "C_LITHOLOGY" ;
    skos:prefLabel "Calcirudite"@en ;
    skos:topConceptOf <http://anzsoil.org/def/au/asls/substrate> ;
.

<http://anzsoil.org/def/au/asls/substrate/lithology-LC>
    a
        <http://anzsoil.org/def/au/asls/substrate/Lithology-rock> ,
        skos:Concept ;
    rdfs:isDefinedBy <http://anzsoil.org/def/au/asls/substrate> ;
    rdfs:seeAlso <http://anzsoil.org/def/au/asls/substrate> ;
    skos:definition "Silcrete (Sedimentary rock, chemical or organic)"@en ;
    skos:inScheme <http://anzsoil.org/def/au/asls/substrate> ;
    skos:notation "LC" ;
    skos:note "C_LITHOLOGY" ;
    skos:prefLabel "Silcrete"@en ;
    skos:topConceptOf <http://anzsoil.org/def/au/asls/substrate> ;
.

<http://anzsoil.org/def/au/asls/substrate/lithology-LI>
    a
        <http://anzsoil.org/def/au/asls/substrate/Lithology-rock> ,
        skos:Concept ;
    rdfs:isDefinedBy <http://anzsoil.org/def/au/asls/substrate> ;
    rdfs:seeAlso <http://anzsoil.org/def/au/asls/substrate> ;
    skos:definition "Limestone (Sedimentary rock, detrital)"@en ;
    skos:inScheme <http://anzsoil.org/def/au/asls/substrate> ;
    skos:notation "LI" ;
    skos:note "C_LITHOLOGY" ;
    skos:prefLabel "Limestone"@en ;
    skos:topConceptOf <http://anzsoil.org/def/au/asls/substrate> ;
.

<http://anzsoil.org/def/au/asls/substrate/lithology-M>
    a
        <http://anzsoil.org/def/au/asls/substrate/Lithology-rock> ,
        skos:Concept ;
    rdfs:isDefinedBy <http://anzsoil.org/def/au/asls/substrate> ;
    rdfs:seeAlso <http://anzsoil.org/def/au/asls/substrate> ;
    skos:definition "Lithology is same as the substrate material"@en ;
    skos:inScheme <http://anzsoil.org/def/au/asls/substrate> ;
    skos:notation "M" ;
    skos:note "C_LITHOLOGY" ;
    skos:prefLabel "Same as substrate material"@en ;
    skos:topConceptOf <http://anzsoil.org/def/au/asls/substrate> ;
.

<http://anzsoil.org/def/au/asls/substrate/lithology-MB>
    a
        <http://anzsoil.org/def/au/asls/substrate/Lithology-rock> ,
        skos:Concept ;
    rdfs:isDefinedBy <http://anzsoil.org/def/au/asls/substrate> ;
    rdfs:seeAlso <http://anzsoil.org/def/au/asls/substrate> ;
    skos:definition "Marble (Metamorphic rock)"@en ;
    skos:inScheme <http://anzsoil.org/def/au/asls/substrate> ;
    skos:notation "MB" ;
    skos:note "C_LITHOLOGY" ;
    skos:prefLabel "Marble"@en ;
    skos:topConceptOf <http://anzsoil.org/def/au/asls/substrate> ;
.

<http://anzsoil.org/def/au/asls/substrate/lithology-MD>
    a
        <http://anzsoil.org/def/au/asls/substrate/Lithology-rock> ,
        skos:Concept ;
    rdfs:isDefinedBy <http://anzsoil.org/def/au/asls/substrate> ;
    rdfs:seeAlso <http://anzsoil.org/def/au/asls/substrate> ;
    skos:definition "Microdiorite (Igneous rock)"@en ;
    skos:inScheme <http://anzsoil.org/def/au/asls/substrate> ;
    skos:notation "MD" ;
    skos:note "C_LITHOLOGY" ;
    skos:prefLabel "Microdiorite"@en ;
    skos:topConceptOf <http://anzsoil.org/def/au/asls/substrate> ;
.

<http://anzsoil.org/def/au/asls/substrate/lithology-ME>
    a
        <http://anzsoil.org/def/au/asls/substrate/Lithology-rock> ,
        skos:Concept ;
    rdfs:isDefinedBy <http://anzsoil.org/def/au/asls/substrate> ;
    rdfs:seeAlso <http://anzsoil.org/def/au/asls/substrate> ;
    skos:definition "Metamorphic rock (Unidentified)"@en ;
    skos:inScheme <http://anzsoil.org/def/au/asls/substrate> ;
    skos:notation "ME" ;
    skos:note "C_LITHOLOGY" ;
    skos:prefLabel "Metamorphic rock"@en ;
    skos:topConceptOf <http://anzsoil.org/def/au/asls/substrate> ;
.

<http://anzsoil.org/def/au/asls/substrate/lithology-MG>
    a
        <http://anzsoil.org/def/au/asls/substrate/Lithology-rock> ,
        skos:Concept ;
    rdfs:isDefinedBy <http://anzsoil.org/def/au/asls/substrate> ;
    rdfs:seeAlso <http://anzsoil.org/def/au/asls/substrate> ;
    skos:definition "Microgranite (Igneous rock)"@en ;
    skos:inScheme <http://anzsoil.org/def/au/asls/substrate> ;
    skos:notation "MG" ;
    skos:note "C_LITHOLOGY" ;
    skos:prefLabel "Microgranite"@en ;
    skos:topConceptOf <http://anzsoil.org/def/au/asls/substrate> ;
.

<http://anzsoil.org/def/au/asls/substrate/lithology-MI>
    a
        <http://anzsoil.org/def/au/asls/substrate/Lithology-rock> ,
        skos:Concept ;
    rdfs:isDefinedBy <http://anzsoil.org/def/au/asls/substrate> ;
    rdfs:seeAlso <http://anzsoil.org/def/au/asls/substrate> ;
    skos:definition "Migmatite (Metamorphic rock)"@en ;
    skos:inScheme <http://anzsoil.org/def/au/asls/substrate> ;
    skos:notation "MI" ;
    skos:note "C_LITHOLOGY" ;
    skos:prefLabel "Migmatite"@en ;
    skos:topConceptOf <http://anzsoil.org/def/au/asls/substrate> ;
.

<http://anzsoil.org/def/au/asls/substrate/lithology-MS>
    a
        <http://anzsoil.org/def/au/asls/substrate/Lithology-rock> ,
        skos:Concept ;
    rdfs:isDefinedBy <http://anzsoil.org/def/au/asls/substrate> ;
    rdfs:seeAlso <http://anzsoil.org/def/au/asls/substrate> ;
    skos:definition "Microsyenite (Igneous rock)"@en ;
    skos:inScheme <http://anzsoil.org/def/au/asls/substrate> ;
    skos:notation "MS" ;
    skos:note "C_LITHOLOGY" ;
    skos:prefLabel "Microsyenite"@en ;
    skos:topConceptOf <http://anzsoil.org/def/au/asls/substrate> ;
.

<http://anzsoil.org/def/au/asls/substrate/lithology-MU>
    a
        <http://anzsoil.org/def/au/asls/substrate/Lithology-rock> ,
        skos:Concept ;
    rdfs:isDefinedBy <http://anzsoil.org/def/au/asls/substrate> ;
    rdfs:seeAlso <http://anzsoil.org/def/au/asls/substrate> ;
    skos:definition "Mudstone (Sedimentary rock, detrital)"@en ;
    skos:inScheme <http://anzsoil.org/def/au/asls/substrate> ;
    skos:notation "MU" ;
    skos:note "C_LITHOLOGY" ;
    skos:prefLabel "Mudstone"@en ;
    skos:topConceptOf <http://anzsoil.org/def/au/asls/substrate> ;
.

<http://anzsoil.org/def/au/asls/substrate/lithology-MY>
    a
        <http://anzsoil.org/def/au/asls/substrate/Lithology-rock> ,
        skos:Concept ;
    rdfs:isDefinedBy <http://anzsoil.org/def/au/asls/substrate> ;
    rdfs:seeAlso <http://anzsoil.org/def/au/asls/substrate> ;
    skos:definition "Mylonite (Metamorphic rock)"@en ;
    skos:inScheme <http://anzsoil.org/def/au/asls/substrate> ;
    skos:notation "MY" ;
    skos:note "C_LITHOLOGY" ;
    skos:prefLabel "Mylonite"@en ;
    skos:topConceptOf <http://anzsoil.org/def/au/asls/substrate> ;
.

<http://anzsoil.org/def/au/asls/substrate/lithology-PC>
    a
        <http://anzsoil.org/def/au/asls/substrate/Lithology-rock> ,
        skos:Concept ;
    rdfs:isDefinedBy <http://anzsoil.org/def/au/asls/substrate> ;
    rdfs:seeAlso <http://anzsoil.org/def/au/asls/substrate> ;
    skos:definition "Porcellanite (Sedimentary rock, chemical or organic)"@en ;
    skos:inScheme <http://anzsoil.org/def/au/asls/substrate> ;
    skos:notation "PC" ;
    skos:note "C_LITHOLOGY" ;
    skos:prefLabel "Porcellanite"@en ;
    skos:topConceptOf <http://anzsoil.org/def/au/asls/substrate> ;
.

<http://anzsoil.org/def/au/asls/substrate/lithology-PE>
    a
        <http://anzsoil.org/def/au/asls/substrate/Lithology-rock> ,
        skos:Concept ;
    rdfs:isDefinedBy <http://anzsoil.org/def/au/asls/substrate> ;
    rdfs:seeAlso <http://anzsoil.org/def/au/asls/substrate> ;
    skos:definition "Peridotite (Igneous rock)"@en ;
    skos:inScheme <http://anzsoil.org/def/au/asls/substrate> ;
    skos:notation "PE" ;
    skos:note "C_LITHOLOGY" ;
    skos:prefLabel "Peridotite"@en ;
    skos:topConceptOf <http://anzsoil.org/def/au/asls/substrate> ;
.

<http://anzsoil.org/def/au/asls/substrate/lithology-PG>
    a
        <http://anzsoil.org/def/au/asls/substrate/Lithology-rock> ,
        skos:Concept ;
    rdfs:isDefinedBy <http://anzsoil.org/def/au/asls/substrate> ;
    rdfs:seeAlso <http://anzsoil.org/def/au/asls/substrate> ;
    skos:definition "Pegmatite (Igneous rock)"@en ;
    skos:inScheme <http://anzsoil.org/def/au/asls/substrate> ;
    skos:notation "PG" ;
    skos:note "C_LITHOLOGY" ;
    skos:prefLabel "Pegmatite"@en ;
    skos:topConceptOf <http://anzsoil.org/def/au/asls/substrate> ;
.

<http://anzsoil.org/def/au/asls/substrate/lithology-PH>
    a
        <http://anzsoil.org/def/au/asls/substrate/Lithology-rock> ,
        skos:Concept ;
    rdfs:isDefinedBy <http://anzsoil.org/def/au/asls/substrate> ;
    rdfs:seeAlso <http://anzsoil.org/def/au/asls/substrate> ;
    skos:definition "Phyllite (Metamorphic rock)"@en ;
    skos:inScheme <http://anzsoil.org/def/au/asls/substrate> ;
    skos:notation "PH" ;
    skos:note "C_LITHOLOGY" ;
    skos:prefLabel "Phyllite"@en ;
    skos:topConceptOf <http://anzsoil.org/def/au/asls/substrate> ;
.

<http://anzsoil.org/def/au/asls/substrate/lithology-PL>
    a
        <http://anzsoil.org/def/au/asls/substrate/Lithology-rock> ,
        skos:Concept ;
    rdfs:isDefinedBy <http://anzsoil.org/def/au/asls/substrate> ;
    rdfs:seeAlso <http://anzsoil.org/def/au/asls/substrate> ;
    skos:definition "Phonolite (Igneous rock)"@en ;
    skos:inScheme <http://anzsoil.org/def/au/asls/substrate> ;
    skos:notation "PL" ;
    skos:note "C_LITHOLOGY" ;
    skos:prefLabel "Phonolite"@en ;
    skos:topConceptOf <http://anzsoil.org/def/au/asls/substrate> ;
.

<http://anzsoil.org/def/au/asls/substrate/lithology-PO>
    a
        <http://anzsoil.org/def/au/asls/substrate/Lithology-rock> ,
        skos:Concept ;
    rdfs:isDefinedBy <http://anzsoil.org/def/au/asls/substrate> ;
    rdfs:seeAlso <http://anzsoil.org/def/au/asls/substrate> ;
    skos:definition "Porphyry (Igneous rock)"@en ;
    skos:inScheme <http://anzsoil.org/def/au/asls/substrate> ;
    skos:notation "PO" ;
    skos:note "C_LITHOLOGY" ;
    skos:prefLabel "Porphyry"@en ;
    skos:topConceptOf <http://anzsoil.org/def/au/asls/substrate> ;
.

<http://anzsoil.org/def/au/asls/substrate/lithology-PY>
    a
        <http://anzsoil.org/def/au/asls/substrate/Lithology-rock> ,
        skos:Concept ;
    rdfs:isDefinedBy <http://anzsoil.org/def/au/asls/substrate> ;
    rdfs:seeAlso <http://anzsoil.org/def/au/asls/substrate> ;
    skos:definition "Pyroxenite (Igneous rock)"@en ;
    skos:inScheme <http://anzsoil.org/def/au/asls/substrate> ;
    skos:notation "PY" ;
    skos:note "C_LITHOLOGY" ;
    skos:prefLabel "Pyroxenite"@en ;
    skos:topConceptOf <http://anzsoil.org/def/au/asls/substrate> ;
.

<http://anzsoil.org/def/au/asls/substrate/lithology-QP>
    a
        <http://anzsoil.org/def/au/asls/substrate/Lithology-rock> ,
        skos:Concept ;
    rdfs:isDefinedBy <http://anzsoil.org/def/au/asls/substrate> ;
    rdfs:seeAlso <http://anzsoil.org/def/au/asls/substrate> ;
    skos:definition "Quartz porphyry (Igneous rock)"@en ;
    skos:inScheme <http://anzsoil.org/def/au/asls/substrate> ;
    skos:notation "QP" ;
    skos:note "C_LITHOLOGY" ;
    skos:prefLabel "Quartz porphyry"@en ;
    skos:topConceptOf <http://anzsoil.org/def/au/asls/substrate> ;
.

<http://anzsoil.org/def/au/asls/substrate/lithology-QS>
    a
        <http://anzsoil.org/def/au/asls/substrate/Lithology-rock> ,
        skos:Concept ;
    rdfs:isDefinedBy <http://anzsoil.org/def/au/asls/substrate> ;
    rdfs:seeAlso <http://anzsoil.org/def/au/asls/substrate> ;
    skos:definition "Quartz sandstone (Sedimentary rock, detrital)"@en ;
    skos:inScheme <http://anzsoil.org/def/au/asls/substrate> ;
    skos:notation "QS" ;
    skos:note "C_LITHOLOGY" ;
    skos:prefLabel "Quartz sandstone"@en ;
    skos:topConceptOf <http://anzsoil.org/def/au/asls/substrate> ;
.

<http://anzsoil.org/def/au/asls/substrate/lithology-QU>
    a
        <http://anzsoil.org/def/au/asls/substrate/Lithology-rock> ,
        skos:Concept ;
    rdfs:isDefinedBy <http://anzsoil.org/def/au/asls/substrate> ;
    rdfs:seeAlso <http://anzsoil.org/def/au/asls/substrate> ;
    skos:definition "Quartzite (Metamorphic rock)"@en ;
    skos:inScheme <http://anzsoil.org/def/au/asls/substrate> ;
    skos:notation "QU" ;
    skos:note "C_LITHOLOGY" ;
    skos:prefLabel "Quartzite"@en ;
    skos:topConceptOf <http://anzsoil.org/def/au/asls/substrate> ;
.

<http://anzsoil.org/def/au/asls/substrate/lithology-QZ>
    a
        <http://anzsoil.org/def/au/asls/substrate/Lithology-rock> ,
        skos:Concept ;
    rdfs:isDefinedBy <http://anzsoil.org/def/au/asls/substrate> ;
    rdfs:seeAlso <http://anzsoil.org/def/au/asls/substrate> ;
    skos:definition "Quartz (Igneous rock)"@en ;
    skos:inScheme <http://anzsoil.org/def/au/asls/substrate> ;
    skos:notation "QZ" ;
    skos:note "C_LITHOLOGY" ;
    skos:prefLabel "Quartz"@en ;
    skos:topConceptOf <http://anzsoil.org/def/au/asls/substrate> ;
.

<http://anzsoil.org/def/au/asls/substrate/lithology-R>
    a
        <http://anzsoil.org/def/au/asls/substrate/Lithology-rock> ,
        skos:Concept ;
    rdfs:isDefinedBy <http://anzsoil.org/def/au/asls/substrate> ;
    rdfs:seeAlso <http://anzsoil.org/def/au/asls/substrate> ;
    skos:definition "Lithology is same as the rock outcrop"@en ;
    skos:inScheme <http://anzsoil.org/def/au/asls/substrate> ;
    skos:notation "R" ;
    skos:note "C_LITHOLOGY" ;
    skos:prefLabel "Same as rock outcrop"@en ;
    skos:topConceptOf <http://anzsoil.org/def/au/asls/substrate> ;
.

<http://anzsoil.org/def/au/asls/substrate/lithology-RB>
    a
        <http://anzsoil.org/def/au/asls/substrate/Lithology-rock> ,
        skos:Concept ;
    rdfs:isDefinedBy <http://anzsoil.org/def/au/asls/substrate> ;
    rdfs:seeAlso <http://anzsoil.org/def/au/asls/substrate> ;
    skos:definition "Red-brown hardpan (Sedimentary rock, chemical or organic)"@en ;
    skos:inScheme <http://anzsoil.org/def/au/asls/substrate> ;
    skos:notation "RB" ;
    skos:note "C_LITHOLOGY" ;
    skos:prefLabel "Red-brown hardpan"@en ;
    skos:topConceptOf <http://anzsoil.org/def/au/asls/substrate> ;
.

<http://anzsoil.org/def/au/asls/substrate/lithology-RH>
    a
        <http://anzsoil.org/def/au/asls/substrate/Lithology-rock> ,
        skos:Concept ;
    rdfs:isDefinedBy <http://anzsoil.org/def/au/asls/substrate> ;
    rdfs:seeAlso <http://anzsoil.org/def/au/asls/substrate> ;
    skos:definition "Rhyolite (Igneous rock)"@en ;
    skos:inScheme <http://anzsoil.org/def/au/asls/substrate> ;
    skos:notation "RH" ;
    skos:note "C_LITHOLOGY" ;
    skos:prefLabel "Rhyolite"@en ;
    skos:topConceptOf <http://anzsoil.org/def/au/asls/substrate> ;
.

<http://anzsoil.org/def/au/asls/substrate/lithology-SA>
    a
        <http://anzsoil.org/def/au/asls/substrate/Lithology-rock> ,
        skos:Concept ;
    rdfs:isDefinedBy <http://anzsoil.org/def/au/asls/substrate> ;
    rdfs:seeAlso <http://anzsoil.org/def/au/asls/substrate> ;
    skos:definition "Sandstone (Sedimentary rock, detrital)"@en ;
    skos:inScheme <http://anzsoil.org/def/au/asls/substrate> ;
    skos:notation "SA" ;
    skos:note "C_LITHOLOGY" ;
    skos:prefLabel "Sandstone"@en ;
    skos:topConceptOf <http://anzsoil.org/def/au/asls/substrate> ;
.

<http://anzsoil.org/def/au/asls/substrate/lithology-SD>
    a
        <http://anzsoil.org/def/au/asls/substrate/Lithology-rock> ,
        skos:Concept ;
    rdfs:isDefinedBy <http://anzsoil.org/def/au/asls/substrate> ;
    rdfs:seeAlso <http://anzsoil.org/def/au/asls/substrate> ;
    skos:definition "Detrital sedimentary rock (Unidentified)"@en ;
    skos:inScheme <http://anzsoil.org/def/au/asls/substrate> ;
    skos:notation "SD" ;
    skos:note "C_LITHOLOGY" ;
    skos:prefLabel "Detrital sedimentary rock"@en ;
    skos:topConceptOf <http://anzsoil.org/def/au/asls/substrate> ;
.

<http://anzsoil.org/def/au/asls/substrate/lithology-SH>
    a
        <http://anzsoil.org/def/au/asls/substrate/Lithology-rock> ,
        skos:Concept ;
    rdfs:isDefinedBy <http://anzsoil.org/def/au/asls/substrate> ;
    rdfs:seeAlso <http://anzsoil.org/def/au/asls/substrate> ;
    skos:definition "Shale (Igneous rock)"@en ;
    skos:inScheme <http://anzsoil.org/def/au/asls/substrate> ;
    skos:notation "SH" ;
    skos:note "C_LITHOLOGY" ;
    skos:prefLabel "Shale"@en ;
    skos:topConceptOf <http://anzsoil.org/def/au/asls/substrate> ;
.

<http://anzsoil.org/def/au/asls/substrate/lithology-SL>
    a
        <http://anzsoil.org/def/au/asls/substrate/Lithology-rock> ,
        skos:Concept ;
    rdfs:isDefinedBy <http://anzsoil.org/def/au/asls/substrate> ;
    rdfs:seeAlso <http://anzsoil.org/def/au/asls/substrate> ;
    skos:definition "Slate (Sedimentary rock, detrital)"@en ;
    skos:inScheme <http://anzsoil.org/def/au/asls/substrate> ;
    skos:notation "SL" ;
    skos:note "C_LITHOLOGY" ;
    skos:prefLabel "Slate"@en ;
    skos:topConceptOf <http://anzsoil.org/def/au/asls/substrate> ;
.

<http://anzsoil.org/def/au/asls/substrate/lithology-SN>
    a
        <http://anzsoil.org/def/au/asls/substrate/Lithology-unconsolidated> ,
        skos:Concept ;
    dcterms:identifier "http://anzsoil.org/def/au/asls/substrate/lithology-SN" ;
    rdfs:isDefinedBy <http://anzsoil.org/def/au/asls/substrate> ;
    rdfs:seeAlso <http://anzsoil.org/def/au/asls/substrate> ;
    skos:definition """Very coarse grained
>60 mm
Non-volcanic
Without significant carbonate""" ;
    skos:inScheme <http://anzsoil.org/def/au/asls/substrate> ;
    skos:notation "SN" ;
    skos:prefLabel "Stones"@en ;
    skos:topConceptOf <http://anzsoil.org/def/au/asls/substrate> ;
.

<http://anzsoil.org/def/au/asls/substrate/lithology-SR>
    a
        <http://anzsoil.org/def/au/asls/substrate/Lithology-rock> ,
        skos:Concept ;
    rdfs:isDefinedBy <http://anzsoil.org/def/au/asls/substrate> ;
    rdfs:seeAlso <http://anzsoil.org/def/au/asls/substrate> ;
    skos:definition "Serpentinite (Igneous rock)"@en ;
    skos:inScheme <http://anzsoil.org/def/au/asls/substrate> ;
    skos:notation "SR" ;
    skos:note "C_LITHOLOGY" ;
    skos:prefLabel "Serpentinite"@en ;
    skos:topConceptOf <http://anzsoil.org/def/au/asls/substrate> ;
.

<http://anzsoil.org/def/au/asls/substrate/lithology-ST>
    a
        <http://anzsoil.org/def/au/asls/substrate/Lithology-rock> ,
        skos:Concept ;
    rdfs:isDefinedBy <http://anzsoil.org/def/au/asls/substrate> ;
    rdfs:seeAlso <http://anzsoil.org/def/au/asls/substrate> ;
    skos:definition "Schist (Metamorphic rock)"@en ;
    skos:inScheme <http://anzsoil.org/def/au/asls/substrate> ;
    skos:notation "ST" ;
    skos:note "C_LITHOLOGY" ;
    skos:prefLabel "Schist"@en ;
    skos:topConceptOf <http://anzsoil.org/def/au/asls/substrate> ;
.

<http://anzsoil.org/def/au/asls/substrate/lithology-SY>
    a
        <http://anzsoil.org/def/au/asls/substrate/Lithology-rock> ,
        skos:Concept ;
    rdfs:isDefinedBy <http://anzsoil.org/def/au/asls/substrate> ;
    rdfs:seeAlso <http://anzsoil.org/def/au/asls/substrate> ;
    skos:definition "Syenite (Metamorphic rock)"@en ;
    skos:inScheme <http://anzsoil.org/def/au/asls/substrate> ;
    skos:notation "SY" ;
    skos:note "C_LITHOLOGY" ;
    skos:prefLabel "Syenite"@en ;
    skos:topConceptOf <http://anzsoil.org/def/au/asls/substrate> ;
.

<http://anzsoil.org/def/au/asls/substrate/lithology-TR>
    a
        <http://anzsoil.org/def/au/asls/substrate/Lithology-rock> ,
        skos:Concept ;
    rdfs:isDefinedBy <http://anzsoil.org/def/au/asls/substrate> ;
    rdfs:seeAlso <http://anzsoil.org/def/au/asls/substrate> ;
    skos:definition "Trachyte (Igneous rock)"@en ;
    skos:inScheme <http://anzsoil.org/def/au/asls/substrate> ;
    skos:notation "TR" ;
    skos:note "C_LITHOLOGY" ;
    skos:prefLabel "Trachyte"@en ;
    skos:topConceptOf <http://anzsoil.org/def/au/asls/substrate> ;
.

<http://anzsoil.org/def/au/asls/substrate/lithology-TU>
    a
        <http://anzsoil.org/def/au/asls/substrate/Lithology-rock> ,
        skos:Concept ;
    rdfs:isDefinedBy <http://anzsoil.org/def/au/asls/substrate> ;
    rdfs:seeAlso <http://anzsoil.org/def/au/asls/substrate> ;
    skos:definition "Tuff (Igneous rock)"@en ;
    skos:inScheme <http://anzsoil.org/def/au/asls/substrate> ;
    skos:notation "TU" ;
    skos:note "C_LITHOLOGY" ;
    skos:prefLabel "Tuff"@en ;
    skos:topConceptOf <http://anzsoil.org/def/au/asls/substrate> ;
.

<http://anzsoil.org/def/au/asls/substrate/lithology-UC>
    a
        <http://anzsoil.org/def/au/asls/substrate/Lithology-rock> ,
        skos:Concept ;
    rdfs:isDefinedBy <http://anzsoil.org/def/au/asls/substrate> ;
    rdfs:seeAlso <http://anzsoil.org/def/au/asls/substrate> ;
    skos:definition "Unconsolidated material (Unidentified)"@en ;
    skos:inScheme <http://anzsoil.org/def/au/asls/substrate> ;
    skos:notation "UC" ;
    skos:note "C_LITHOLOGY" ;
    skos:prefLabel "Unconsolidated material"@en ;
    skos:topConceptOf <http://anzsoil.org/def/au/asls/substrate> ;
.

<http://anzsoil.org/def/au/asls/substrate/lithology-VB>
    a
        <http://anzsoil.org/def/au/asls/substrate/Lithology-rock> ,
        skos:Concept ;
    rdfs:isDefinedBy <http://anzsoil.org/def/au/asls/substrate> ;
    rdfs:seeAlso <http://anzsoil.org/def/au/asls/substrate> ;
    skos:definition "Volcanic breccia (Sedimentary rock, pyroclastic)"@en ;
    skos:inScheme <http://anzsoil.org/def/au/asls/substrate> ;
    skos:notation "VB" ;
    skos:note "C_LITHOLOGY" ;
    skos:prefLabel "Volcanic breccia"@en ;
    skos:topConceptOf <http://anzsoil.org/def/au/asls/substrate> ;
.

<http://anzsoil.org/def/au/asls/substrate/lithology-VG>
    a
        <http://anzsoil.org/def/au/asls/substrate/Lithology-rock> ,
        skos:Concept ;
    rdfs:isDefinedBy <http://anzsoil.org/def/au/asls/substrate> ;
    rdfs:seeAlso <http://anzsoil.org/def/au/asls/substrate> ;
    skos:definition "Volcanic glass (Igneous rock)"@en ;
    skos:inScheme <http://anzsoil.org/def/au/asls/substrate> ;
    skos:notation "VG" ;
    skos:note "C_LITHOLOGY" ;
    skos:prefLabel "Volcanic glass"@en ;
    skos:topConceptOf <http://anzsoil.org/def/au/asls/substrate> ;
.

<http://anzsoil.org/def/au/asls/substrate/lithology-ZS>
    a
        <http://anzsoil.org/def/au/asls/substrate/Lithology-rock> ,
        skos:Concept ;
    rdfs:isDefinedBy <http://anzsoil.org/def/au/asls/substrate> ;
    rdfs:seeAlso <http://anzsoil.org/def/au/asls/substrate> ;
    skos:definition "Siltstone (Unconsolidated material)"@en ;
    skos:inScheme <http://anzsoil.org/def/au/asls/substrate> ;
    skos:notation "ZS" ;
    skos:note "C_LITHOLOGY" ;
    skos:prefLabel "Siltstone"@en ;
    skos:topConceptOf <http://anzsoil.org/def/au/asls/substrate> ;
.

<http://anzsoil.org/def/au/asls/substrate/material-strength-M>
    a
        <http://anzsoil.org/def/au/asls/substrate/Material-strength> ,
        skos:Concept ;
    rdfs:isDefinedBy <http://anzsoil.org/def/au/asls/substrate> ;
    rdfs:seeAlso <http://anzsoil.org/def/au/asls/substrate> ;
    skos:definition "50-100 MPa based on field estimate of strength class after striking or cutting the rock material - Knife:Nil or slight mark, Pick:indents shallowly, Hammer (single blow):Breaks readily into a few large and some small fragments"@en ;
    skos:inScheme <http://anzsoil.org/def/au/asls/substrate> ;
    skos:notation "M" ;
    skos:prefLabel "Moderately strong rock"@en ;
    skos:topConceptOf <http://anzsoil.org/def/au/asls/substrate> ;
.

<http://anzsoil.org/def/au/asls/substrate/material-strength-S>
    a
        <http://anzsoil.org/def/au/asls/substrate/Material-strength> ,
        skos:Concept ;
    rdfs:isDefinedBy <http://anzsoil.org/def/au/asls/substrate> ;
    rdfs:seeAlso <http://anzsoil.org/def/au/asls/substrate> ;
    skos:definition "100-200 MPa based on field estimate of strength class after striking or cutting the rock material - Knife:Nil, Pick:Nil, Hammer (single blow):Breaks into one or two large fragments"@en ;
    skos:inScheme <http://anzsoil.org/def/au/asls/substrate> ;
    skos:notation "S" ;
    skos:prefLabel "Strong rock"@en ;
    skos:topConceptOf <http://anzsoil.org/def/au/asls/substrate> ;
.

<http://anzsoil.org/def/au/asls/substrate/material-strength-VS>
    a
        <http://anzsoil.org/def/au/asls/substrate/Material-strength> ,
        skos:Concept ;
    rdfs:isDefinedBy <http://anzsoil.org/def/au/asls/substrate> ;
    rdfs:seeAlso <http://anzsoil.org/def/au/asls/substrate> ;
    skos:definition ">200 MPa based on field estimate of strength class after striking or cutting the rock material - Knife:Nil, Pick:Nil, Hammer (single blow):Nil"@en ;
    skos:inScheme <http://anzsoil.org/def/au/asls/substrate> ;
    skos:notation "VS" ;
    skos:prefLabel "Very strong rock"@en ;
    skos:topConceptOf <http://anzsoil.org/def/au/asls/substrate> ;
.

<http://anzsoil.org/def/au/asls/substrate/material-strength-VW>
    a
        <http://anzsoil.org/def/au/asls/substrate/Material-strength> ,
        skos:Concept ;
    rdfs:isDefinedBy <http://anzsoil.org/def/au/asls/substrate> ;
    rdfs:seeAlso <http://anzsoil.org/def/au/asls/substrate> ;
    skos:definition "1-25 MPa based on field estimate of strength class after striking or cutting the rock material - Knife:Deep cut, Pick:crumbles, Hammer (single blow):Flattened or powdered"@en ;
    skos:inScheme <http://anzsoil.org/def/au/asls/substrate> ;
    skos:notation "VW" ;
    skos:prefLabel "Very weak rock"@en ;
    skos:topConceptOf <http://anzsoil.org/def/au/asls/substrate> ;
.

<http://anzsoil.org/def/au/asls/substrate/material-strength-W>
    a
        <http://anzsoil.org/def/au/asls/substrate/Material-strength> ,
        skos:Concept ;
    rdfs:isDefinedBy <http://anzsoil.org/def/au/asls/substrate> ;
    rdfs:seeAlso <http://anzsoil.org/def/au/asls/substrate> ;
    skos:definition "25-50 MPa based on field estimate of strength class after striking or cutting the rock material - Knife:Shallow cut or scratch, Pick:indents deeply, Hammer (single blow):Shattered into many small fragments"@en ;
    skos:inScheme <http://anzsoil.org/def/au/asls/substrate> ;
    skos:notation "W" ;
    skos:prefLabel "Weak rock"@en ;
    skos:topConceptOf <http://anzsoil.org/def/au/asls/substrate> ;
.

<http://anzsoil.org/def/au/asls/substrate/material-structure-B>
    a
        <http://anzsoil.org/def/au/asls/substrate/Substrate-structure> ,
        skos:Concept ;
    rdfs:isDefinedBy <http://anzsoil.org/def/au/asls/substrate> ;
    rdfs:seeAlso <http://anzsoil.org/def/au/asls/substrate> ;
    skos:definition "with planar surfaces marking successively deposited layers." ;
    skos:inScheme <http://anzsoil.org/def/au/asls/substrate> ;
    skos:notation "B" ;
    skos:prefLabel "Bedded"@en ;
    skos:topConceptOf <http://anzsoil.org/def/au/asls/substrate> ;
.

<http://anzsoil.org/def/au/asls/substrate/material-structure-C>
    a
        <http://anzsoil.org/def/au/asls/substrate/Substrate-structure> ,
        skos:Concept ;
    rdfs:isDefinedBy <http://anzsoil.org/def/au/asls/substrate> ;
    rdfs:seeAlso <http://anzsoil.org/def/au/asls/substrate> ;
    skos:definition "spheroidal concretions cemented together." ;
    skos:inScheme <http://anzsoil.org/def/au/asls/substrate> ;
    skos:notation "C" ;
    skos:prefLabel "Concretionary"@en ;
    skos:topConceptOf <http://anzsoil.org/def/au/asls/substrate> ;
.

<http://anzsoil.org/def/au/asls/substrate/material-structure-F>
    a
        <http://anzsoil.org/def/au/asls/substrate/Substrate-structure> ,
        skos:Concept ;
    rdfs:isDefinedBy <http://anzsoil.org/def/au/asls/substrate> ;
    rdfs:seeAlso <http://anzsoil.org/def/au/asls/substrate> ;
    skos:definition "easily split along closely spaced parallel planes." ;
    skos:inScheme <http://anzsoil.org/def/au/asls/substrate> ;
    skos:notation "F" ;
    skos:prefLabel "Fissile"@en ;
    skos:topConceptOf <http://anzsoil.org/def/au/asls/substrate> ;
.

<http://anzsoil.org/def/au/asls/substrate/material-structure-L>
    a
        <http://anzsoil.org/def/au/asls/substrate/Substrate-structure> ,
        skos:Concept ;
    rdfs:isDefinedBy <http://anzsoil.org/def/au/asls/substrate> ;
    rdfs:seeAlso <http://anzsoil.org/def/au/asls/substrate> ;
    skos:definition "planar arrangement of textural or structural textures." ;
    skos:inScheme <http://anzsoil.org/def/au/asls/substrate> ;
    skos:notation "L" ;
    skos:prefLabel "Foliated"@en ;
    skos:topConceptOf <http://anzsoil.org/def/au/asls/substrate> ;
.

<http://anzsoil.org/def/au/asls/substrate/material-structure-P>
    a
        <http://anzsoil.org/def/au/asls/substrate/Substrate-structure> ,
        skos:Concept ;
    rdfs:isDefinedBy <http://anzsoil.org/def/au/asls/substrate> ;
    rdfs:seeAlso <http://anzsoil.org/def/au/asls/substrate> ;
    skos:definition "plate-like units cemented together." ;
    skos:inScheme <http://anzsoil.org/def/au/asls/substrate> ;
    skos:notation "P" ;
    skos:prefLabel "Platy"@en ;
    skos:topConceptOf <http://anzsoil.org/def/au/asls/substrate> ;
.

<http://anzsoil.org/def/au/asls/substrate/material-structure-R>
    a
        <http://anzsoil.org/def/au/asls/substrate/Substrate-structure> ,
        skos:Concept ;
    rdfs:isDefinedBy <http://anzsoil.org/def/au/asls/substrate> ;
    rdfs:seeAlso <http://anzsoil.org/def/au/asls/substrate> ;
    skos:definition "worm-like structure and/or cavities." ;
    skos:inScheme <http://anzsoil.org/def/au/asls/substrate> ;
    skos:notation "R" ;
    skos:prefLabel "Vermicular"@en ;
    skos:topConceptOf <http://anzsoil.org/def/au/asls/substrate> ;
.

<http://anzsoil.org/def/au/asls/substrate/material-structure-S>
    a
        <http://anzsoil.org/def/au/asls/substrate/Substrate-structure> ,
        skos:Concept ;
    rdfs:isDefinedBy <http://anzsoil.org/def/au/asls/substrate> ;
    rdfs:seeAlso <http://anzsoil.org/def/au/asls/substrate> ;
    skos:definition "sponge-like structure having large pores, which may or may not be filled with softer material." ;
    skos:inScheme <http://anzsoil.org/def/au/asls/substrate> ;
    skos:notation "S" ;
    skos:prefLabel "Vesicular"@en ;
    skos:topConceptOf <http://anzsoil.org/def/au/asls/substrate> ;
.

<http://anzsoil.org/def/au/asls/substrate/material-structure-V>
    a
        <http://anzsoil.org/def/au/asls/substrate/Substrate-structure> ,
        skos:Concept ;
    rdfs:isDefinedBy <http://anzsoil.org/def/au/asls/substrate> ;
    rdfs:seeAlso <http://anzsoil.org/def/au/asls/substrate> ;
    skos:definition "no recognisable structure" ;
    skos:inScheme <http://anzsoil.org/def/au/asls/substrate> ;
    skos:notation "V" ;
    skos:prefLabel "Massive"@en ;
    skos:topConceptOf <http://anzsoil.org/def/au/asls/substrate> ;
.

<http://anzsoil.org/def/au/asls/substrate/mineral-composition-C>
    a
        <http://anzsoil.org/def/au/asls/substrate/Substrate-mineral-composition> ,
        skos:Concept ;
    dcterms:identifier "http://anzsoil.org/def/au/asls/substrate/mineral-composition-C" ;
    rdfs:isDefinedBy <http://anzsoil.org/def/au/asls/substrate> ;
    rdfs:seeAlso <http://anzsoil.org/def/au/asls/substrate> ;
    skos:definition "Carbonaceous material"@en ;
    skos:inScheme <http://anzsoil.org/def/au/asls/substrate> ;
    skos:notation "C" ;
    skos:prefLabel "Carbonaceous material"@en ;
    skos:topConceptOf <http://anzsoil.org/def/au/asls/substrate> ;
.

<http://anzsoil.org/def/au/asls/substrate/mineral-composition-D>
    a
        <http://anzsoil.org/def/au/asls/substrate/Substrate-mineral-composition> ,
        skos:Concept ;
    dcterms:identifier "http://anzsoil.org/def/au/asls/substrate/mineral-composition-D" ;
    rdfs:isDefinedBy <http://anzsoil.org/def/au/asls/substrate> ;
    rdfs:seeAlso <http://anzsoil.org/def/au/asls/substrate> ;
    skos:definition "Dark minerals"@en ;
    skos:inScheme <http://anzsoil.org/def/au/asls/substrate> ;
    skos:notation "D" ;
    skos:prefLabel "Dark minerals"@en ;
    skos:topConceptOf <http://anzsoil.org/def/au/asls/substrate> ;
.

<http://anzsoil.org/def/au/asls/substrate/mineral-composition-F>
    a
        <http://anzsoil.org/def/au/asls/substrate/Substrate-mineral-composition> ,
        skos:Concept ;
    dcterms:identifier "http://anzsoil.org/def/au/asls/substrate/mineral-composition-F" ;
    rdfs:isDefinedBy <http://anzsoil.org/def/au/asls/substrate> ;
    rdfs:seeAlso <http://anzsoil.org/def/au/asls/substrate> ;
    skos:definition "Feldspar"@en ;
    skos:inScheme <http://anzsoil.org/def/au/asls/substrate> ;
    skos:notation "F" ;
    skos:prefLabel "Feldspar"@en ;
    skos:topConceptOf <http://anzsoil.org/def/au/asls/substrate> ;
.

<http://anzsoil.org/def/au/asls/substrate/mineral-composition-G>
    a
        <http://anzsoil.org/def/au/asls/substrate/Substrate-mineral-composition> ,
        skos:Concept ;
    dcterms:identifier "http://anzsoil.org/def/au/asls/substrate/mineral-composition-G" ;
    rdfs:isDefinedBy <http://anzsoil.org/def/au/asls/substrate> ;
    rdfs:seeAlso <http://anzsoil.org/def/au/asls/substrate> ;
    skos:definition "Glauconite"@en ;
    skos:inScheme <http://anzsoil.org/def/au/asls/substrate> ;
    skos:notation "G" ;
    skos:prefLabel "Glauconite"@en ;
    skos:topConceptOf <http://anzsoil.org/def/au/asls/substrate> ;
.

<http://anzsoil.org/def/au/asls/substrate/mineral-composition-K>
    a
        <http://anzsoil.org/def/au/asls/substrate/Substrate-mineral-composition> ,
        skos:Concept ;
    dcterms:identifier "http://anzsoil.org/def/au/asls/substrate/mineral-composition-K" ;
    rdfs:isDefinedBy <http://anzsoil.org/def/au/asls/substrate> ;
    rdfs:seeAlso <http://anzsoil.org/def/au/asls/substrate> ;
    skos:definition "Carbonates (react with 1-molar HCl)"@en ;
    skos:inScheme <http://anzsoil.org/def/au/asls/substrate> ;
    skos:notation "K" ;
    skos:prefLabel "Carbonates (react with 1-molar HCl)"@en ;
    skos:topConceptOf <http://anzsoil.org/def/au/asls/substrate> ;
.

<http://anzsoil.org/def/au/asls/substrate/mineral-composition-L>
    a
        <http://anzsoil.org/def/au/asls/substrate/Substrate-mineral-composition> ,
        skos:Concept ;
    dcterms:identifier "http://anzsoil.org/def/au/asls/substrate/mineral-composition-L" ;
    rdfs:isDefinedBy <http://anzsoil.org/def/au/asls/substrate> ;
    rdfs:seeAlso <http://anzsoil.org/def/au/asls/substrate> ;
    skos:definition "Clays (argillaceous)"@en ;
    skos:inScheme <http://anzsoil.org/def/au/asls/substrate> ;
    skos:notation "L" ;
    skos:prefLabel "Clays (argillaceous)"@en ;
    skos:topConceptOf <http://anzsoil.org/def/au/asls/substrate> ;
.

<http://anzsoil.org/def/au/asls/substrate/mineral-composition-M>
    a
        <http://anzsoil.org/def/au/asls/substrate/Substrate-mineral-composition> ,
        skos:Concept ;
    rdfs:isDefinedBy <http://anzsoil.org/def/au/asls/substrate> ;
    rdfs:seeAlso <http://anzsoil.org/def/au/asls/substrate> ;
    skos:definition "Mica"@en ;
    skos:inScheme <http://anzsoil.org/def/au/asls/substrate> ;
    skos:notation "M" ;
    skos:prefLabel "Mica"@en ;
    skos:topConceptOf <http://anzsoil.org/def/au/asls/substrate> ;
.

<http://anzsoil.org/def/au/asls/substrate/mineral-composition-Q>
    a
        <http://anzsoil.org/def/au/asls/substrate/Substrate-mineral-composition> ,
        skos:Concept ;
    rdfs:isDefinedBy <http://anzsoil.org/def/au/asls/substrate> ;
    rdfs:seeAlso <http://anzsoil.org/def/au/asls/substrate> ;
    skos:definition "Quartz"@en ;
    skos:inScheme <http://anzsoil.org/def/au/asls/substrate> ;
    skos:notation "Q" ;
    skos:prefLabel "Quartz"@en ;
    skos:topConceptOf <http://anzsoil.org/def/au/asls/substrate> ;
.

<http://anzsoil.org/def/au/asls/substrate/mineral-composition-S>
    a
        <http://anzsoil.org/def/au/asls/substrate/Substrate-mineral-composition> ,
        skos:Concept ;
    dcterms:identifier "http://anzsoil.org/def/au/asls/substrate/mineral-composition-S" ;
    rdfs:isDefinedBy <http://anzsoil.org/def/au/asls/substrate> ;
    rdfs:seeAlso <http://anzsoil.org/def/au/asls/substrate> ;
    skos:definition "Sesquioxides"@en ;
    skos:inScheme <http://anzsoil.org/def/au/asls/substrate> ;
    skos:notation "S" ;
    skos:prefLabel "Sesquioxides"@en ;
    skos:topConceptOf <http://anzsoil.org/def/au/asls/substrate> ;
.

<http://anzsoil.org/def/au/asls/substrate/mineral-composition-Y>
    a
        <http://anzsoil.org/def/au/asls/substrate/Substrate-mineral-composition> ,
        skos:Concept ;
    dcterms:identifier "http://anzsoil.org/def/au/asls/substrate/mineral-composition-Y" ;
    rdfs:isDefinedBy <http://anzsoil.org/def/au/asls/substrate> ;
    rdfs:seeAlso <http://anzsoil.org/def/au/asls/substrate> ;
    skos:definition "Gypsum"@en ;
    skos:inScheme <http://anzsoil.org/def/au/asls/substrate> ;
    skos:notation "Y" ;
    skos:prefLabel "Gypsum"@en ;
    skos:topConceptOf <http://anzsoil.org/def/au/asls/substrate> ;
.

<http://anzsoil.org/def/au/asls/substrate/observation-depth>
    a
        <http://anzsoil.org/def/au/asls/substrate/sampling> ,
        skos:Concept ;
    rdfs:isDefinedBy <http://anzsoil.org/def/au/asls/substrate> ;
    rdfs:seeAlso <http://anzsoil.org/def/au/asls/substrate> ;
    skos:definition "Measure or estimate, in metres, the depth of the point of observation of substrate material below the land surface." ;
    skos:inScheme <http://anzsoil.org/def/au/asls/substrate> ;
    skos:prefLabel "Observation depth"@en ;
    skos:topConceptOf <http://anzsoil.org/def/au/asls/substrate> ;
.

<http://anzsoil.org/def/au/asls/substrate/observation-type-A>
    a
        <http://anzsoil.org/def/au/asls/substrate/type-of-substrate-observation> ,
        skos:Concept ;
    rdfs:isDefinedBy <http://anzsoil.org/def/au/asls/substrate> ;
    rdfs:seeAlso <http://anzsoil.org/def/au/asls/substrate> ;
    skos:definition "Auger boring is used to describe the substrate."@en ;
    skos:inScheme <http://anzsoil.org/def/au/asls/substrate> ;
    skos:notation "A" ;
    skos:prefLabel "Auger boring"@en ;
    skos:topConceptOf <http://anzsoil.org/def/au/asls/substrate> ;
.

<http://anzsoil.org/def/au/asls/substrate/observation-type-C>
    a
        <http://anzsoil.org/def/au/asls/substrate/type-of-substrate-observation> ,
        skos:Concept ;
    rdfs:isDefinedBy <http://anzsoil.org/def/au/asls/substrate> ;
    rdfs:seeAlso <http://anzsoil.org/def/au/asls/substrate> ;
    skos:definition "The substrate is described from a soil core that it relatively undisturbed."@en ;
    skos:inScheme <http://anzsoil.org/def/au/asls/substrate> ;
    skos:notation "C" ;
    skos:prefLabel "Relatively undisturbed soil core"@en ;
    skos:topConceptOf <http://anzsoil.org/def/au/asls/substrate> ;
.

<http://anzsoil.org/def/au/asls/substrate/observation-type-E>
    a
        <http://anzsoil.org/def/au/asls/substrate/type-of-substrate-observation> ,
        skos:Concept ;
    rdfs:isDefinedBy <http://anzsoil.org/def/au/asls/substrate> ;
    rdfs:seeAlso <http://anzsoil.org/def/au/asls/substrate> ;
    skos:definition "An existing vertical exposure (e.g. road cutting) can be used to describe the substrate."@en ;
    skos:inScheme <http://anzsoil.org/def/au/asls/substrate> ;
    skos:notation "E" ;
    skos:prefLabel "Existing vertical exposure"@en ;
    skos:topConceptOf <http://anzsoil.org/def/au/asls/substrate> ;
.

<http://anzsoil.org/def/au/asls/substrate/observation-type-O>
    a
        <http://anzsoil.org/def/au/asls/substrate/type-of-substrate-observation> ,
        skos:Concept ;
    rdfs:isDefinedBy <http://anzsoil.org/def/au/asls/substrate> ;
    rdfs:seeAlso <http://anzsoil.org/def/au/asls/substrate> ;
    skos:definition "Outcrop, where presumed continuous with substrate"@en ;
    skos:inScheme <http://anzsoil.org/def/au/asls/substrate> ;
    skos:notation "O" ;
    skos:prefLabel "Substrate outcrop"@en ;
    skos:topConceptOf <http://anzsoil.org/def/au/asls/substrate> ;
.

<http://anzsoil.org/def/au/asls/substrate/observation-type-P>
    a
        <http://anzsoil.org/def/au/asls/substrate/type-of-substrate-observation> ,
        skos:Concept ;
    rdfs:isDefinedBy <http://anzsoil.org/def/au/asls/substrate> ;
    rdfs:seeAlso <http://anzsoil.org/def/au/asls/substrate> ;
    skos:definition "The soil pit is one of several types of observation used to describe the substrate."@en ;
    skos:inScheme <http://anzsoil.org/def/au/asls/substrate> ;
    skos:notation "P" ;
    skos:prefLabel "Soil pit"@en ;
    skos:topConceptOf <http://anzsoil.org/def/au/asls/substrate> ;
.

<http://anzsoil.org/def/au/asls/substrate/porosity-0>
    a
        <http://anzsoil.org/def/au/asls/substrate/Substrate-porosity> ,
        skos:Concept ;
    rdfs:isDefinedBy <http://anzsoil.org/def/au/asls/substrate> ;
    rdfs:seeAlso <http://anzsoil.org/def/au/asls/substrate> ;
    skos:definition "Non porous, dense"@en ;
    skos:inScheme <http://anzsoil.org/def/au/asls/substrate> ;
    skos:notation "0" ;
    skos:prefLabel "Non porous, dense"@en ;
    skos:topConceptOf <http://anzsoil.org/def/au/asls/substrate> ;
.

<http://anzsoil.org/def/au/asls/substrate/porosity-1>
    a
        <http://anzsoil.org/def/au/asls/substrate/Substrate-porosity> ,
        skos:Concept ;
    rdfs:isDefinedBy <http://anzsoil.org/def/au/asls/substrate> ;
    rdfs:seeAlso <http://anzsoil.org/def/au/asls/substrate> ;
    skos:definition "Slightly porous"@en ;
    skos:inScheme <http://anzsoil.org/def/au/asls/substrate> ;
    skos:notation "1" ;
    skos:prefLabel "Slightly porous"@en ;
    skos:topConceptOf <http://anzsoil.org/def/au/asls/substrate> ;
.

<http://anzsoil.org/def/au/asls/substrate/porosity-2>
    a
        <http://anzsoil.org/def/au/asls/substrate/Substrate-porosity> ,
        skos:Concept ;
    rdfs:isDefinedBy <http://anzsoil.org/def/au/asls/substrate> ;
    rdfs:seeAlso <http://anzsoil.org/def/au/asls/substrate> ;
    skos:definition "Porous "@en ;
    skos:inScheme <http://anzsoil.org/def/au/asls/substrate> ;
    skos:notation "2" ;
    skos:prefLabel "Porous"@en ;
    skos:topConceptOf <http://anzsoil.org/def/au/asls/substrate> ;
.

<http://anzsoil.org/def/au/asls/substrate/sample-distance>
    a skos:Concept ;
    rdfs:isDefinedBy <http://anzsoil.org/def/au/asls/substrate> ;
    rdfs:seeAlso <http://anzsoil.org/def/au/asls/substrate> ;
    skos:definition "Estimate the distance in metres of the point of observation of substrate material from the point of soil observation."@en ;
    skos:inScheme <http://anzsoil.org/def/au/asls/substrate> ;
    skos:prefLabel "Substrate-soil distance"@en ;
    skos:topConceptOf <http://anzsoil.org/def/au/asls/substrate> ;
.

<http://anzsoil.org/def/au/asls/substrate/texture-A>
    a
        <http://anzsoil.org/def/au/asls/substrate/Field-texture> ,
        skos:Concept ;
    rdfs:isDefinedBy <http://anzsoil.org/def/au/asls/substrate> ;
    rdfs:seeAlso <http://anzsoil.org/def/au/asls/substrate> ;
    skos:definition "without visible crystalline or fragmental texture, even through a hand lens." ;
    skos:inScheme <http://anzsoil.org/def/au/asls/substrate> ;
    skos:notation "A" ;
    skos:prefLabel "Amorphous"@en ;
    skos:topConceptOf <http://anzsoil.org/def/au/asls/substrate> ;
.

<http://anzsoil.org/def/au/asls/substrate/texture-F>
    a
        <http://anzsoil.org/def/au/asls/substrate/Field-texture> ,
        skos:Concept ;
    rdfs:isDefinedBy <http://anzsoil.org/def/au/asls/substrate> ;
    rdfs:seeAlso <http://anzsoil.org/def/au/asls/substrate> ;
    skos:definition "consisting of mineral or rock particles that are broken or abraded." ;
    skos:inScheme <http://anzsoil.org/def/au/asls/substrate> ;
    skos:notation "F" ;
    skos:prefLabel "Fragmental"@en ;
    skos:topConceptOf <http://anzsoil.org/def/au/asls/substrate> ;
.

<http://anzsoil.org/def/au/asls/substrate/texture-P>
    a
        <http://anzsoil.org/def/au/asls/substrate/Field-texture> ,
        skos:Concept ;
    rdfs:isDefinedBy <http://anzsoil.org/def/au/asls/substrate> ;
    rdfs:seeAlso <http://anzsoil.org/def/au/asls/substrate> ;
    skos:definition "crystalline, with individual larger crystals in a matrix of much smaller crystals or glass." ;
    skos:inScheme <http://anzsoil.org/def/au/asls/substrate> ;
    skos:notation "P" ;
    skos:prefLabel "Porphyritic"@en ;
    skos:topConceptOf <http://anzsoil.org/def/au/asls/substrate> ;
.

<http://anzsoil.org/def/au/asls/substrate/texture-X>
    a
        <http://anzsoil.org/def/au/asls/substrate/Field-texture> ,
        skos:Concept ;
    rdfs:isDefinedBy <http://anzsoil.org/def/au/asls/substrate> ;
    rdfs:seeAlso <http://anzsoil.org/def/au/asls/substrate> ;
    skos:definition "consisting of interlocking mineral crystals." ;
    skos:inScheme <http://anzsoil.org/def/au/asls/substrate> ;
    skos:notation "X" ;
    skos:prefLabel "Crystalline (non-porphyritic)"@en ;
    skos:topConceptOf <http://anzsoil.org/def/au/asls/substrate> ;
.

geo:hasGeometry
    a
        rdf:Property ,
        rdfs:Resource ,
        owl:ObjectProperty ;
    rdfs:label "hasGeometry"@en ;
    dc:contributor "Matthew Perry" ;
    dc:creator "OGC GeoSPARQL 1.0 Standard Working Group" ;
    dc:date "2011-06-16"^^xsd:date ;
    dc:description """
      A spatial representation for a given feature.
    """@en ;
    rdfs:comment """
      A spatial representation for a given feature.
    """@en ;
    rdfs:domain geo:Feature ;
    rdfs:isDefinedBy
        <http://www.opengis.net/ont/geosparql> ,
        <http://www.opengis.net/spec/geosparql/1.0> ;
    rdfs:range geo:Geometry ;
    rdfs:seeAlso
        <http://www.opengis.net/ont/geosparql> ,
        <http://www.opengis.net/spec/geosparql/1.0> ;
    rdfs:subPropertyOf geo:hasGeometry ;
    skos:definition """
      A spatial representation for a given feature.
    """@en ;
    skos:prefLabel "hasGeometry"@en ;
.

rdfs:seeAlso
    a
        rdf:Property ,
        rdfs:Resource ;
    rdfs:subPropertyOf rdfs:seeAlso ;
.

<http://anzsoil.org/def/au/asls/substrate/genesis-GY>
    a
        <http://anzsoil.org/def/au/asls/substrate/Mass-genetic-type> ,
        <http://anzsoil.org/def/au/asls/substrate/Rock-genesis-hardened-evaporite> ,
        <http://anzsoil.org/def/au/asls/substrate/Rock-genesis-sediments> ,
        skos:Concept ;
    rdfs:isDefinedBy <http://anzsoil.org/def/au/asls/substrate> ;
    rdfs:seeAlso <http://anzsoil.org/def/au/asls/substrate> ;
    skos:definition "evaporite consisting of hydrated calcium sulphate. Non-hydrated calcium sulphate forms closely related masses called anhydrite. It may subsequently be transported by wind as fine crystals and form lunettes or more widespread sedimentary layers blanketing the landscape." ;
    skos:inScheme <http://anzsoil.org/def/au/asls/substrate> ;
    skos:notation "GY" ;
    skos:prefLabel "Gypsum"@en ;
    skos:topConceptOf <http://anzsoil.org/def/au/asls/substrate> ;
.

<http://anzsoil.org/def/au/asls/substrate/lithology-AF>
    a
        <http://anzsoil.org/def/au/asls/substrate/Lithology-rock> ,
        <http://anzsoil.org/def/au/asls/substrate/Lithology-unconsolidated> ,
        skos:Concept ;
    rdfs:isDefinedBy <http://anzsoil.org/def/au/asls/substrate> ;
    rdfs:seeAlso <http://anzsoil.org/def/au/asls/substrate> ;
    skos:definition """Fine grained
0.002-0.06 mm
Volcanic"""@en ;
    skos:inScheme <http://anzsoil.org/def/au/asls/substrate> ;
    skos:notation "AF" ;
    skos:note "C_LITHOLOGY" ;
    skos:prefLabel "Volcanic ash (fine)"@en ;
    skos:topConceptOf <http://anzsoil.org/def/au/asls/substrate> ;
.

<http://anzsoil.org/def/au/asls/substrate/lithology-AS>
    a
        <http://anzsoil.org/def/au/asls/substrate/Lithology-rock> ,
        <http://anzsoil.org/def/au/asls/substrate/Lithology-unconsolidated> ,
        skos:Concept ;
    rdfs:isDefinedBy <http://anzsoil.org/def/au/asls/substrate> ;
    rdfs:seeAlso <http://anzsoil.org/def/au/asls/substrate> ;
    skos:definition """Medium grained
0.06-2 mm
Volcanic"""@en ;
    skos:inScheme <http://anzsoil.org/def/au/asls/substrate> ;
    skos:notation "AS" ;
    skos:note "C_LITHOLOGY" ;
    skos:prefLabel "Volcanic ash (sandy)"@en ;
    skos:topConceptOf <http://anzsoil.org/def/au/asls/substrate> ;
.

<http://anzsoil.org/def/au/asls/substrate/lithology-BB>
    a
        <http://anzsoil.org/def/au/asls/substrate/Lithology-rock> ,
        <http://anzsoil.org/def/au/asls/substrate/Lithology-unconsolidated> ,
        skos:Concept ;
    rdfs:isDefinedBy <http://anzsoil.org/def/au/asls/substrate> ;
    rdfs:seeAlso <http://anzsoil.org/def/au/asls/substrate> ;
    skos:definition """Very coarse grained
>60 mm
Volcanic"""@en ;
    skos:inScheme <http://anzsoil.org/def/au/asls/substrate> ;
    skos:notation "BB" ;
    skos:note "C_LITHOLOGY" ;
    skos:prefLabel "Bombs (or blocks)"@en ;
    skos:topConceptOf <http://anzsoil.org/def/au/asls/substrate> ;
.

<http://anzsoil.org/def/au/asls/substrate/lithology-C>
    a
        <http://anzsoil.org/def/au/asls/substrate/Lithology-rock> ,
        <http://anzsoil.org/def/au/asls/substrate/Lithology-unconsolidated> ,
        skos:Concept ;
    rdfs:isDefinedBy <http://anzsoil.org/def/au/asls/substrate> ;
    rdfs:seeAlso <http://anzsoil.org/def/au/asls/substrate> ;
    skos:definition """Very fine grained
<0.002 mm
Non-volcanic
Without significant carbonate"""@en ;
    skos:inScheme <http://anzsoil.org/def/au/asls/substrate> ;
    skos:notation "C" ;
    skos:note "C_LITHOLOGY" ;
    skos:prefLabel "Clay"@en ;
    skos:topConceptOf <http://anzsoil.org/def/au/asls/substrate> ;
.

<http://anzsoil.org/def/au/asls/substrate/lithology-GV>
    a
        <http://anzsoil.org/def/au/asls/substrate/Lithology-rock> ,
        <http://anzsoil.org/def/au/asls/substrate/Lithology-unconsolidated> ,
        skos:Concept ;
    rdfs:isDefinedBy <http://anzsoil.org/def/au/asls/substrate> ;
    rdfs:seeAlso <http://anzsoil.org/def/au/asls/substrate> ;
    skos:definition """Coarse grained
2-60 mm
Non-volcanic
Without significant carbonate"""@en ;
    skos:inScheme <http://anzsoil.org/def/au/asls/substrate> ;
    skos:notation "GV" ;
    skos:note "C_LITHOLOGY" ;
    skos:prefLabel "Gravel"@en ;
    skos:topConceptOf <http://anzsoil.org/def/au/asls/substrate> ;
.

<http://anzsoil.org/def/au/asls/substrate/lithology-KS>
    a
        <http://anzsoil.org/def/au/asls/substrate/Lithology-rock> ,
        <http://anzsoil.org/def/au/asls/substrate/Lithology-unconsolidated> ,
        skos:Concept ;
    rdfs:isDefinedBy <http://anzsoil.org/def/au/asls/substrate> ;
    rdfs:seeAlso <http://anzsoil.org/def/au/asls/substrate> ;
    skos:definition """Medium grained
0.06-2 mm
Non-volcanic
With significant carbonate"""@en ;
    skos:inScheme <http://anzsoil.org/def/au/asls/substrate> ;
    skos:notation "KS" ;
    skos:note "C_LITHOLOGY" ;
    skos:prefLabel "Calcareous sand"@en ;
    skos:topConceptOf <http://anzsoil.org/def/au/asls/substrate> ;
.

<http://anzsoil.org/def/au/asls/substrate/lithology-ML>
    a
        <http://anzsoil.org/def/au/asls/substrate/Lithology-rock> ,
        <http://anzsoil.org/def/au/asls/substrate/Lithology-unconsolidated> ,
        skos:Concept ;
    rdfs:isDefinedBy <http://anzsoil.org/def/au/asls/substrate> ;
    rdfs:seeAlso <http://anzsoil.org/def/au/asls/substrate> ;
    skos:definition """Very fine grained
<0.002 mm
Non-volcanic
With significant carbonate"""@en ;
    skos:inScheme <http://anzsoil.org/def/au/asls/substrate> ;
    skos:notation "ML" ;
    skos:note "C_LITHOLOGY" ;
    skos:prefLabel "Marl"@en ;
    skos:topConceptOf <http://anzsoil.org/def/au/asls/substrate> ;
.

<http://anzsoil.org/def/au/asls/substrate/lithology-S>
    a
        <http://anzsoil.org/def/au/asls/substrate/Lithology-rock> ,
        <http://anzsoil.org/def/au/asls/substrate/Lithology-unconsolidated> ,
        skos:Concept ;
    rdfs:isDefinedBy <http://anzsoil.org/def/au/asls/substrate> ;
    rdfs:seeAlso <http://anzsoil.org/def/au/asls/substrate> ;
    skos:definition """medium grained
0.06-2 mm
Non-volcanic
Without significant carbonate"""@en ;
    skos:inScheme <http://anzsoil.org/def/au/asls/substrate> ;
    skos:notation "S" ;
    skos:note "C_LITHOLOGY" ;
    skos:prefLabel "Sand"@en ;
    skos:topConceptOf <http://anzsoil.org/def/au/asls/substrate> ;
.

<http://anzsoil.org/def/au/asls/substrate/lithology-SK>
    a
        <http://anzsoil.org/def/au/asls/substrate/Lithology-rock> ,
        <http://anzsoil.org/def/au/asls/substrate/Lithology-unconsolidated> ,
        skos:Concept ;
    rdfs:isDefinedBy <http://anzsoil.org/def/au/asls/substrate> ;
    rdfs:seeAlso <http://anzsoil.org/def/au/asls/substrate> ;
    skos:definition """Coarse grained
2-60 mm
Volcanic"""@en ;
    skos:inScheme <http://anzsoil.org/def/au/asls/substrate> ;
    skos:notation "SK" ;
    skos:note "C_LITHOLOGY" ;
    skos:prefLabel "Scoria"@en ;
    skos:topConceptOf <http://anzsoil.org/def/au/asls/substrate> ;
.

<http://anzsoil.org/def/au/asls/substrate/lithology-Z>
    a
        <http://anzsoil.org/def/au/asls/substrate/Lithology-rock> ,
        <http://anzsoil.org/def/au/asls/substrate/Lithology-unconsolidated> ,
        skos:Concept ;
    rdfs:isDefinedBy <http://anzsoil.org/def/au/asls/substrate> ;
    rdfs:seeAlso <http://anzsoil.org/def/au/asls/substrate> ;
    skos:definition """Silt (Sedimentary rock, detrital)
fine grained
0.002-0.06 mm
Non-volcanic
Without significant carbonate"""@en ;
    skos:inScheme <http://anzsoil.org/def/au/asls/substrate> ;
    skos:notation "Z" ;
    skos:note "C_LITHOLOGY" ;
    skos:prefLabel "Silt"@en ;
    skos:topConceptOf <http://anzsoil.org/def/au/asls/substrate> ;
.

geo:hasSerialization
    a
        rdf:Property ,
        rdfs:Resource ,
        owl:DatatypeProperty ;
    rdfs:label "has serialization"@en ;
    dc:contributor "Matthew Perry" ;
    dc:creator "OGC GeoSPARQL 1.0 Standard Working Group" ;
    dc:date "2011-06-16"^^xsd:date ;
    dc:description """
      Connects a geometry object with its text-based serialization.
    """@en ;
    rdfs:comment """
      Connects a geometry object with its text-based serialization.
    """@en ;
    rdfs:domain geo:Geometry ;
    rdfs:isDefinedBy
        <http://www.opengis.net/ont/geosparql> ,
        <http://www.opengis.net/spec/geosparql/1.0> ;
    rdfs:range rdfs:Literal ;
    rdfs:seeAlso
        <http://www.opengis.net/ont/geosparql> ,
        <http://www.opengis.net/spec/geosparql/1.0> ;
    rdfs:subPropertyOf geo:hasSerialization ;
    skos:definition """
      Connects a geometry object with its text-based serialization.
    """@en ;
    skos:prefLabel "has serialization"@en ;
.

<http://www.opengis.net/ont/geosparql>
    a owl:Ontology ;
    dc:creator "Open Geospatial Consortium" ;
    dc:date "2012-04-30"^^xsd:date ;
    dc:description "An RDF/OWL vocabulary for representing spatial information" ;
    dc:source
        <http://www.opengis.net/doc/IS/geosparql/1.0> ,
        "OGC GeoSPARQL – A Geographic Query Language for RDF Data OGC 11-052r5" ;
    rdfs:seeAlso
        <http://www.opengis.net/def/function/ogc-geosparql/1.0> ,
        <http://www.opengis.net/def/rule/ogc-geosparql/1.0> ,
        <http://www.opengis.net/doc/IS/geosparql/1.0> ;
    owl:imports
        dc: ,
        <http://www.opengis.net/ont/gml> ,
        <http://www.opengis.net/ont/sf> ,
        <http://www.w3.org/2004/02/skos/core> ;
    owl:versionInfo "OGC GeoSPARQL 1.0" ;
.

<http://anzsoil.org/def/au/asls/substrate>
    a
        owl:Ontology ,
        skos:ConceptScheme ;
    dcterms:contributor
        <https://orcid.org/0000-0002-0693-1899> ,
        <https://orcid.org/0000-0002-3884-3420> ;
    dcterms:created "2021-04-07"^^xsd:date ;
    dcterms:creator 
        [
            a schema:Person ;
            schema:email ""^^xsd:anyURI ;
            schema:name "R.C. McDonald" ;
        ] ,
        [
            a schema:Person ;
            schema:email ""^^xsd:anyURI ;
            schema:name "R.F. Isbell" ;
        ] ;
    dcterms:isFormatOf <https://catalogue.nla.gov.au/Record/4273240> ;
    dcterms:modified "2025-06-07"^^xsd:date ;
    dcterms:publisher <https://linked.data.gov.au/org/csiro> ;
    dcterms:rights "copyright CSIRO 2009, 2021. All rights reserved."@en ;
    dcterms:source "National Committee on Soil and Terrain (2009), 'Australian soil and land survey field handbook (3rd edn).' (CSIRO Publishing: Melbourne)"@en ;
    dcterms:title "Substrate classifiers" ;
    rdfs:seeAlso "https://www.publish.csiro.au/book/5230"^^xsd:anyURI ;
    skos:changeNote
        "2022-07-26 - add observable-properties collection" ,
        "2022-07-26 - removed dcterms:description and rdfs:label - duplicates skos:definition and skos:prefLabel" ,
        "2022-07-28 - Completed the rest of the substrate chapter" ,
        "2022-07-29 - replace `sosa:ObservableProperty` type on enumerations with `skos:related` link to the OP in the domain model" ,
        "2022-11-23 - Rename collections for consistency with ANSIS" ,
        "2022-12-07 - remove observable-properties collection" ,
        "2025-06-07 - made VocPub conformant; used prefLabels for missing definitions" ;
    skos:definition """This vocabulary is a machine-readable representation of the classifiers described in chapter 9 Substrate, by R.C. McDonald and R.F. Isbell, in Australian soil and land survey field handbook (3rd edn)

This vocabulary deals with materials and masses of earth or rock that do not show pedological development. They are not soils, but typically underlie them.

This chapter deals with materials and masses of earth (see page 163) or rock that do not show pedological development. They are not soils, but typically underlie them. The substrate includes the R horizon and that part of the C horizon that shows no pedological development (page 106), but excludes the solum, buried soil horizons (including D horizons), and pans. The substrate beneath a soil profile may or may not be the parent material of the soil.

The properties of the substrate should be described as objectively as possible. The first group of properties refers to the material or substance in an intact state, as would be seen in a hand-sized specimen without cracks. Such properties serve to identify the type of rock, such as sandstone, or unconsolidated material, such as clay. A second group of properties comprising spacing of discontinuities, alteration, and mass strength refers to substrate masses. These require observations of areas of greater dimensions. Types of substrate mass are classified mainly according to their inferred origin. Examples are alluvium, parna, ferricrete and saprolite.

The substrate should be observed at the point of the soil profile observation or as close to it as may be practicable. Large vertical exposures of the substrate may reveal the spatial variation of substrate features.""" ;
    skos:hasTopConcept
        <http://anzsoil.org/def/au/asls/substrate/alteration-F> ,
        <http://anzsoil.org/def/au/asls/substrate/alteration-K> ,
        <http://anzsoil.org/def/au/asls/substrate/alteration-L> ,
        <http://anzsoil.org/def/au/asls/substrate/alteration-O> ,
        <http://anzsoil.org/def/au/asls/substrate/alteration-S> ,
        <http://anzsoil.org/def/au/asls/substrate/confidence-certain> ,
        <http://anzsoil.org/def/au/asls/substrate/confidence-doubtful> ,
        <http://anzsoil.org/def/au/asls/substrate/confidence-not-parent> ,
        <http://anzsoil.org/def/au/asls/substrate/confidence-probable> ,
        <http://anzsoil.org/def/au/asls/substrate/discontinuity-spacing-B> ,
        <http://anzsoil.org/def/au/asls/substrate/discontinuity-spacing-C> ,
        <http://anzsoil.org/def/au/asls/substrate/discontinuity-spacing-F> ,
        <http://anzsoil.org/def/au/asls/substrate/discontinuity-spacing-M> ,
        <http://anzsoil.org/def/au/asls/substrate/discontinuity-spacing-S> ,
        <http://anzsoil.org/def/au/asls/substrate/genesis-AC> ,
        <http://anzsoil.org/def/au/asls/substrate/genesis-AL> ,
        <http://anzsoil.org/def/au/asls/substrate/genesis-AT> ,
        <http://anzsoil.org/def/au/asls/substrate/genesis-BE> ,
        <http://anzsoil.org/def/au/asls/substrate/genesis-CD> ,
        <http://anzsoil.org/def/au/asls/substrate/genesis-CN> ,
        <http://anzsoil.org/def/au/asls/substrate/genesis-CO> ,
        <http://anzsoil.org/def/au/asls/substrate/genesis-DR> ,
        <http://anzsoil.org/def/au/asls/substrate/genesis-ED> ,
        <http://anzsoil.org/def/au/asls/substrate/genesis-ES> ,
        <http://anzsoil.org/def/au/asls/substrate/genesis-ET> ,
        <http://anzsoil.org/def/au/asls/substrate/genesis-EV> ,
        <http://anzsoil.org/def/au/asls/substrate/genesis-FC> ,
        <http://anzsoil.org/def/au/asls/substrate/genesis-FI> ,
        <http://anzsoil.org/def/au/asls/substrate/genesis-GY> ,
        <http://anzsoil.org/def/au/asls/substrate/genesis-HA> ,
        <http://anzsoil.org/def/au/asls/substrate/genesis-IG> ,
        <http://anzsoil.org/def/au/asls/substrate/genesis-IN> ,
        <http://anzsoil.org/def/au/asls/substrate/genesis-KC> ,
        <http://anzsoil.org/def/au/asls/substrate/genesis-LA> ,
        <http://anzsoil.org/def/au/asls/substrate/genesis-LC> ,
        <http://anzsoil.org/def/au/asls/substrate/genesis-LD> ,
        <http://anzsoil.org/def/au/asls/substrate/genesis-LO> ,
        <http://anzsoil.org/def/au/asls/substrate/genesis-MA> ,
        <http://anzsoil.org/def/au/asls/substrate/genesis-MD> ,
        <http://anzsoil.org/def/au/asls/substrate/genesis-ME> ,
        <http://anzsoil.org/def/au/asls/substrate/genesis-PA> ,
        <http://anzsoil.org/def/au/asls/substrate/genesis-PC> ,
        <http://anzsoil.org/def/au/asls/substrate/genesis-PL> ,
        <http://anzsoil.org/def/au/asls/substrate/genesis-PW> ,
        <http://anzsoil.org/def/au/asls/substrate/genesis-RB> ,
        <http://anzsoil.org/def/au/asls/substrate/genesis-SA> ,
        <http://anzsoil.org/def/au/asls/substrate/genesis-SC> ,
        <http://anzsoil.org/def/au/asls/substrate/genesis-SD> ,
        <http://anzsoil.org/def/au/asls/substrate/genesis-SE> ,
        <http://anzsoil.org/def/au/asls/substrate/genesis-SH> ,
        <http://anzsoil.org/def/au/asls/substrate/genesis-SP> ,
        <http://anzsoil.org/def/au/asls/substrate/genesis-SR> ,
        <http://anzsoil.org/def/au/asls/substrate/genesis-ST> ,
        <http://anzsoil.org/def/au/asls/substrate/genesis-TI> ,
        <http://anzsoil.org/def/au/asls/substrate/genesis-VA> ,
        <http://anzsoil.org/def/au/asls/substrate/genesis-VO> ,
        <http://anzsoil.org/def/au/asls/substrate/grain-size-1> ,
        <http://anzsoil.org/def/au/asls/substrate/grain-size-2> ,
        <http://anzsoil.org/def/au/asls/substrate/grain-size-3> ,
        <http://anzsoil.org/def/au/asls/substrate/lithology-AC> ,
        <http://anzsoil.org/def/au/asls/substrate/lithology-AD> ,
        <http://anzsoil.org/def/au/asls/substrate/lithology-AF> ,
        <http://anzsoil.org/def/au/asls/substrate/lithology-AG> ,
        <http://anzsoil.org/def/au/asls/substrate/lithology-AH> ,
        <http://anzsoil.org/def/au/asls/substrate/lithology-AM> ,
        <http://anzsoil.org/def/au/asls/substrate/lithology-AN> ,
        <http://anzsoil.org/def/au/asls/substrate/lithology-AP> ,
        <http://anzsoil.org/def/au/asls/substrate/lithology-AR> ,
        <http://anzsoil.org/def/au/asls/substrate/lithology-AS> ,
        <http://anzsoil.org/def/au/asls/substrate/lithology-BA> ,
        <http://anzsoil.org/def/au/asls/substrate/lithology-BB> ,
        <http://anzsoil.org/def/au/asls/substrate/lithology-BO> ,
        <http://anzsoil.org/def/au/asls/substrate/lithology-BR> ,
        <http://anzsoil.org/def/au/asls/substrate/lithology-C> ,
        <http://anzsoil.org/def/au/asls/substrate/lithology-CB> ,
        <http://anzsoil.org/def/au/asls/substrate/lithology-CG> ,
        <http://anzsoil.org/def/au/asls/substrate/lithology-CH> ,
        <http://anzsoil.org/def/au/asls/substrate/lithology-CO> ,
        <http://anzsoil.org/def/au/asls/substrate/lithology-CU> ,
        <http://anzsoil.org/def/au/asls/substrate/lithology-DI> ,
        <http://anzsoil.org/def/au/asls/substrate/lithology-DM> ,
        <http://anzsoil.org/def/au/asls/substrate/lithology-DR> ,
        <http://anzsoil.org/def/au/asls/substrate/lithology-FC> ,
        <http://anzsoil.org/def/au/asls/substrate/lithology-GA> ,
        <http://anzsoil.org/def/au/asls/substrate/lithology-GD> ,
        <http://anzsoil.org/def/au/asls/substrate/lithology-GE> ,
        <http://anzsoil.org/def/au/asls/substrate/lithology-GN> ,
        <http://anzsoil.org/def/au/asls/substrate/lithology-GR> ,
        <http://anzsoil.org/def/au/asls/substrate/lithology-GS> ,
        <http://anzsoil.org/def/au/asls/substrate/lithology-GV> ,
        <http://anzsoil.org/def/au/asls/substrate/lithology-GW> ,
        <http://anzsoil.org/def/au/asls/substrate/lithology-GY> ,
        <http://anzsoil.org/def/au/asls/substrate/lithology-HA> ,
        <http://anzsoil.org/def/au/asls/substrate/lithology-HO> ,
        <http://anzsoil.org/def/au/asls/substrate/lithology-IG> ,
        <http://anzsoil.org/def/au/asls/substrate/lithology-JA> ,
        <http://anzsoil.org/def/au/asls/substrate/lithology-KA> ,
        <http://anzsoil.org/def/au/asls/substrate/lithology-KC> ,
        <http://anzsoil.org/def/au/asls/substrate/lithology-KL> ,
        <http://anzsoil.org/def/au/asls/substrate/lithology-KM> ,
        <http://anzsoil.org/def/au/asls/substrate/lithology-KR> ,
        <http://anzsoil.org/def/au/asls/substrate/lithology-KS> ,
        <http://anzsoil.org/def/au/asls/substrate/lithology-LC> ,
        <http://anzsoil.org/def/au/asls/substrate/lithology-LI> ,
        <http://anzsoil.org/def/au/asls/substrate/lithology-M> ,
        <http://anzsoil.org/def/au/asls/substrate/lithology-MB> ,
        <http://anzsoil.org/def/au/asls/substrate/lithology-MD> ,
        <http://anzsoil.org/def/au/asls/substrate/lithology-ME> ,
        <http://anzsoil.org/def/au/asls/substrate/lithology-MG> ,
        <http://anzsoil.org/def/au/asls/substrate/lithology-MI> ,
        <http://anzsoil.org/def/au/asls/substrate/lithology-ML> ,
        <http://anzsoil.org/def/au/asls/substrate/lithology-MS> ,
        <http://anzsoil.org/def/au/asls/substrate/lithology-MU> ,
        <http://anzsoil.org/def/au/asls/substrate/lithology-MY> ,
        <http://anzsoil.org/def/au/asls/substrate/lithology-PC> ,
        <http://anzsoil.org/def/au/asls/substrate/lithology-PE> ,
        <http://anzsoil.org/def/au/asls/substrate/lithology-PG> ,
        <http://anzsoil.org/def/au/asls/substrate/lithology-PH> ,
        <http://anzsoil.org/def/au/asls/substrate/lithology-PL> ,
        <http://anzsoil.org/def/au/asls/substrate/lithology-PO> ,
        <http://anzsoil.org/def/au/asls/substrate/lithology-PY> ,
        <http://anzsoil.org/def/au/asls/substrate/lithology-QP> ,
        <http://anzsoil.org/def/au/asls/substrate/lithology-QS> ,
        <http://anzsoil.org/def/au/asls/substrate/lithology-QU> ,
        <http://anzsoil.org/def/au/asls/substrate/lithology-QZ> ,
        <http://anzsoil.org/def/au/asls/substrate/lithology-R> ,
        <http://anzsoil.org/def/au/asls/substrate/lithology-RB> ,
        <http://anzsoil.org/def/au/asls/substrate/lithology-RH> ,
        <http://anzsoil.org/def/au/asls/substrate/lithology-S> ,
        <http://anzsoil.org/def/au/asls/substrate/lithology-SA> ,
        <http://anzsoil.org/def/au/asls/substrate/lithology-SD> ,
        <http://anzsoil.org/def/au/asls/substrate/lithology-SH> ,
        <http://anzsoil.org/def/au/asls/substrate/lithology-SK> ,
        <http://anzsoil.org/def/au/asls/substrate/lithology-SL> ,
        <http://anzsoil.org/def/au/asls/substrate/lithology-SN> ,
        <http://anzsoil.org/def/au/asls/substrate/lithology-SR> ,
        <http://anzsoil.org/def/au/asls/substrate/lithology-ST> ,
        <http://anzsoil.org/def/au/asls/substrate/lithology-SY> ,
        <http://anzsoil.org/def/au/asls/substrate/lithology-TR> ,
        <http://anzsoil.org/def/au/asls/substrate/lithology-TU> ,
        <http://anzsoil.org/def/au/asls/substrate/lithology-UC> ,
        <http://anzsoil.org/def/au/asls/substrate/lithology-VB> ,
        <http://anzsoil.org/def/au/asls/substrate/lithology-VG> ,
        <http://anzsoil.org/def/au/asls/substrate/lithology-Z> ,
        <http://anzsoil.org/def/au/asls/substrate/lithology-ZS> ,
        <http://anzsoil.org/def/au/asls/substrate/material-strength-M> ,
        <http://anzsoil.org/def/au/asls/substrate/material-strength-S> ,
        <http://anzsoil.org/def/au/asls/substrate/material-strength-VS> ,
        <http://anzsoil.org/def/au/asls/substrate/material-strength-VW> ,
        <http://anzsoil.org/def/au/asls/substrate/material-strength-W> ,
        <http://anzsoil.org/def/au/asls/substrate/material-structure-B> ,
        <http://anzsoil.org/def/au/asls/substrate/material-structure-C> ,
        <http://anzsoil.org/def/au/asls/substrate/material-structure-F> ,
        <http://anzsoil.org/def/au/asls/substrate/material-structure-L> ,
        <http://anzsoil.org/def/au/asls/substrate/material-structure-P> ,
        <http://anzsoil.org/def/au/asls/substrate/material-structure-R> ,
        <http://anzsoil.org/def/au/asls/substrate/material-structure-S> ,
        <http://anzsoil.org/def/au/asls/substrate/material-structure-V> ,
        <http://anzsoil.org/def/au/asls/substrate/mineral-composition-C> ,
        <http://anzsoil.org/def/au/asls/substrate/mineral-composition-D> ,
        <http://anzsoil.org/def/au/asls/substrate/mineral-composition-F> ,
        <http://anzsoil.org/def/au/asls/substrate/mineral-composition-G> ,
        <http://anzsoil.org/def/au/asls/substrate/mineral-composition-K> ,
        <http://anzsoil.org/def/au/asls/substrate/mineral-composition-L> ,
        <http://anzsoil.org/def/au/asls/substrate/mineral-composition-M> ,
        <http://anzsoil.org/def/au/asls/substrate/mineral-composition-Q> ,
        <http://anzsoil.org/def/au/asls/substrate/mineral-composition-S> ,
        <http://anzsoil.org/def/au/asls/substrate/mineral-composition-Y> ,
        <http://anzsoil.org/def/au/asls/substrate/observation-depth> ,
        <http://anzsoil.org/def/au/asls/substrate/observation-type-A> ,
        <http://anzsoil.org/def/au/asls/substrate/observation-type-C> ,
        <http://anzsoil.org/def/au/asls/substrate/observation-type-E> ,
        <http://anzsoil.org/def/au/asls/substrate/observation-type-O> ,
        <http://anzsoil.org/def/au/asls/substrate/observation-type-P> ,
        <http://anzsoil.org/def/au/asls/substrate/porosity-0> ,
        <http://anzsoil.org/def/au/asls/substrate/porosity-1> ,
        <http://anzsoil.org/def/au/asls/substrate/porosity-2> ,
        <http://anzsoil.org/def/au/asls/substrate/sample-distance> ,
        <http://anzsoil.org/def/au/asls/substrate/texture-A> ,
        <http://anzsoil.org/def/au/asls/substrate/texture-F> ,
        <http://anzsoil.org/def/au/asls/substrate/texture-P> ,
        <http://anzsoil.org/def/au/asls/substrate/texture-X> ;
    skos:historyNote "The data was converted from the print representation to this linked-data form by Linda Gregory assisted by Simon J D Cox" ;
    skos:notation "substrate"@en ;
    skos:prefLabel "Substrate classifiers"@en ;
    schema:license <http://purl.org/NET/rdflicense/cc-by4.0> ;
.
